@prefix cskg-ont: <http://scholkg.kmi.open.ac.uk/cskg/ontology#> .
@prefix owl: <http://www.w3.org/2002/07/owl#> .
@prefix rdf: <http://www.w3.org/1999/02/22-rdf-syntax-ns#> .
@prefix rdfs: <http://www.w3.org/2000/01/rdf-schema#> .

cskg-ont:CSOTopic a owl:Class ;
    rdfs:comment "A Topic of the Computer Science Ontology" .

cskg-ont:MagPaper a owl:Class ;
    rdfs:comment "A paper indexed in the Microsoft Academic Graph dataset" .

cskg-ont:Wikidata a owl:Class ;
    rdfs:comment "An entry of Wikidata" .

cskg-ont:hasSupport a owl:DatatypeProperty ;
    rdfs:comment "This property indicates the number of papers from where the predicate between subject and object comes from." ;
    rdfs:domain cskg-ont:Statement ;
    rdfs:range rdfs:Literal .

cskg-ont:isInferredByTransitivity a owl:DatatypeProperty ;
    rdfs:comment "This property indicates if the statement was inferred by transitivity. If 'false' it means that it was derived directly from the papers. If 'true' it means that it was inferred when computing the transitive closure of AI-KG." ;
    rdfs:domain cskg-ont:Statement ;
    rdfs:range rdfs:Literal .

cskg-ont:isInverse a owl:DatatypeProperty ;
    rdfs:comment "This property indicates if the statement was derived by inferring the inverse relation of a relation originally extracted from the corpus of paper." ;
    rdfs:domain cskg-ont:Statement ;
    rdfs:range rdfs:Literal .

cskg-ont:acquiresMaterial a owl:ObjectProperty ;
    rdfs:comment "This relation indicates that an instance belonging to one class in { Method, OtherEntity, Task } acquires an instance of  Material. It is designed based on the following predicates extracted by the NLP pipeline: select,accumulate,recoup,source,receive,acquire,regain,retrieve,obtain,accrue,borrow,subselect,inherit,accept,collect,gather,store,attract,get,capture,record,achieve" ;
    rdfs:domain _:N1f3d128b6fda402dbc1b86103dfda554 ;
    rdfs:range cskg-ont:Material ;
    rdfs:subPropertyOf cskg-ont:acquires ;
    owl:inverseOf cskg-ont:materialAcquiredBy .

cskg-ont:acquiresMethod a owl:ObjectProperty,
        owl:TransitiveProperty ;
    rdfs:comment "This relation indicates that an instance belonging to one class in { Method, OtherEntity, Task } acquires an instance of  Method. It is designed based on the following predicates extracted by the NLP pipeline: select,accumulate,recoup,source,receive,acquire,regain,retrieve,obtain,accrue,borrow,subselect,inherit,accept,collect,gather,store,attract,get,capture,record,achieve" ;
    rdfs:domain _:Nb537d70acb5d4f7b83ce9774ba62ee76 ;
    rdfs:range cskg-ont:Method ;
    rdfs:subPropertyOf cskg-ont:acquires ;
    owl:inverseOf cskg-ont:methodAcquiredBy .

cskg-ont:acquiresMetric a owl:ObjectProperty ;
    rdfs:comment "This relation indicates that an instance belonging to one class in { Method, OtherEntity, Task } acquires an instance of  Metric. It is designed based on the following predicates extracted by the NLP pipeline: select,accumulate,recoup,source,receive,acquire,regain,retrieve,obtain,accrue,borrow,subselect,inherit,accept,collect,gather,store,attract,get,capture,record,achieve" ;
    rdfs:domain _:Ne250491a99094a61a35c8792c5f8c59c ;
    rdfs:range cskg-ont:Metric ;
    rdfs:subPropertyOf cskg-ont:acquires ;
    owl:inverseOf cskg-ont:metricAcquiredBy .

cskg-ont:acquiresOtherEntity a owl:ObjectProperty,
        owl:TransitiveProperty ;
    rdfs:comment "This relation indicates that an instance belonging to one class in { Method, OtherEntity, Task } acquires an instance of  OtherEntity. It is designed based on the following predicates extracted by the NLP pipeline: select,accumulate,recoup,source,receive,acquire,regain,retrieve,obtain,accrue,borrow,subselect,inherit,accept,collect,gather,store,attract,get,capture,record,achieve" ;
    rdfs:domain _:N1457e755bb5841c594cfec96662ad8f6 ;
    rdfs:range cskg-ont:OtherEntity ;
    rdfs:subPropertyOf cskg-ont:acquires ;
    owl:inverseOf cskg-ont:otherentityAcquiredBy .

cskg-ont:acquiresTask a owl:ObjectProperty,
        owl:TransitiveProperty ;
    rdfs:comment "This relation indicates that an instance belonging to one class in { Method, Task } acquires an instance of  Task. It is designed based on the following predicates extracted by the NLP pipeline: select,accumulate,recoup,source,receive,acquire,regain,retrieve,obtain,accrue,borrow,subselect,inherit,accept,collect,gather,store,attract,get,capture,record,achieve" ;
    rdfs:domain _:N35e6671791614fab9c31cbb63e75adba ;
    rdfs:range cskg-ont:Task ;
    rdfs:subPropertyOf cskg-ont:acquires ;
    owl:inverseOf cskg-ont:taskAcquiredBy .

cskg-ont:adaptsMaterial a owl:ObjectProperty ;
    rdfs:comment "This relation indicates that an instance belonging to one class in { Method, OtherEntity, Task } adapts an instance of  Material. It is designed based on the following predicates extracted by the NLP pipeline: readapt,adjust,conform,adapt,gear,readjust,fit,assimilate,accommodate,personalize,customize,specialize,generalize,tailor,refine" ;
    rdfs:domain _:N8653196663b34e288e5950f343e490a8 ;
    rdfs:range cskg-ont:Material ;
    rdfs:subPropertyOf cskg-ont:adapts ;
    owl:inverseOf cskg-ont:materialAdaptedBy .

cskg-ont:adaptsMethod a owl:ObjectProperty,
        owl:TransitiveProperty ;
    rdfs:comment "This relation indicates that an instance belonging to one class in { Method, OtherEntity, Task } adapts an instance of  Method. It is designed based on the following predicates extracted by the NLP pipeline: readapt,adjust,conform,adapt,gear,readjust,fit,assimilate,accommodate,personalize,customize,specialize,generalize,tailor,refine" ;
    rdfs:domain _:N76f3d2c578754615a35c5ed25ed29481 ;
    rdfs:range cskg-ont:Method ;
    rdfs:subPropertyOf cskg-ont:adapts ;
    owl:inverseOf cskg-ont:methodAdaptedBy .

cskg-ont:adaptsMetric a owl:ObjectProperty ;
    rdfs:comment "This relation indicates that an instance belonging to one class in { Method, OtherEntity, Task } adapts an instance of  Metric. It is designed based on the following predicates extracted by the NLP pipeline: readapt,adjust,conform,adapt,gear,readjust,fit,assimilate,accommodate,personalize,customize,specialize,generalize,tailor,refine" ;
    rdfs:domain _:N1f6623cc3bef4f9e98932345e573de01 ;
    rdfs:range cskg-ont:Metric ;
    rdfs:subPropertyOf cskg-ont:adapts ;
    owl:inverseOf cskg-ont:metricAdaptedBy .

cskg-ont:adaptsOtherEntity a owl:ObjectProperty,
        owl:TransitiveProperty ;
    rdfs:comment "This relation indicates that an instance belonging to one class in { Method, OtherEntity, Task } adapts an instance of  OtherEntity. It is designed based on the following predicates extracted by the NLP pipeline: readapt,adjust,conform,adapt,gear,readjust,fit,assimilate,accommodate,personalize,customize,specialize,generalize,tailor,refine" ;
    rdfs:domain _:Na677c9cf1eec4b199058fa4c7497de9a ;
    rdfs:range cskg-ont:OtherEntity ;
    rdfs:subPropertyOf cskg-ont:adapts ;
    owl:inverseOf cskg-ont:otherentityAdaptedBy .

cskg-ont:adaptsTask a owl:ObjectProperty,
        owl:TransitiveProperty ;
    rdfs:comment "This relation indicates that an instance belonging to one class in { Method, OtherEntity, Task } adapts an instance of  Task. It is designed based on the following predicates extracted by the NLP pipeline: readapt,adjust,conform,adapt,gear,readjust,fit,assimilate,accommodate,personalize,customize,specialize,generalize,tailor,refine" ;
    rdfs:domain _:Nbad3c5cc49e541bcab922a7e6e1576e7 ;
    rdfs:range cskg-ont:Task ;
    rdfs:subPropertyOf cskg-ont:adapts ;
    owl:inverseOf cskg-ont:taskAdaptedBy .

cskg-ont:affectsMaterial a owl:ObjectProperty ;
    rdfs:comment "This relation indicates that an instance belonging to one class in { Material, Method, OtherEntity, Task } affects an instance of  Material. It is designed based on the following predicates extracted by the NLP pipeline: placate,provoke,engage,console,impair,repulse,shake,discombobulate,threaten,inflame,thrill,satisfy,unsettle,kill,enrapture,outrage,disgruntle,reassure,discompose,interest,alarm,engross,afflict,manipulate,edit,update,increase,replace,modify,fatigue,refresh,cut" ;
    rdfs:domain _:N4a044612beb04386bcdaada212d06ee5 ;
    rdfs:range cskg-ont:Material ;
    rdfs:subPropertyOf cskg-ont:affects ;
    owl:inverseOf cskg-ont:materialAffectedBy .

cskg-ont:affectsMethod a owl:ObjectProperty ;
    rdfs:comment "This relation indicates that an instance belonging to one class in { Method, Metric, OtherEntity, Task } affects an instance of  Method. It is designed based on the following predicates extracted by the NLP pipeline: placate,provoke,engage,console,impair,repulse,shake,discombobulate,threaten,inflame,thrill,satisfy,unsettle,kill,enrapture,outrage,disgruntle,reassure,discompose,interest,alarm,engross,afflict,manipulate,edit,update,increase,replace,modify,fatigue,refresh,cut" ;
    rdfs:domain _:N1bb86d25c9754b338b0a373bccca95bf ;
    rdfs:range cskg-ont:Method ;
    rdfs:subPropertyOf cskg-ont:affects ;
    owl:inverseOf cskg-ont:methodAffectedBy .

cskg-ont:affectsMetric a owl:ObjectProperty ;
    rdfs:comment "This relation indicates that an instance belonging to one class in { Method, Metric, OtherEntity, Task } affects an instance of  Metric. It is designed based on the following predicates extracted by the NLP pipeline: placate,provoke,engage,console,impair,repulse,shake,discombobulate,threaten,inflame,thrill,satisfy,unsettle,kill,enrapture,outrage,disgruntle,reassure,discompose,interest,alarm,engross,afflict,manipulate,edit,update,increase,replace,modify,fatigue,refresh,cut" ;
    rdfs:domain _:N1802d0de86f3405b9653a79f47cac09e ;
    rdfs:range cskg-ont:Metric ;
    rdfs:subPropertyOf cskg-ont:affects ;
    owl:inverseOf cskg-ont:metricAffectedBy .

cskg-ont:affectsOtherEntity a owl:ObjectProperty ;
    rdfs:comment "This relation indicates that an instance belonging to one class in { Material, Method, Metric, OtherEntity, Task } affects an instance of  OtherEntity. It is designed based on the following predicates extracted by the NLP pipeline: placate,provoke,engage,console,impair,repulse,shake,discombobulate,threaten,inflame,thrill,satisfy,unsettle,kill,enrapture,outrage,disgruntle,reassure,discompose,interest,alarm,engross,afflict,manipulate,edit,update,increase,replace,modify,fatigue,refresh,cut" ;
    rdfs:domain _:Nc42629e2ebbf4afd9c50c37db59f9d93 ;
    rdfs:range cskg-ont:OtherEntity ;
    rdfs:subPropertyOf cskg-ont:affects ;
    owl:inverseOf cskg-ont:otherentityAffectedBy .

cskg-ont:affectsTask a owl:ObjectProperty ;
    rdfs:comment "This relation indicates that an instance belonging to one class in { Method, Metric, OtherEntity, Task } affects an instance of  Task. It is designed based on the following predicates extracted by the NLP pipeline: placate,provoke,engage,console,impair,repulse,shake,discombobulate,threaten,inflame,thrill,satisfy,unsettle,kill,enrapture,outrage,disgruntle,reassure,discompose,interest,alarm,engross,afflict,manipulate,edit,update,increase,replace,modify,fatigue,refresh,cut" ;
    rdfs:domain _:N1067ae94682b42c18653eadaac85deff ;
    rdfs:range cskg-ont:Task ;
    rdfs:subPropertyOf cskg-ont:affects ;
    owl:inverseOf cskg-ont:taskAffectedBy .

cskg-ont:analyzesMaterial a owl:ObjectProperty ;
    rdfs:comment "This relation indicates that an instance belonging to one class in { Method, Metric, OtherEntity, Task } analyzes an instance of  Material. It is designed based on the following predicates extracted by the NLP pipeline: analyze,assess,study,try_on,scan,approximate,proofread,inspect,sample,research,check,appraise,analyse,examine,watch,audit,feel_out,go_over,consult,survey,test,assay,try,evaluate,investigate,monitor,regard,peruse,review,try_out,measure,calculate,address,estimate" ;
    rdfs:domain _:Ne5f8f2eed38342769aec9a55551ff1a3 ;
    rdfs:range cskg-ont:Material ;
    rdfs:subPropertyOf cskg-ont:analyzes ;
    owl:inverseOf cskg-ont:materialAnalyzedBy .

cskg-ont:analyzesMethod a owl:ObjectProperty,
        owl:TransitiveProperty ;
    rdfs:comment "This relation indicates that an instance belonging to one class in { Method, Metric, OtherEntity, Task } analyzes an instance of  Method. It is designed based on the following predicates extracted by the NLP pipeline: analyze,assess,study,try_on,scan,approximate,proofread,inspect,sample,research,check,appraise,analyse,examine,watch,audit,feel_out,go_over,consult,survey,test,assay,try,evaluate,investigate,monitor,regard,peruse,review,try_out,measure,calculate,address,estimate" ;
    rdfs:domain _:N78e421076cfc4a1ea744c6a381116451 ;
    rdfs:range cskg-ont:Method ;
    rdfs:subPropertyOf cskg-ont:analyzes ;
    owl:inverseOf cskg-ont:methodAnalyzedBy .

cskg-ont:analyzesMetric a owl:ObjectProperty ;
    rdfs:comment "This relation indicates that an instance belonging to one class in { Method, Metric, OtherEntity, Task } analyzes an instance of  Metric. It is designed based on the following predicates extracted by the NLP pipeline: analyze,assess,study,try_on,scan,approximate,proofread,inspect,sample,research,check,appraise,analyse,examine,watch,audit,feel_out,go_over,consult,survey,test,assay,try,evaluate,investigate,monitor,regard,peruse,review,try_out,measure,calculate,address,estimate" ;
    rdfs:domain _:N58074e7205704ced9fcc9e9a6a38b145 ;
    rdfs:range cskg-ont:Metric ;
    rdfs:subPropertyOf cskg-ont:analyzes ;
    owl:inverseOf cskg-ont:metricAnalyzedBy .

cskg-ont:analyzesOtherEntity a owl:ObjectProperty,
        owl:TransitiveProperty ;
    rdfs:comment "This relation indicates that an instance belonging to one class in { Method, Metric, OtherEntity, Task } analyzes an instance of  OtherEntity. It is designed based on the following predicates extracted by the NLP pipeline: analyze,assess,study,try_on,scan,approximate,proofread,inspect,sample,research,check,appraise,analyse,examine,watch,audit,feel_out,go_over,consult,survey,test,assay,try,evaluate,investigate,monitor,regard,peruse,review,try_out,measure,calculate,address,estimate" ;
    rdfs:domain _:N4546f13a64de4f31ae43d05836a73544 ;
    rdfs:range cskg-ont:OtherEntity ;
    rdfs:subPropertyOf cskg-ont:analyzes ;
    owl:inverseOf cskg-ont:otherentityAnalyzedBy .

cskg-ont:analyzesTask a owl:ObjectProperty,
        owl:TransitiveProperty ;
    rdfs:comment "This relation indicates that an instance belonging to one class in { Method, Metric, Task } analyzes an instance of  Task. It is designed based on the following predicates extracted by the NLP pipeline: analyze,assess,study,try_on,scan,approximate,proofread,inspect,sample,research,check,appraise,analyse,examine,watch,audit,feel_out,go_over,consult,survey,test,assay,try,evaluate,investigate,monitor,regard,peruse,review,try_out,measure,calculate,address,estimate" ;
    rdfs:domain _:N7b2ed255dc74415284c07048e5bd44cf ;
    rdfs:range cskg-ont:Task ;
    rdfs:subPropertyOf cskg-ont:analyzes ;
    owl:inverseOf cskg-ont:taskAnalyzedBy .

cskg-ont:annotatesMaterial a owl:ObjectProperty ;
    rdfs:comment "This relation indicates that an instance belonging to one class in { Method, Metric, OtherEntity, Task } annotates an instance of  Material. It is designed based on the following predicates extracted by the NLP pipeline: scar,stipple,annotate,stamp,embroider,incise,inscribe,engrave,applique,imprint,paint,reinscribe,mark,sign,tag,label" ;
    rdfs:domain _:Nba6a0d4144a14fc188678d3c3fff1a40 ;
    rdfs:range cskg-ont:Material ;
    rdfs:subPropertyOf cskg-ont:annotates ;
    owl:inverseOf cskg-ont:materialAnnotatedBy .

cskg-ont:annotatesMethod a owl:ObjectProperty ;
    rdfs:comment "This relation indicates that an instance belonging to one class in { Method, Task } annotates an instance of  Method. It is designed based on the following predicates extracted by the NLP pipeline: scar,stipple,annotate,stamp,embroider,incise,inscribe,engrave,applique,imprint,paint,reinscribe,mark,sign,tag,label" ;
    rdfs:domain _:N325b3b8c68e44ac286527bae7a46fc96 ;
    rdfs:range cskg-ont:Method ;
    rdfs:subPropertyOf cskg-ont:annotates ;
    owl:inverseOf cskg-ont:methodAnnotatedBy .

cskg-ont:annotatesOtherEntity a owl:ObjectProperty ;
    rdfs:comment "This relation indicates that an instance belonging to one class in { Method, OtherEntity } annotates an instance of  OtherEntity. It is designed based on the following predicates extracted by the NLP pipeline: scar,stipple,annotate,stamp,embroider,incise,inscribe,engrave,applique,imprint,paint,reinscribe,mark,sign,tag,label" ;
    rdfs:domain _:Na3b25ebacb6c48179625b2df35224994 ;
    rdfs:range cskg-ont:OtherEntity ;
    rdfs:subPropertyOf cskg-ont:annotates ;
    owl:inverseOf cskg-ont:otherentityAnnotatedBy .

cskg-ont:annotatesTask a owl:ObjectProperty ;
    rdfs:comment "This relation indicates that an instance belonging to one class in { Method, Task } annotates an instance of  Task. It is designed based on the following predicates extracted by the NLP pipeline: scar,stipple,annotate,stamp,embroider,incise,inscribe,engrave,applique,imprint,paint,reinscribe,mark,sign,tag,label" ;
    rdfs:domain _:Nf0d2aa6e99b04ae6944e92df8712aec0 ;
    rdfs:range cskg-ont:Task ;
    rdfs:subPropertyOf cskg-ont:annotates ;
    owl:inverseOf cskg-ont:taskAnnotatedBy .

cskg-ont:automatesMethod a owl:ObjectProperty ;
    rdfs:comment "This relation indicates that an instance belonging to one class in { Method, Task } automates an instance of  Method. It is designed based on the following predicates extracted by the NLP pipeline: automate" ;
    rdfs:domain _:N8207716fbb6a4c14a67b17f93eb075d0 ;
    rdfs:range cskg-ont:Method ;
    rdfs:subPropertyOf cskg-ont:automates ;
    owl:inverseOf cskg-ont:methodAutomatedBy .

cskg-ont:automatesOtherEntity a owl:ObjectProperty ;
    rdfs:comment "This relation indicates that an instance belonging to one class in { Method, OtherEntity } automates an instance of  OtherEntity. It is designed based on the following predicates extracted by the NLP pipeline: automate" ;
    rdfs:domain _:N0dfe945b3ba44539b8d155270cf03b90 ;
    rdfs:range cskg-ont:OtherEntity ;
    rdfs:subPropertyOf cskg-ont:automates ;
    owl:inverseOf cskg-ont:otherentityAutomatedBy .

cskg-ont:automatesTask a owl:ObjectProperty ;
    rdfs:comment "This relation indicates that an instance belonging to one class in { Method, OtherEntity } automates an instance of  Task. It is designed based on the following predicates extracted by the NLP pipeline: automate" ;
    rdfs:domain _:N2aa6a5f8122f449185ed52bbf0a15b7f ;
    rdfs:range cskg-ont:Task ;
    rdfs:subPropertyOf cskg-ont:automates ;
    owl:inverseOf cskg-ont:taskAutomatedBy .

cskg-ont:based-onMaterial a owl:ObjectProperty,
        owl:TransitiveProperty ;
    rdfs:comment "This relation indicates that an instance belonging to one class in { Material, Method, Metric, OtherEntity, Task } based-on an instance of  Material. It is designed based on the following predicates extracted by the NLP pipeline: base,ground,found,construe,build,establish" ;
    rdfs:domain _:Ne7974f69047f4510883a7ef0862ea28f ;
    rdfs:range cskg-ont:Material ;
    rdfs:subPropertyOf cskg-ont:based-on ;
    owl:inverseOf cskg-ont:materialBases .

cskg-ont:based-onMethod a owl:ObjectProperty,
        owl:TransitiveProperty ;
    rdfs:comment "This relation indicates that an instance belonging to one class in { Material, Method, Metric, OtherEntity, Task } based-on an instance of  Method. It is designed based on the following predicates extracted by the NLP pipeline: base,ground,found,construe,build,establish" ;
    rdfs:domain _:N08fd05694b3f44ebb87a0f020839acee ;
    rdfs:range cskg-ont:Method ;
    rdfs:subPropertyOf cskg-ont:based-on ;
    owl:inverseOf cskg-ont:methodBases .

cskg-ont:based-onMetric a owl:ObjectProperty,
        owl:TransitiveProperty ;
    rdfs:comment "This relation indicates that an instance belonging to one class in { Material, Method, Metric, OtherEntity, Task } based-on an instance of  Metric. It is designed based on the following predicates extracted by the NLP pipeline: base,ground,found,construe,build,establish" ;
    rdfs:domain _:N3affbed2bf194787b6196c968430d26c ;
    rdfs:range cskg-ont:Metric ;
    rdfs:subPropertyOf cskg-ont:based-on ;
    owl:inverseOf cskg-ont:metricBases .

cskg-ont:based-onOtherEntity a owl:ObjectProperty,
        owl:TransitiveProperty ;
    rdfs:comment "This relation indicates that an instance belonging to one class in { Material, Method, Metric, OtherEntity, Task } based-on an instance of  OtherEntity. It is designed based on the following predicates extracted by the NLP pipeline: base,ground,found,construe,build,establish" ;
    rdfs:domain _:Ndc503fa6ad354569a9c6b9e17e337ef8 ;
    rdfs:range cskg-ont:OtherEntity ;
    rdfs:subPropertyOf cskg-ont:based-on ;
    owl:inverseOf cskg-ont:otherentityBases .

cskg-ont:based-onTask a owl:ObjectProperty,
        owl:TransitiveProperty ;
    rdfs:comment "This relation indicates that an instance belonging to one class in { Material, Method, Metric, OtherEntity, Task } based-on an instance of  Task. It is designed based on the following predicates extracted by the NLP pipeline: base,ground,found,construe,build,establish" ;
    rdfs:domain _:Ne8dc2f8964064602885a66d293f855e5 ;
    rdfs:range cskg-ont:Task ;
    rdfs:subPropertyOf cskg-ont:based-on ;
    owl:inverseOf cskg-ont:taskBases .

cskg-ont:causesMaterial a owl:ObjectProperty ;
    rdfs:comment "This relation indicates that an instance belonging to one class in { Material, Method, OtherEntity, Task } causes an instance of  Material. It is designed based on the following predicates extracted by the NLP pipeline: cause,influence" ;
    rdfs:domain _:Nd209a2155624478ea7c6565c8ea0f04a ;
    rdfs:range cskg-ont:Material ;
    rdfs:subPropertyOf cskg-ont:causes ;
    owl:inverseOf cskg-ont:materialCausedBy .

cskg-ont:causesMethod a owl:ObjectProperty ;
    rdfs:comment "This relation indicates that an instance belonging to one class in { Method, Metric, OtherEntity, Task } causes an instance of  Method. It is designed based on the following predicates extracted by the NLP pipeline: cause,influence" ;
    rdfs:domain _:Nbc785b4cd6cb4bcfa9eaa81652c25a8f ;
    rdfs:range cskg-ont:Method ;
    rdfs:subPropertyOf cskg-ont:causes ;
    owl:inverseOf cskg-ont:methodCausedBy .

cskg-ont:causesMetric a owl:ObjectProperty ;
    rdfs:comment "This relation indicates that an instance belonging to one class in { Method, Metric, OtherEntity } causes an instance of  Metric. It is designed based on the following predicates extracted by the NLP pipeline: cause,influence" ;
    rdfs:domain _:Na5876f2af4d34f668446c417e896ca6f ;
    rdfs:range cskg-ont:Metric ;
    rdfs:subPropertyOf cskg-ont:causes ;
    owl:inverseOf cskg-ont:metricCausedBy .

cskg-ont:causesOtherEntity a owl:ObjectProperty ;
    rdfs:comment "This relation indicates that an instance belonging to one class in { Material, Method, Metric, OtherEntity, Task } causes an instance of  OtherEntity. It is designed based on the following predicates extracted by the NLP pipeline: cause,influence" ;
    rdfs:domain _:N834f5e422e534f37a004eeed1df1d02a ;
    rdfs:range cskg-ont:OtherEntity ;
    rdfs:subPropertyOf cskg-ont:causes ;
    owl:inverseOf cskg-ont:otherentityCausedBy .

cskg-ont:causesTask a owl:ObjectProperty ;
    rdfs:comment "This relation indicates that an instance belonging to one class in { Method, Metric, OtherEntity, Task } causes an instance of  Task. It is designed based on the following predicates extracted by the NLP pipeline: cause,influence" ;
    rdfs:domain _:N0e7780581a8a4d36a89b991aa4e88270 ;
    rdfs:range cskg-ont:Task ;
    rdfs:subPropertyOf cskg-ont:causes ;
    owl:inverseOf cskg-ont:taskCausedBy .

cskg-ont:classifiesMaterial a owl:ObjectProperty ;
    rdfs:comment "This relation indicates that an instance belonging to one class in { Method, Metric, OtherEntity, Task } classifies an instance of  Material. It is designed based on the following predicates extracted by the NLP pipeline: regroup,bracket,categorize,recode,chunk,code,separate,group,sort,sort_out,catalogue,classify,class,number,seed,reclassify,grade" ;
    rdfs:domain _:Ne6c5b294919942d0a05ec31ccf7d1e5f ;
    rdfs:range cskg-ont:Material ;
    rdfs:subPropertyOf cskg-ont:classifies ;
    owl:inverseOf cskg-ont:materialClassifiedBy .

cskg-ont:classifiesMethod a owl:ObjectProperty ;
    rdfs:comment "This relation indicates that an instance belonging to one class in { Method, Metric, OtherEntity, Task } classifies an instance of  Method. It is designed based on the following predicates extracted by the NLP pipeline: regroup,bracket,categorize,recode,chunk,code,separate,group,sort,sort_out,catalogue,classify,class,number,seed,reclassify,grade" ;
    rdfs:domain _:N96bcde7c4ac345708387678406877c6f ;
    rdfs:range cskg-ont:Method ;
    rdfs:subPropertyOf cskg-ont:classifies ;
    owl:inverseOf cskg-ont:methodClassifiedBy .

cskg-ont:classifiesMetric a owl:ObjectProperty ;
    rdfs:comment "This relation indicates that an instance belonging to one class in { Method, Metric, OtherEntity } classifies an instance of  Metric. It is designed based on the following predicates extracted by the NLP pipeline: regroup,bracket,categorize,recode,chunk,code,separate,group,sort,sort_out,catalogue,classify,class,number,seed,reclassify,grade" ;
    rdfs:domain _:N5454fd48e8d24c3ba6385a8dbd5c286e ;
    rdfs:range cskg-ont:Metric ;
    rdfs:subPropertyOf cskg-ont:classifies ;
    owl:inverseOf cskg-ont:metricClassifiedBy .

cskg-ont:classifiesOtherEntity a owl:ObjectProperty ;
    rdfs:comment "This relation indicates that an instance belonging to one class in { Method, Metric, OtherEntity } classifies an instance of  OtherEntity. It is designed based on the following predicates extracted by the NLP pipeline: regroup,bracket,categorize,recode,chunk,code,separate,group,sort,sort_out,catalogue,classify,class,number,seed,reclassify,grade" ;
    rdfs:domain _:N0b7d5a96f896460586a5c3412f211a2f ;
    rdfs:range cskg-ont:OtherEntity ;
    rdfs:subPropertyOf cskg-ont:classifies ;
    owl:inverseOf cskg-ont:otherentityClassifiedBy .

cskg-ont:classifiesTask a owl:ObjectProperty ;
    rdfs:comment "This relation indicates that an instance belonging to one class in { Method, Metric, OtherEntity, Task } classifies an instance of  Task. It is designed based on the following predicates extracted by the NLP pipeline: regroup,bracket,categorize,recode,chunk,code,separate,group,sort,sort_out,catalogue,classify,class,number,seed,reclassify,grade" ;
    rdfs:domain _:N2ef7f44fc61b4c279d0516a584ce1183 ;
    rdfs:range cskg-ont:Task ;
    rdfs:subPropertyOf cskg-ont:classifies ;
    owl:inverseOf cskg-ont:taskClassifiedBy .

cskg-ont:contributes-toMaterial a owl:ObjectProperty ;
    rdfs:comment "This relation indicates that an instance belonging to one class in { Method, OtherEntity, Task } contributes-to an instance of  Material. It is designed based on the following predicates extracted by the NLP pipeline: abnegate,gift,pass_out,turn-over,restore,turn-in,give-out,disburse,give-away,proffer,distribute,remit,transfer,extend,shell_out,give-up,hand_out,refer,disseminate,contribute" ;
    rdfs:domain _:N502287740d5e4306a36a494e175957e8 ;
    rdfs:range cskg-ont:Material ;
    rdfs:subPropertyOf cskg-ont:contributes-to ;
    owl:inverseOf cskg-ont:materialContributedBy .

cskg-ont:contributes-toMethod a owl:ObjectProperty ;
    rdfs:comment "This relation indicates that an instance belonging to one class in { Method, Metric, OtherEntity, Task } contributes-to an instance of  Method. It is designed based on the following predicates extracted by the NLP pipeline: abnegate,gift,pass_out,turn-over,restore,turn-in,give-out,disburse,give-away,proffer,distribute,remit,transfer,extend,shell_out,give-up,hand_out,refer,disseminate,contribute" ;
    rdfs:domain _:N0053e46091564bada9a0447722971667 ;
    rdfs:range cskg-ont:Method ;
    rdfs:subPropertyOf cskg-ont:contributes-to ;
    owl:inverseOf cskg-ont:methodContributedBy .

cskg-ont:contributes-toMetric a owl:ObjectProperty ;
    rdfs:comment "This relation indicates that an instance belonging to one class in { Method, Metric, OtherEntity, Task } contributes-to an instance of  Metric. It is designed based on the following predicates extracted by the NLP pipeline: abnegate,gift,pass_out,turn-over,restore,turn-in,give-out,disburse,give-away,proffer,distribute,remit,transfer,extend,shell_out,give-up,hand_out,refer,disseminate,contribute" ;
    rdfs:domain _:N689f07c9e0f04b3d90b900367988b31d ;
    rdfs:range cskg-ont:Metric ;
    rdfs:subPropertyOf cskg-ont:contributes-to ;
    owl:inverseOf cskg-ont:metricContributedBy .

cskg-ont:contributes-toOtherEntity a owl:ObjectProperty ;
    rdfs:comment "This relation indicates that an instance belonging to one class in { Method, Metric, OtherEntity, Task } contributes-to an instance of  OtherEntity. It is designed based on the following predicates extracted by the NLP pipeline: abnegate,gift,pass_out,turn-over,restore,turn-in,give-out,disburse,give-away,proffer,distribute,remit,transfer,extend,shell_out,give-up,hand_out,refer,disseminate,contribute" ;
    rdfs:domain _:N69404871f6734e52a230c04a387f8ba5 ;
    rdfs:range cskg-ont:OtherEntity ;
    rdfs:subPropertyOf cskg-ont:contributes-to ;
    owl:inverseOf cskg-ont:otherentityContributedBy .

cskg-ont:contributes-toTask a owl:ObjectProperty ;
    rdfs:comment "This relation indicates that an instance belonging to one class in { Method, OtherEntity, Task } contributes-to an instance of  Task. It is designed based on the following predicates extracted by the NLP pipeline: abnegate,gift,pass_out,turn-over,restore,turn-in,give-out,disburse,give-away,proffer,distribute,remit,transfer,extend,shell_out,give-up,hand_out,refer,disseminate,contribute" ;
    rdfs:domain _:N05212fdb40c2415597e72a670c36a9cb ;
    rdfs:range cskg-ont:Task ;
    rdfs:subPropertyOf cskg-ont:contributes-to ;
    owl:inverseOf cskg-ont:taskContributedBy .

cskg-ont:discussesMaterial a owl:ObjectProperty ;
    rdfs:comment "This relation indicates that an instance belonging to one class in { Task } discusses an instance of  Material. It is designed based on the following predicates extracted by the NLP pipeline: debate,discuss,chatter,confer,converse,argue,discus" ;
    rdfs:domain _:N6c31b3331102496698c40fe4ec35d364 ;
    rdfs:range cskg-ont:Material ;
    rdfs:subPropertyOf cskg-ont:discusses ;
    owl:inverseOf cskg-ont:materialDiscussedBy .

cskg-ont:discussesMethod a owl:ObjectProperty ;
    rdfs:comment "This relation indicates that an instance belonging to one class in { Method, Task } discusses an instance of  Method. It is designed based on the following predicates extracted by the NLP pipeline: debate,discuss,chatter,confer,converse,argue,discus" ;
    rdfs:domain _:Nc6e13c900be140a09f05f8a8026e8bd1 ;
    rdfs:range cskg-ont:Method ;
    rdfs:subPropertyOf cskg-ont:discusses ;
    owl:inverseOf cskg-ont:methodDiscussedBy .

cskg-ont:discussesMetric a owl:ObjectProperty ;
    rdfs:comment "This relation indicates that an instance belonging to one class in { Task } discusses an instance of  Metric. It is designed based on the following predicates extracted by the NLP pipeline: debate,discuss,chatter,confer,converse,argue,discus" ;
    rdfs:domain _:Nbdede62bcfd74bcd89207501aff28ae0 ;
    rdfs:range cskg-ont:Metric ;
    rdfs:subPropertyOf cskg-ont:discusses ;
    owl:inverseOf cskg-ont:metricDiscussedBy .

cskg-ont:discussesOtherEntity a owl:ObjectProperty ;
    rdfs:comment "This relation indicates that an instance belonging to one class in { Task } discusses an instance of  OtherEntity. It is designed based on the following predicates extracted by the NLP pipeline: debate,discuss,chatter,confer,converse,argue,discus" ;
    rdfs:domain _:N500da0682b05415fbc855afa0ad3b3de ;
    rdfs:range cskg-ont:OtherEntity ;
    rdfs:subPropertyOf cskg-ont:discusses ;
    owl:inverseOf cskg-ont:otherentityDiscussedBy .

cskg-ont:discussesTask a owl:ObjectProperty ;
    rdfs:comment "This relation indicates that an instance belonging to one class in { Task } discusses an instance of  Task. It is designed based on the following predicates extracted by the NLP pipeline: debate,discuss,chatter,confer,converse,argue,discus" ;
    rdfs:domain _:Na4e8e1ac70ae44409f0bd9176f121197 ;
    rdfs:range cskg-ont:Task ;
    rdfs:subPropertyOf cskg-ont:discusses ;
    owl:inverseOf cskg-ont:taskDiscussedBy .

cskg-ont:executesMaterial a owl:ObjectProperty,
        owl:TransitiveProperty ;
    rdfs:comment "This relation indicates that an instance belonging to one class in { Method, OtherEntity, Task } executes an instance of  Material. It is designed based on the following predicates extracted by the NLP pipeline: perform,execute,operate,run,simulate,play,work,train,action" ;
    rdfs:domain _:Nb5fb8f3ae4ef4e2093ed8d706e47a824 ;
    rdfs:range cskg-ont:Material ;
    rdfs:subPropertyOf cskg-ont:executes ;
    owl:inverseOf cskg-ont:materialExecutedBy .

cskg-ont:executesMethod a owl:ObjectProperty,
        owl:TransitiveProperty ;
    rdfs:comment "This relation indicates that an instance belonging to one class in { Method, Metric, OtherEntity, Task } executes an instance of  Method. It is designed based on the following predicates extracted by the NLP pipeline: perform,execute,operate,run,simulate,play,work,train,action" ;
    rdfs:domain _:N4aeafb7a405e4e7b91141051e25e7321 ;
    rdfs:range cskg-ont:Method ;
    rdfs:subPropertyOf cskg-ont:executes ;
    owl:inverseOf cskg-ont:methodExecutedBy .

cskg-ont:executesOtherEntity a owl:ObjectProperty,
        owl:TransitiveProperty ;
    rdfs:comment "This relation indicates that an instance belonging to one class in { Method, Metric, OtherEntity, Task } executes an instance of  OtherEntity. It is designed based on the following predicates extracted by the NLP pipeline: perform,execute,operate,run,simulate,play,work,train,action" ;
    rdfs:domain _:Ne749f6d04ff04b2cbee667ec125f6efb ;
    rdfs:range cskg-ont:OtherEntity ;
    rdfs:subPropertyOf cskg-ont:executes ;
    owl:inverseOf cskg-ont:otherentityExecutedBy .

cskg-ont:executesTask a owl:ObjectProperty,
        owl:TransitiveProperty ;
    rdfs:comment "This relation indicates that an instance belonging to one class in { Method, Task } executes an instance of  Task. It is designed based on the following predicates extracted by the NLP pipeline: perform,execute,operate,run,simulate,play,work,train,action" ;
    rdfs:domain _:Na8087c12038741179751d08d18e7e3bc ;
    rdfs:range cskg-ont:Task ;
    rdfs:subPropertyOf cskg-ont:executes ;
    owl:inverseOf cskg-ont:taskExecutedBy .

cskg-ont:extractsMaterial a owl:ObjectProperty,
        owl:TransitiveProperty ;
    rdfs:comment "This relation indicates that an instance belonging to one class in { Material, Method, OtherEntity, Task } extracts an instance of  Material. It is designed based on the following predicates extracted by the NLP pipeline: extract,mine,induce,infer" ;
    rdfs:domain _:N247eb93c5ce04deba8a07ed3bdad5221 ;
    rdfs:range cskg-ont:Material ;
    rdfs:subPropertyOf cskg-ont:extracts ;
    owl:inverseOf cskg-ont:materialExtractedBy .

cskg-ont:extractsMethod a owl:ObjectProperty,
        owl:TransitiveProperty ;
    rdfs:comment "This relation indicates that an instance belonging to one class in { Material, Method, OtherEntity, Task } extracts an instance of  Method. It is designed based on the following predicates extracted by the NLP pipeline: extract,mine,induce,infer" ;
    rdfs:domain _:Nbda0a556387e4fe5a06a56ee9bf2b863 ;
    rdfs:range cskg-ont:Method ;
    rdfs:subPropertyOf cskg-ont:extracts ;
    owl:inverseOf cskg-ont:methodExtractedBy .

cskg-ont:extractsMetric a owl:ObjectProperty,
        owl:TransitiveProperty ;
    rdfs:comment "This relation indicates that an instance belonging to one class in { Material, Method, OtherEntity, Task } extracts an instance of  Metric. It is designed based on the following predicates extracted by the NLP pipeline: extract,mine,induce,infer" ;
    rdfs:domain _:N3104c110b5ba4b969038f41603f6014c ;
    rdfs:range cskg-ont:Metric ;
    rdfs:subPropertyOf cskg-ont:extracts ;
    owl:inverseOf cskg-ont:metricExtractedBy .

cskg-ont:extractsOtherEntity a owl:ObjectProperty,
        owl:TransitiveProperty ;
    rdfs:comment "This relation indicates that an instance belonging to one class in { Material, Method, OtherEntity, Task } extracts an instance of  OtherEntity. It is designed based on the following predicates extracted by the NLP pipeline: extract,mine,induce,infer" ;
    rdfs:domain _:N9f08bcc4907946cfb720f28808183be3 ;
    rdfs:range cskg-ont:OtherEntity ;
    rdfs:subPropertyOf cskg-ont:extracts ;
    owl:inverseOf cskg-ont:otherentityExtractedBy .

cskg-ont:extractsTask a owl:ObjectProperty,
        owl:TransitiveProperty ;
    rdfs:comment "This relation indicates that an instance belonging to one class in { Material, Method, Task } extracts an instance of  Task. It is designed based on the following predicates extracted by the NLP pipeline: extract,mine,induce,infer" ;
    rdfs:domain _:N2cbdf4d21ad247858a139a0db3288bb9 ;
    rdfs:range cskg-ont:Task ;
    rdfs:subPropertyOf cskg-ont:extracts ;
    owl:inverseOf cskg-ont:taskExtractedBy .

cskg-ont:guidesMaterial a owl:ObjectProperty ;
    rdfs:comment "This relation indicates that an instance belonging to one class in { OtherEntity } guides an instance of  Material. It is designed based on the following predicates extracted by the NLP pipeline: steer,conduct,guide,misdirect,lead,escort,accompany,direct" ;
    rdfs:domain _:N70a6aff9428c4ea997f361b97a6d662c ;
    rdfs:range cskg-ont:Material ;
    rdfs:subPropertyOf cskg-ont:guides ;
    owl:inverseOf cskg-ont:materialGuidedBy .

cskg-ont:guidesMethod a owl:ObjectProperty ;
    rdfs:comment "This relation indicates that an instance belonging to one class in { Method, Metric, OtherEntity, Task } guides an instance of  Method. It is designed based on the following predicates extracted by the NLP pipeline: steer,conduct,guide,misdirect,lead,escort,accompany,direct" ;
    rdfs:domain _:N51d8015b10504c6db235279c00bf373e ;
    rdfs:range cskg-ont:Method ;
    rdfs:subPropertyOf cskg-ont:guides ;
    owl:inverseOf cskg-ont:methodGuidedBy .

cskg-ont:guidesMetric a owl:ObjectProperty ;
    rdfs:comment "This relation indicates that an instance belonging to one class in { Method, Metric, OtherEntity, Task } guides an instance of  Metric. It is designed based on the following predicates extracted by the NLP pipeline: steer,conduct,guide,misdirect,lead,escort,accompany,direct" ;
    rdfs:domain _:Na18faff524ce44c3a7bd793776599add ;
    rdfs:range cskg-ont:Metric ;
    rdfs:subPropertyOf cskg-ont:guides ;
    owl:inverseOf cskg-ont:metricGuidedBy .

cskg-ont:guidesOtherEntity a owl:ObjectProperty ;
    rdfs:comment "This relation indicates that an instance belonging to one class in { Method, Metric, OtherEntity, Task } guides an instance of  OtherEntity. It is designed based on the following predicates extracted by the NLP pipeline: steer,conduct,guide,misdirect,lead,escort,accompany,direct" ;
    rdfs:domain _:Naa71c951c7094ee78260e723b1581218 ;
    rdfs:range cskg-ont:OtherEntity ;
    rdfs:subPropertyOf cskg-ont:guides ;
    owl:inverseOf cskg-ont:otherentityGuidedBy .

cskg-ont:guidesTask a owl:ObjectProperty ;
    rdfs:comment "This relation indicates that an instance belonging to one class in { Method, OtherEntity, Task } guides an instance of  Task. It is designed based on the following predicates extracted by the NLP pipeline: steer,conduct,guide,misdirect,lead,escort,accompany,direct" ;
    rdfs:domain _:N5ae634f65eac4fedb488fffb891db558 ;
    rdfs:range cskg-ont:Task ;
    rdfs:subPropertyOf cskg-ont:guides ;
    owl:inverseOf cskg-ont:taskGuidedBy .

cskg-ont:highlightsMaterial a owl:ObjectProperty ;
    rdfs:comment "This relation indicates that an instance belonging to one class in { Material, Method, Metric, OtherEntity, Task } highlights an instance of  Material. It is designed based on the following predicates extracted by the NLP pipeline: highlight,emphasize" ;
    rdfs:domain _:N08286035189c4c1d815e149a72050a9d ;
    rdfs:range cskg-ont:Material ;
    rdfs:subPropertyOf cskg-ont:highlights ;
    owl:inverseOf cskg-ont:materialHighlightedBy .

cskg-ont:highlightsMethod a owl:ObjectProperty ;
    rdfs:comment "This relation indicates that an instance belonging to one class in { Material, Method, Metric, OtherEntity, Task } highlights an instance of  Method. It is designed based on the following predicates extracted by the NLP pipeline: highlight,emphasize" ;
    rdfs:domain _:N47b3eb8ba4ff46eeae0ebc5471a01be0 ;
    rdfs:range cskg-ont:Method ;
    rdfs:subPropertyOf cskg-ont:highlights ;
    owl:inverseOf cskg-ont:methodHighlightedBy .

cskg-ont:highlightsMetric a owl:ObjectProperty ;
    rdfs:comment "This relation indicates that an instance belonging to one class in { Material, Method, Metric, OtherEntity, Task } highlights an instance of  Metric. It is designed based on the following predicates extracted by the NLP pipeline: highlight,emphasize" ;
    rdfs:domain _:N7d3fce177c8d4cb5af61d158778e6aee ;
    rdfs:range cskg-ont:Metric ;
    rdfs:subPropertyOf cskg-ont:highlights ;
    owl:inverseOf cskg-ont:metricHighlightedBy .

cskg-ont:highlightsOtherEntity a owl:ObjectProperty ;
    rdfs:comment "This relation indicates that an instance belonging to one class in { Material, Method, Metric, OtherEntity, Task } highlights an instance of  OtherEntity. It is designed based on the following predicates extracted by the NLP pipeline: highlight,emphasize" ;
    rdfs:domain _:N546ebba2acea45c98854bbcd3e5e186c ;
    rdfs:range cskg-ont:OtherEntity ;
    rdfs:subPropertyOf cskg-ont:highlights ;
    owl:inverseOf cskg-ont:otherentityHighlightedBy .

cskg-ont:highlightsTask a owl:ObjectProperty ;
    rdfs:comment "This relation indicates that an instance belonging to one class in { Material, Method, OtherEntity, Task } highlights an instance of  Task. It is designed based on the following predicates extracted by the NLP pipeline: highlight,emphasize" ;
    rdfs:domain _:Nd3ca8cbb75dc405ca9d7fef969d2dc40 ;
    rdfs:range cskg-ont:Task ;
    rdfs:subPropertyOf cskg-ont:highlights ;
    owl:inverseOf cskg-ont:taskHighlightedBy .

cskg-ont:identifiesMaterial a owl:ObjectProperty ;
    rdfs:comment "This relation indicates that an instance belonging to one class in { Method, OtherEntity, Task } identifies an instance of  Material. It is designed based on the following predicates extracted by the NLP pipeline: identify,detect,filter,recognize,locate" ;
    rdfs:domain _:Nb30f3123fa034f52bf3b37967b773741 ;
    rdfs:range cskg-ont:Material ;
    rdfs:subPropertyOf cskg-ont:identifies ;
    owl:inverseOf cskg-ont:materialIdentifiedBy .

cskg-ont:identifiesMethod a owl:ObjectProperty ;
    rdfs:comment "This relation indicates that an instance belonging to one class in { Method, OtherEntity, Task } identifies an instance of  Method. It is designed based on the following predicates extracted by the NLP pipeline: identify,detect,filter,recognize,locate" ;
    rdfs:domain _:N2824d69514f949f49091964a1b85a3a6 ;
    rdfs:range cskg-ont:Method ;
    rdfs:subPropertyOf cskg-ont:identifies ;
    owl:inverseOf cskg-ont:methodIdentifiedBy .

cskg-ont:identifiesMetric a owl:ObjectProperty ;
    rdfs:comment "This relation indicates that an instance belonging to one class in { Method, OtherEntity, Task } identifies an instance of  Metric. It is designed based on the following predicates extracted by the NLP pipeline: identify,detect,filter,recognize,locate" ;
    rdfs:domain _:N14089d541ce349aaaa4fd1b63fd36a00 ;
    rdfs:range cskg-ont:Metric ;
    rdfs:subPropertyOf cskg-ont:identifies ;
    owl:inverseOf cskg-ont:metricIdentifiedBy .

cskg-ont:identifiesOtherEntity a owl:ObjectProperty ;
    rdfs:comment "This relation indicates that an instance belonging to one class in { Method, OtherEntity, Task } identifies an instance of  OtherEntity. It is designed based on the following predicates extracted by the NLP pipeline: identify,detect,filter,recognize,locate" ;
    rdfs:domain _:N32d7ae61b2634b3fa1855613b102b731 ;
    rdfs:range cskg-ont:OtherEntity ;
    rdfs:subPropertyOf cskg-ont:identifies ;
    owl:inverseOf cskg-ont:otherentityIdentifiedBy .

cskg-ont:identifiesTask a owl:ObjectProperty ;
    rdfs:comment "This relation indicates that an instance belonging to one class in { Method, OtherEntity, Task } identifies an instance of  Task. It is designed based on the following predicates extracted by the NLP pipeline: identify,detect,filter,recognize,locate" ;
    rdfs:domain _:N6fc28ae3bc614aa5a75fd033d634fbf2 ;
    rdfs:range cskg-ont:Task ;
    rdfs:subPropertyOf cskg-ont:identifies ;
    owl:inverseOf cskg-ont:taskIdentifiedBy .

cskg-ont:improvesMaterial a owl:ObjectProperty ;
    rdfs:comment "This relation indicates that an instance belonging to one class in { Method, Metric, OtherEntity, Task } improves an instance of  Material. It is designed based on the following predicates extracted by the NLP pipeline: improve,evolve,grow,enrich,expand,augment,raise,enhance,advance,gain,optimize" ;
    rdfs:domain _:N153e4415eed74d11915734588e6374d6 ;
    rdfs:range cskg-ont:Material ;
    rdfs:subPropertyOf cskg-ont:improves ;
    owl:inverseOf cskg-ont:materialImprovedBy .

cskg-ont:improvesMethod a owl:ObjectProperty ;
    rdfs:comment "This relation indicates that an instance belonging to one class in { Material, Method, Metric, OtherEntity, Task } improves an instance of  Method. It is designed based on the following predicates extracted by the NLP pipeline: improve,evolve,grow,enrich,expand,augment,raise,enhance,advance,gain,optimize" ;
    rdfs:domain _:Nf64606f7c1a94762924496d321d021f3 ;
    rdfs:range cskg-ont:Method ;
    rdfs:subPropertyOf cskg-ont:improves ;
    owl:inverseOf cskg-ont:methodImprovedBy .

cskg-ont:improvesMetric a owl:ObjectProperty ;
    rdfs:comment "This relation indicates that an instance belonging to one class in { Method, Metric, OtherEntity, Task } improves an instance of  Metric. It is designed based on the following predicates extracted by the NLP pipeline: improve,evolve,grow,enrich,expand,augment,raise,enhance,advance,gain,optimize" ;
    rdfs:domain _:Na29cd5ad9ddc439d8d35a10b6625d264 ;
    rdfs:range cskg-ont:Metric ;
    rdfs:subPropertyOf cskg-ont:improves ;
    owl:inverseOf cskg-ont:metricImprovedBy .

cskg-ont:improvesOtherEntity a owl:ObjectProperty ;
    rdfs:comment "This relation indicates that an instance belonging to one class in { Method, Metric, OtherEntity, Task } improves an instance of  OtherEntity. It is designed based on the following predicates extracted by the NLP pipeline: improve,evolve,grow,enrich,expand,augment,raise,enhance,advance,gain,optimize" ;
    rdfs:domain _:N5b30fa28b8f649bc95dba7dbc8229030 ;
    rdfs:range cskg-ont:OtherEntity ;
    rdfs:subPropertyOf cskg-ont:improves ;
    owl:inverseOf cskg-ont:otherentityImprovedBy .

cskg-ont:improvesTask a owl:ObjectProperty ;
    rdfs:comment "This relation indicates that an instance belonging to one class in { Material, Method, Metric, Task } improves an instance of  Task. It is designed based on the following predicates extracted by the NLP pipeline: improve,evolve,grow,enrich,expand,augment,raise,enhance,advance,gain,optimize" ;
    rdfs:domain _:Nc386a051f3e9404782512bb5046e9df6 ;
    rdfs:range cskg-ont:Task ;
    rdfs:subPropertyOf cskg-ont:improves ;
    owl:inverseOf cskg-ont:taskImprovedBy .

cskg-ont:includesMaterial a owl:ObjectProperty,
        owl:TransitiveProperty ;
    rdfs:comment "This relation indicates that an instance belonging to one class in { Material, Method, OtherEntity, Task } includes an instance of  Material. It is designed by the Feature-of and Part-of relationships extracted by the DyGIE++. It is also designed based on the following predicates extracted by the NLP pipeline: 'relate,include,involve,engage,enroll,embed,contain,comprise,carry,cover,consider,share,mount,have,equip,install" ;
    rdfs:domain _:Nf9a039f5b7e649a9afbe2d6d8659f9fb ;
    rdfs:range cskg-ont:Material ;
    rdfs:subPropertyOf cskg-ont:includes ;
    owl:inverseOf cskg-ont:materialIncludedBy .

cskg-ont:includesMethod a owl:ObjectProperty,
        owl:TransitiveProperty ;
    rdfs:comment "This relation indicates that an instance belonging to one class in { Method, OtherEntity, Task } includes an instance of  Method. It is designed by the Feature-of and Part-of relationships extracted by the DyGIE++. It is also designed based on the following predicates extracted by the NLP pipeline: 'relate,include,involve,engage,enroll,embed,contain,comprise,carry,cover,consider,share,mount,have,equip,install" ;
    rdfs:domain _:Nf653e74b64c64b5fb48fb838f3e9088c ;
    rdfs:range cskg-ont:Method ;
    rdfs:subPropertyOf cskg-ont:includes ;
    owl:inverseOf cskg-ont:methodIncludedBy .

cskg-ont:includesMetric a owl:ObjectProperty ;
    rdfs:comment "This relation indicates that an instance belonging to one class in { Material, Method, OtherEntity, Task } includes an instance of  Metric. It is designed by the Feature-of and Part-of relationships extracted by the DyGIE++. It is also designed based on the following predicates extracted by the NLP pipeline: 'relate,include,involve,engage,enroll,embed,contain,comprise,carry,cover,consider,share,mount,have,equip,install" ;
    rdfs:domain _:N1b7fcb3709b14ff3b9f3959d221e3dca ;
    rdfs:range cskg-ont:Metric ;
    rdfs:subPropertyOf cskg-ont:includes ;
    owl:inverseOf cskg-ont:metricIncludedBy .

cskg-ont:includesOtherEntity a owl:ObjectProperty,
        owl:TransitiveProperty ;
    rdfs:comment "This relation indicates that an instance belonging to one class in { Material, Method, OtherEntity, Task } includes an instance of  OtherEntity. It is designed by the Feature-of and Part-of relationships extracted by the DyGIE++. It is also designed based on the following predicates extracted by the NLP pipeline: 'relate,include,involve,engage,enroll,embed,contain,comprise,carry,cover,consider,share,mount,have,equip,install" ;
    rdfs:domain _:N9c7a820d81f24625baa100d6ee6bbd5e ;
    rdfs:range cskg-ont:OtherEntity ;
    rdfs:subPropertyOf cskg-ont:includes ;
    owl:inverseOf cskg-ont:otherentityIncludedBy .

cskg-ont:includesTask a owl:ObjectProperty,
        owl:TransitiveProperty ;
    rdfs:comment "This relation indicates that an instance belonging to one class in { Method, Task } includes an instance of  Task. It is designed by the Feature-of and Part-of relationships extracted by the DyGIE++. It is also designed based on the following predicates extracted by the NLP pipeline: 'relate,include,involve,engage,enroll,embed,contain,comprise,carry,cover,consider,share,mount,have,equip,install" ;
    rdfs:domain _:Nfe8a492d8bc446d6badfb8ef747c73f5 ;
    rdfs:range cskg-ont:Task ;
    rdfs:subPropertyOf cskg-ont:includes ;
    owl:inverseOf cskg-ont:taskIncludedBy .

cskg-ont:interacts-withMaterial a owl:ObjectProperty ;
    rdfs:comment "This relation indicates that an instance belonging to one class in { Material, Method, Metric, OtherEntity, Task } interacts-with an instance of  Material. It is designed based on the following predicates extracted by the NLP pipeline: renegotiate,compromise,agree,debate,interact,collaborate,disagree,communicate,haggle,interlink,participate" ;
    rdfs:domain _:N9022ec3d1df544c39293f06d4a2915b4 ;
    rdfs:range cskg-ont:Material ;
    rdfs:subPropertyOf cskg-ont:interacts-with ;
    owl:inverseOf cskg-ont:materialInteracts-With .

cskg-ont:interacts-withMethod a owl:ObjectProperty ;
    rdfs:comment "This relation indicates that an instance belonging to one class in { Material, Method, Metric, OtherEntity, Task } interacts-with an instance of  Method. It is designed based on the following predicates extracted by the NLP pipeline: renegotiate,compromise,agree,debate,interact,collaborate,disagree,communicate,haggle,interlink,participate" ;
    rdfs:domain _:N30ac83d4034e493dbbf4dced9bfc0300 ;
    rdfs:range cskg-ont:Method ;
    rdfs:subPropertyOf cskg-ont:interacts-with ;
    owl:inverseOf cskg-ont:methodInteracts-With .

cskg-ont:interacts-withMetric a owl:ObjectProperty ;
    rdfs:comment "This relation indicates that an instance belonging to one class in { Material, Method, Metric, OtherEntity, Task } interacts-with an instance of  Metric. It is designed based on the following predicates extracted by the NLP pipeline: renegotiate,compromise,agree,debate,interact,collaborate,disagree,communicate,haggle,interlink,participate" ;
    rdfs:domain _:N4f8cc36c01214c6ba562824bbde43bd2 ;
    rdfs:range cskg-ont:Metric ;
    rdfs:subPropertyOf cskg-ont:interacts-with ;
    owl:inverseOf cskg-ont:metricInteracts-With .

cskg-ont:interacts-withOtherEntity a owl:ObjectProperty ;
    rdfs:comment "This relation indicates that an instance belonging to one class in { Material, Method, Metric, OtherEntity, Task } interacts-with an instance of  OtherEntity. It is designed based on the following predicates extracted by the NLP pipeline: renegotiate,compromise,agree,debate,interact,collaborate,disagree,communicate,haggle,interlink,participate" ;
    rdfs:domain _:N0c6045d04e2d4fb698e46d314ee9ca52 ;
    rdfs:range cskg-ont:OtherEntity ;
    rdfs:subPropertyOf cskg-ont:interacts-with ;
    owl:inverseOf cskg-ont:otherentityInteracts-With .

cskg-ont:interacts-withTask a owl:ObjectProperty ;
    rdfs:comment "This relation indicates that an instance belonging to one class in { Material, Method, Metric, OtherEntity, Task } interacts-with an instance of  Task. It is designed based on the following predicates extracted by the NLP pipeline: renegotiate,compromise,agree,debate,interact,collaborate,disagree,communicate,haggle,interlink,participate" ;
    rdfs:domain _:N60a43915fb6c4bd483370f770935a5b9 ;
    rdfs:range cskg-ont:Task ;
    rdfs:subPropertyOf cskg-ont:interacts-with ;
    owl:inverseOf cskg-ont:taskInteracts-With .

cskg-ont:lacksMaterial a owl:ObjectProperty ;
    rdfs:comment "This relation indicates that an instance belonging to one class in { Material, Method, Metric, OtherEntity, Task } lacks an instance of  Material. It is designed based on the following predicates extracted by the NLP pipeline: lack" ;
    rdfs:domain _:N842e98b9e8e240b8b24fc5a53f53effa ;
    rdfs:range cskg-ont:Material ;
    rdfs:subPropertyOf cskg-ont:lacks ;
    owl:inverseOf cskg-ont:materialLackedof .

cskg-ont:lacksMethod a owl:ObjectProperty ;
    rdfs:comment "This relation indicates that an instance belonging to one class in { Material, Method, Metric, OtherEntity, Task } lacks an instance of  Method. It is designed based on the following predicates extracted by the NLP pipeline: lack" ;
    rdfs:domain _:N8fe46fa8ab734ea18a302a274498734c ;
    rdfs:range cskg-ont:Method ;
    rdfs:subPropertyOf cskg-ont:lacks ;
    owl:inverseOf cskg-ont:methodLackedof .

cskg-ont:lacksMetric a owl:ObjectProperty ;
    rdfs:comment "This relation indicates that an instance belonging to one class in { Material, Method, OtherEntity, Task } lacks an instance of  Metric. It is designed based on the following predicates extracted by the NLP pipeline: lack" ;
    rdfs:domain _:N4d1a78f54cdb41009c4456a977760171 ;
    rdfs:range cskg-ont:Metric ;
    rdfs:subPropertyOf cskg-ont:lacks ;
    owl:inverseOf cskg-ont:metricLackedof .

cskg-ont:lacksOtherEntity a owl:ObjectProperty ;
    rdfs:comment "This relation indicates that an instance belonging to one class in { Material, Method, Metric, OtherEntity, Task } lacks an instance of  OtherEntity. It is designed based on the following predicates extracted by the NLP pipeline: lack" ;
    rdfs:domain _:N5c7e8edce3d54f2e84a531e2b82c0fb4 ;
    rdfs:range cskg-ont:OtherEntity ;
    rdfs:subPropertyOf cskg-ont:lacks ;
    owl:inverseOf cskg-ont:otherentityLackedof .

cskg-ont:lacksTask a owl:ObjectProperty ;
    rdfs:comment "This relation indicates that an instance belonging to one class in { Material, Method, Task } lacks an instance of  Task. It is designed based on the following predicates extracted by the NLP pipeline: lack" ;
    rdfs:domain _:N1199cb3160fd4657961cd60acea9c881 ;
    rdfs:range cskg-ont:Task ;
    rdfs:subPropertyOf cskg-ont:lacks ;
    owl:inverseOf cskg-ont:taskLackedof .

cskg-ont:learnsMaterial a owl:ObjectProperty ;
    rdfs:comment "This relation indicates that an instance belonging to one class in { Material, Method, OtherEntity, Task } learns an instance of  Material. It is designed based on the following predicates extracted by the NLP pipeline: memorize,glean,learn,study,absorb,assimilate,cram,relearn,read" ;
    rdfs:domain _:N64948af7aad5415789b62c973ad807e4 ;
    rdfs:range cskg-ont:Material ;
    rdfs:subPropertyOf cskg-ont:learns ;
    owl:inverseOf cskg-ont:materialLearnedBy .

cskg-ont:learnsMethod a owl:ObjectProperty ;
    rdfs:comment "This relation indicates that an instance belonging to one class in { Material, Method, OtherEntity, Task } learns an instance of  Method. It is designed based on the following predicates extracted by the NLP pipeline: memorize,glean,learn,study,absorb,assimilate,cram,relearn,read" ;
    rdfs:domain _:Nbcdeafe6bedf4949bb33dd323b560164 ;
    rdfs:range cskg-ont:Method ;
    rdfs:subPropertyOf cskg-ont:learns ;
    owl:inverseOf cskg-ont:methodLearnedBy .

cskg-ont:learnsOtherEntity a owl:ObjectProperty ;
    rdfs:comment "This relation indicates that an instance belonging to one class in { Material, Method, OtherEntity, Task } learns an instance of  OtherEntity. It is designed based on the following predicates extracted by the NLP pipeline: memorize,glean,learn,study,absorb,assimilate,cram,relearn,read" ;
    rdfs:domain _:N266241773fb747198e8cee8f7c80f0ce ;
    rdfs:range cskg-ont:OtherEntity ;
    rdfs:subPropertyOf cskg-ont:learns ;
    owl:inverseOf cskg-ont:otherentityLearnedBy .

cskg-ont:learnsTask a owl:ObjectProperty ;
    rdfs:comment "This relation indicates that an instance belonging to one class in { Material, Method, OtherEntity, Task } learns an instance of  Task. It is designed based on the following predicates extracted by the NLP pipeline: memorize,glean,learn,study,absorb,assimilate,cram,relearn,read" ;
    rdfs:domain _:N9ee201229f954e9cb0c1d007f3277890 ;
    rdfs:range cskg-ont:Task ;
    rdfs:subPropertyOf cskg-ont:learns ;
    owl:inverseOf cskg-ont:taskLearnedBy .

cskg-ont:limitsMaterial a owl:ObjectProperty ;
    rdfs:comment "This relation indicates that an instance belonging to one class in { Material, Method, OtherEntity, Task } limits an instance of  Material. It is designed based on the following predicates extracted by the NLP pipeline: reduce,limit,confine,restrain,constrain,restrict,prevent" ;
    rdfs:domain _:N6fbd7b79b82641238ccb201b4c0fc275 ;
    rdfs:range cskg-ont:Material ;
    rdfs:subPropertyOf cskg-ont:limits ;
    owl:inverseOf cskg-ont:materialLimitedBy .

cskg-ont:limitsMethod a owl:ObjectProperty ;
    rdfs:comment "This relation indicates that an instance belonging to one class in { Material, Method, OtherEntity, Task } limits an instance of  Method. It is designed based on the following predicates extracted by the NLP pipeline: reduce,limit,confine,restrain,constrain,restrict,prevent" ;
    rdfs:domain _:Nc935650e9b464fcc9855696059362122 ;
    rdfs:range cskg-ont:Method ;
    rdfs:subPropertyOf cskg-ont:limits ;
    owl:inverseOf cskg-ont:methodLimitedBy .

cskg-ont:limitsMetric a owl:ObjectProperty ;
    rdfs:comment "This relation indicates that an instance belonging to one class in { Material, Method, Metric, OtherEntity } limits an instance of  Metric. It is designed based on the following predicates extracted by the NLP pipeline: reduce,limit,confine,restrain,constrain,restrict,prevent" ;
    rdfs:domain _:N3002f74f0b844bec8d66e889c133c828 ;
    rdfs:range cskg-ont:Metric ;
    rdfs:subPropertyOf cskg-ont:limits ;
    owl:inverseOf cskg-ont:metricLimitedBy .

cskg-ont:limitsOtherEntity a owl:ObjectProperty ;
    rdfs:comment "This relation indicates that an instance belonging to one class in { Material, Method, Metric, OtherEntity, Task } limits an instance of  OtherEntity. It is designed based on the following predicates extracted by the NLP pipeline: reduce,limit,confine,restrain,constrain,restrict,prevent" ;
    rdfs:domain _:N041d55ebb2344a4c821fed0b93a96c07 ;
    rdfs:range cskg-ont:OtherEntity ;
    rdfs:subPropertyOf cskg-ont:limits ;
    owl:inverseOf cskg-ont:otherentityLimitedBy .

cskg-ont:limitsTask a owl:ObjectProperty ;
    rdfs:comment "This relation indicates that an instance belonging to one class in { Material, Method, Metric, OtherEntity, Task } limits an instance of  Task. It is designed based on the following predicates extracted by the NLP pipeline: reduce,limit,confine,restrain,constrain,restrict,prevent" ;
    rdfs:domain _:N1b0212194ffc4a3eae84da8bbd9c1a17 ;
    rdfs:range cskg-ont:Task ;
    rdfs:subPropertyOf cskg-ont:limits ;
    owl:inverseOf cskg-ont:taskLimitedBy .

cskg-ont:linksMaterial a owl:ObjectProperty ;
    rdfs:comment "This relation indicates that an instance belonging to one class in { Method, Metric, Task } links an instance of  Material. It is designed based on the following predicates extracted by the NLP pipeline: fasten,strap,hook,lasso,leash,reeve,peg,rope,seal,clamp,latch,chain,band,trammel,shackle,clasp,knot,button,lock,moor,buckle,yoke,manacle,screw,link,string,pin,tether,paste,anchor,bond,wire,connect" ;
    rdfs:domain _:Nc5e1db55c2f049efb0984d63efb8a66e ;
    rdfs:range cskg-ont:Material ;
    rdfs:subPropertyOf cskg-ont:links ;
    owl:inverseOf cskg-ont:materialLinkedBy .

cskg-ont:linksMethod a owl:ObjectProperty,
        owl:TransitiveProperty ;
    rdfs:comment "This relation indicates that an instance belonging to one class in { Method, OtherEntity, Task } links an instance of  Method. It is designed based on the following predicates extracted by the NLP pipeline: fasten,strap,hook,lasso,leash,reeve,peg,rope,seal,clamp,latch,chain,band,trammel,shackle,clasp,knot,button,lock,moor,buckle,yoke,manacle,screw,link,string,pin,tether,paste,anchor,bond,wire,connect" ;
    rdfs:domain _:N33b475fad8e94666ab0c0d8f6bb77516 ;
    rdfs:range cskg-ont:Method ;
    rdfs:subPropertyOf cskg-ont:links ;
    owl:inverseOf cskg-ont:methodLinkedBy .

cskg-ont:linksOtherEntity a owl:ObjectProperty,
        owl:TransitiveProperty ;
    rdfs:comment "This relation indicates that an instance belonging to one class in { Method, OtherEntity, Task } links an instance of  OtherEntity. It is designed based on the following predicates extracted by the NLP pipeline: fasten,strap,hook,lasso,leash,reeve,peg,rope,seal,clamp,latch,chain,band,trammel,shackle,clasp,knot,button,lock,moor,buckle,yoke,manacle,screw,link,string,pin,tether,paste,anchor,bond,wire,connect" ;
    rdfs:domain _:Naca3ac89fa7b4a57ae86bcc28519a296 ;
    rdfs:range cskg-ont:OtherEntity ;
    rdfs:subPropertyOf cskg-ont:links ;
    owl:inverseOf cskg-ont:otherentityLinkedBy .

cskg-ont:linksTask a owl:ObjectProperty,
        owl:TransitiveProperty ;
    rdfs:comment "This relation indicates that an instance belonging to one class in { Method, OtherEntity, Task } links an instance of  Task. It is designed based on the following predicates extracted by the NLP pipeline: fasten,strap,hook,lasso,leash,reeve,peg,rope,seal,clamp,latch,chain,band,trammel,shackle,clasp,knot,button,lock,moor,buckle,yoke,manacle,screw,link,string,pin,tether,paste,anchor,bond,wire,connect" ;
    rdfs:domain _:N20e3c93bde28431db37c1313ed671e6e ;
    rdfs:range cskg-ont:Task ;
    rdfs:subPropertyOf cskg-ont:links ;
    owl:inverseOf cskg-ont:taskLinkedBy .

cskg-ont:managesMaterial a owl:ObjectProperty ;
    rdfs:comment "This relation indicates that an instance belonging to one class in { Method, Task } manages an instance of  Material. It is designed based on the following predicates extracted by the NLP pipeline: look_out,wait_on,look_after,care,manage,maintain,preserve,keep,handle,treat,deal,configure" ;
    rdfs:domain _:N8a58b70d2de6491b9e2460616c6f8e88 ;
    rdfs:range cskg-ont:Material ;
    rdfs:subPropertyOf cskg-ont:manages ;
    owl:inverseOf cskg-ont:materialManagedBy .

cskg-ont:managesMethod a owl:ObjectProperty,
        owl:TransitiveProperty ;
    rdfs:comment "This relation indicates that an instance belonging to one class in { Method, Task } manages an instance of  Method. It is designed based on the following predicates extracted by the NLP pipeline: look_out,wait_on,look_after,care,manage,maintain,preserve,keep,handle,treat,deal,configure" ;
    rdfs:domain _:Nebf399080e1a4380a2c8f1c7401f0c10 ;
    rdfs:range cskg-ont:Method ;
    rdfs:subPropertyOf cskg-ont:manages ;
    owl:inverseOf cskg-ont:methodManagedBy .

cskg-ont:managesMetric a owl:ObjectProperty ;
    rdfs:comment "This relation indicates that an instance belonging to one class in { Method, Task } manages an instance of  Metric. It is designed based on the following predicates extracted by the NLP pipeline: look_out,wait_on,look_after,care,manage,maintain,preserve,keep,handle,treat,deal,configure" ;
    rdfs:domain _:Nf70066e61f4d46c1993c8d54a7fc726c ;
    rdfs:range cskg-ont:Metric ;
    rdfs:subPropertyOf cskg-ont:manages ;
    owl:inverseOf cskg-ont:metricManagedBy .

cskg-ont:managesOtherEntity a owl:ObjectProperty,
        owl:TransitiveProperty ;
    rdfs:comment "This relation indicates that an instance belonging to one class in { Method, Task } manages an instance of  OtherEntity. It is designed based on the following predicates extracted by the NLP pipeline: look_out,wait_on,look_after,care,manage,maintain,preserve,keep,handle,treat,deal,configure" ;
    rdfs:domain _:N3c0397721de747b089088a59bba638b3 ;
    rdfs:range cskg-ont:OtherEntity ;
    rdfs:subPropertyOf cskg-ont:manages ;
    owl:inverseOf cskg-ont:otherentityManagedBy .

cskg-ont:managesTask a owl:ObjectProperty,
        owl:TransitiveProperty ;
    rdfs:comment "This relation indicates that an instance belonging to one class in { Method, Task } manages an instance of  Task. It is designed based on the following predicates extracted by the NLP pipeline: look_out,wait_on,look_after,care,manage,maintain,preserve,keep,handle,treat,deal,configure" ;
    rdfs:domain _:N618060df18e6473e9d6a6ba16882c462 ;
    rdfs:range cskg-ont:Task ;
    rdfs:subPropertyOf cskg-ont:manages ;
    owl:inverseOf cskg-ont:taskManagedBy .

cskg-ont:matchesMethod a owl:ObjectProperty ;
    rdfs:comment "This relation indicates that an instance belonging to one class in { Method, Task } matches an instance of  Method. It is designed based on the following predicates extracted by the NLP pipeline: harmonize,go,square,dovetail,couple,pair,alternate,align,map,compare,match" ;
    rdfs:domain _:N40a65d8582d6409cae8d3048379836d9 ;
    rdfs:range cskg-ont:Method ;
    rdfs:subPropertyOf cskg-ont:matches ;
    owl:inverseOf cskg-ont:methodMatchedBy .

cskg-ont:matchesMetric a owl:ObjectProperty ;
    rdfs:comment "This relation indicates that an instance belonging to one class in { Method } matches an instance of  Metric. It is designed based on the following predicates extracted by the NLP pipeline: harmonize,go,square,dovetail,couple,pair,alternate,align,map,compare,match" ;
    rdfs:domain _:N3e79eb16e49543fe827090de5929a49d ;
    rdfs:range cskg-ont:Metric ;
    rdfs:subPropertyOf cskg-ont:matches ;
    owl:inverseOf cskg-ont:metricMatchedBy .

cskg-ont:matchesTask a owl:ObjectProperty ;
    rdfs:comment "This relation indicates that an instance belonging to one class in { Method, Task } matches an instance of  Task. It is designed based on the following predicates extracted by the NLP pipeline: harmonize,go,square,dovetail,couple,pair,alternate,align,map,compare,match" ;
    rdfs:domain _:Nf29389327a4f4441a7638e9b87845ca2 ;
    rdfs:range cskg-ont:Task ;
    rdfs:subPropertyOf cskg-ont:matches ;
    owl:inverseOf cskg-ont:taskMatchedBy .

cskg-ont:materialAcquiredBy a owl:ObjectProperty ;
    rdfs:comment "This relation indicates that an instance	 of class Material was acquired by an instance belonging to one of the following classes { Method, OtherEntity, Task }. It is designed based on the following predicates extracted by the NLP pipeline: select,accumulate,recoup,source,receive,acquire,regain,retrieve,obtain,accrue,borrow,subselect,inherit,accept,collect,gather,store,attract,get,capture,record,achieve" ;
    rdfs:domain cskg-ont:Material ;
    rdfs:range _:N1f3d128b6fda402dbc1b86103dfda554 ;
    rdfs:subPropertyOf cskg-ont:acquiredBy ;
    owl:inverseOf cskg-ont:acquiresMaterial .

cskg-ont:materialAdaptedBy a owl:ObjectProperty ;
    rdfs:comment "This relation indicates that an instance	 of class Material was adapted by an instance belonging to one of the following classes { Method, OtherEntity, Task }. It is designed based on the following predicates extracted by the NLP pipeline: readapt,adjust,conform,adapt,gear,readjust,fit,assimilate,accommodate,personalize,customize,specialize,generalize,tailor,refine" ;
    rdfs:domain cskg-ont:Material ;
    rdfs:range _:N8653196663b34e288e5950f343e490a8 ;
    rdfs:subPropertyOf cskg-ont:adaptedBy ;
    owl:inverseOf cskg-ont:adaptsMaterial .

cskg-ont:materialAffectedBy a owl:ObjectProperty ;
    rdfs:comment "This relation indicates that an instance	 of class Material was affected by an instance belonging to one of the following classes { Material, Method, OtherEntity, Task }. It is designed based on the following predicates extracted by the NLP pipeline: placate,provoke,engage,console,impair,repulse,shake,discombobulate,threaten,inflame,thrill,satisfy,unsettle,kill,enrapture,outrage,disgruntle,reassure,discompose,interest,alarm,engross,afflict,manipulate,edit,update,increase,replace,modify,fatigue,refresh,cut" ;
    rdfs:domain cskg-ont:Material ;
    rdfs:range _:N4a044612beb04386bcdaada212d06ee5 ;
    rdfs:subPropertyOf cskg-ont:affectedBy ;
    owl:inverseOf cskg-ont:affectsMaterial .

cskg-ont:materialAnalyzedBy a owl:ObjectProperty ;
    rdfs:comment "This relation indicates that an instance	 of class Material was analyzed by an instance belonging to one of the following classes { Method, Metric, OtherEntity, Task }. It is designed based on the following predicates extracted by the NLP pipeline: analyze,assess,study,try_on,scan,approximate,proofread,inspect,sample,research,check,appraise,analyse,examine,watch,audit,feel_out,go_over,consult,survey,test,assay,try,evaluate,investigate,monitor,regard,peruse,review,try_out,measure,calculate,address,estimate" ;
    rdfs:domain cskg-ont:Material ;
    rdfs:range _:Ne5f8f2eed38342769aec9a55551ff1a3 ;
    rdfs:subPropertyOf cskg-ont:analyzedBy ;
    owl:inverseOf cskg-ont:analyzesMaterial .

cskg-ont:materialAnnotatedBy a owl:ObjectProperty ;
    rdfs:comment "This relation indicates that an instance	 of class Material was annotated by an instance belonging to one of the following classes { Method, Metric, OtherEntity, Task }. It is designed based on the following predicates extracted by the NLP pipeline: scar,stipple,annotate,stamp,embroider,incise,inscribe,engrave,applique,imprint,paint,reinscribe,mark,sign,tag,label" ;
    rdfs:domain cskg-ont:Material ;
    rdfs:range _:Nba6a0d4144a14fc188678d3c3fff1a40 ;
    rdfs:subPropertyOf cskg-ont:annotatedBy ;
    owl:inverseOf cskg-ont:annotatesMaterial .

cskg-ont:materialBases a owl:ObjectProperty,
        owl:TransitiveProperty ;
    rdfs:comment "This relation indicates that an instance	 of class Material was bases by an instance belonging to one of the following classes { Material, Method, Metric, OtherEntity, Task }. It is designed based on the following predicates extracted by the NLP pipeline: base,ground,found,construe,build,establish" ;
    rdfs:domain cskg-ont:Material ;
    rdfs:range _:Ne7974f69047f4510883a7ef0862ea28f ;
    rdfs:subPropertyOf cskg-ont:bases ;
    owl:inverseOf cskg-ont:based-onMaterial .

cskg-ont:materialCausedBy a owl:ObjectProperty ;
    rdfs:comment "This relation indicates that an instance	 of class Material was caused by an instance belonging to one of the following classes { Material, Method, OtherEntity, Task }. It is designed based on the following predicates extracted by the NLP pipeline: cause,influence" ;
    rdfs:domain cskg-ont:Material ;
    rdfs:range _:Nd209a2155624478ea7c6565c8ea0f04a ;
    rdfs:subPropertyOf cskg-ont:causedBy ;
    owl:inverseOf cskg-ont:causesMaterial .

cskg-ont:materialClassifiedBy a owl:ObjectProperty ;
    rdfs:comment "This relation indicates that an instance	 of class Material was classified by an instance belonging to one of the following classes { Method, Metric, OtherEntity, Task }. It is designed based on the following predicates extracted by the NLP pipeline: regroup,bracket,categorize,recode,chunk,code,separate,group,sort,sort_out,catalogue,classify,class,number,seed,reclassify,grade" ;
    rdfs:domain cskg-ont:Material ;
    rdfs:range _:Ne6c5b294919942d0a05ec31ccf7d1e5f ;
    rdfs:subPropertyOf cskg-ont:classifiedBy ;
    owl:inverseOf cskg-ont:classifiesMaterial .

cskg-ont:materialContributedBy a owl:ObjectProperty ;
    rdfs:comment "This relation indicates that an instance	 of class Material was contributed by an instance belonging to one of the following classes { Method, OtherEntity, Task }. It is designed based on the following predicates extracted by the NLP pipeline: abnegate,gift,pass_out,turn-over,restore,turn-in,give-out,disburse,give-away,proffer,distribute,remit,transfer,extend,shell_out,give-up,hand_out,refer,disseminate,contribute" ;
    rdfs:domain cskg-ont:Material ;
    rdfs:range _:N502287740d5e4306a36a494e175957e8 ;
    rdfs:subPropertyOf cskg-ont:contributedBy ;
    owl:inverseOf cskg-ont:contributes-toMaterial .

cskg-ont:materialDiscussedBy a owl:ObjectProperty ;
    rdfs:comment "This relation indicates that an instance	 of class Material was discussed by an instance belonging to one of the following classes { Task }. It is designed based on the following predicates extracted by the NLP pipeline: debate,discuss,chatter,confer,converse,argue,discus" ;
    rdfs:domain cskg-ont:Material ;
    rdfs:range _:N6c31b3331102496698c40fe4ec35d364 ;
    rdfs:subPropertyOf cskg-ont:discussedBy ;
    owl:inverseOf cskg-ont:discussesMaterial .

cskg-ont:materialExecutedBy a owl:ObjectProperty,
        owl:TransitiveProperty ;
    rdfs:comment "This relation indicates that an instance	 of class Material was executed by an instance belonging to one of the following classes { Method, OtherEntity, Task }. It is designed based on the following predicates extracted by the NLP pipeline: perform,execute,operate,run,simulate,play,work,train,action" ;
    rdfs:domain cskg-ont:Material ;
    rdfs:range _:Nb5fb8f3ae4ef4e2093ed8d706e47a824 ;
    rdfs:subPropertyOf cskg-ont:executedBy ;
    owl:inverseOf cskg-ont:executesMaterial .

cskg-ont:materialExtractedBy a owl:ObjectProperty,
        owl:TransitiveProperty ;
    rdfs:comment "This relation indicates that an instance	 of class Material was extracted by an instance belonging to one of the following classes { Material, Method, OtherEntity, Task }. It is designed based on the following predicates extracted by the NLP pipeline: extract,mine,induce,infer" ;
    rdfs:domain cskg-ont:Material ;
    rdfs:range _:N247eb93c5ce04deba8a07ed3bdad5221 ;
    rdfs:subPropertyOf cskg-ont:extractedBy ;
    owl:inverseOf cskg-ont:extractsMaterial .

cskg-ont:materialGuidedBy a owl:ObjectProperty ;
    rdfs:comment "This relation indicates that an instance	 of class Material was guided by an instance belonging to one of the following classes { OtherEntity }. It is designed based on the following predicates extracted by the NLP pipeline: steer,conduct,guide,misdirect,lead,escort,accompany,direct" ;
    rdfs:domain cskg-ont:Material ;
    rdfs:range _:N70a6aff9428c4ea997f361b97a6d662c ;
    rdfs:subPropertyOf cskg-ont:guidedBy ;
    owl:inverseOf cskg-ont:guidesMaterial .

cskg-ont:materialHighlightedBy a owl:ObjectProperty ;
    rdfs:comment "This relation indicates that an instance	 of class Material was highlighted by an instance belonging to one of the following classes { Material, Method, Metric, OtherEntity, Task }. It is designed based on the following predicates extracted by the NLP pipeline: highlight,emphasize" ;
    rdfs:domain cskg-ont:Material ;
    rdfs:range _:N08286035189c4c1d815e149a72050a9d ;
    rdfs:subPropertyOf cskg-ont:highlightedBy ;
    owl:inverseOf cskg-ont:highlightsMaterial .

cskg-ont:materialIdentifiedBy a owl:ObjectProperty ;
    rdfs:comment "This relation indicates that an instance	 of class Material was identified by an instance belonging to one of the following classes { Method, OtherEntity, Task }. It is designed based on the following predicates extracted by the NLP pipeline: identify,detect,filter,recognize,locate" ;
    rdfs:domain cskg-ont:Material ;
    rdfs:range _:Nb30f3123fa034f52bf3b37967b773741 ;
    rdfs:subPropertyOf cskg-ont:identifiedBy ;
    owl:inverseOf cskg-ont:identifiesMaterial .

cskg-ont:materialImprovedBy a owl:ObjectProperty ;
    rdfs:comment "This relation indicates that an instance	 of class Material was improved by an instance belonging to one of the following classes { Method, Metric, OtherEntity, Task }. It is designed based on the following predicates extracted by the NLP pipeline: improve,evolve,grow,enrich,expand,augment,raise,enhance,advance,gain,optimize" ;
    rdfs:domain cskg-ont:Material ;
    rdfs:range _:N153e4415eed74d11915734588e6374d6 ;
    rdfs:subPropertyOf cskg-ont:improvedBy ;
    owl:inverseOf cskg-ont:improvesMaterial .

cskg-ont:materialIncludedBy a owl:ObjectProperty,
        owl:TransitiveProperty ;
    rdfs:comment "This relation indicates that an instance	 of class Material was included by an instance belonging to one of the following classes { Material, Method, OtherEntity, Task }. It is designed by the Feature-of and Part-of relationships extracted by the DyGIE++. It is also designed based on the following predicates extracted by the NLP pipeline: 'relate,include,involve,engage,enroll,embed,contain,comprise,carry,cover,consider,share,mount,have,equip,install" ;
    rdfs:domain cskg-ont:Material ;
    rdfs:range _:Nf9a039f5b7e649a9afbe2d6d8659f9fb ;
    rdfs:subPropertyOf cskg-ont:includedBy ;
    owl:inverseOf cskg-ont:includesMaterial .

cskg-ont:materialInteracts-With a owl:ObjectProperty ;
    rdfs:comment "This relation indicates that an instance	 of class Material was interacts-with by an instance belonging to one of the following classes { Material, Method, Metric, OtherEntity, Task }. It is designed based on the following predicates extracted by the NLP pipeline: renegotiate,compromise,agree,debate,interact,collaborate,disagree,communicate,haggle,interlink,participate" ;
    rdfs:domain cskg-ont:Material ;
    rdfs:range _:N9022ec3d1df544c39293f06d4a2915b4 ;
    rdfs:subPropertyOf cskg-ont:interacts-with ;
    owl:inverseOf cskg-ont:interacts-withMaterial .

cskg-ont:materialLackedof a owl:ObjectProperty ;
    rdfs:comment "This relation indicates that an instance	 of class Material was lackedof by an instance belonging to one of the following classes { Material, Method, Metric, OtherEntity, Task }. It is designed based on the following predicates extracted by the NLP pipeline: lack" ;
    rdfs:domain cskg-ont:Material ;
    rdfs:range _:N842e98b9e8e240b8b24fc5a53f53effa ;
    rdfs:subPropertyOf cskg-ont:lackedOf ;
    owl:inverseOf cskg-ont:lacksMaterial .

cskg-ont:materialLearnedBy a owl:ObjectProperty ;
    rdfs:comment "This relation indicates that an instance	 of class Material was learned by an instance belonging to one of the following classes { Material, Method, OtherEntity, Task }. It is designed based on the following predicates extracted by the NLP pipeline: memorize,glean,learn,study,absorb,assimilate,cram,relearn,read" ;
    rdfs:domain cskg-ont:Material ;
    rdfs:range _:N64948af7aad5415789b62c973ad807e4 ;
    rdfs:subPropertyOf cskg-ont:learnedBy ;
    owl:inverseOf cskg-ont:learnsMaterial .

cskg-ont:materialLimitedBy a owl:ObjectProperty ;
    rdfs:comment "This relation indicates that an instance	 of class Material was limited by an instance belonging to one of the following classes { Material, Method, OtherEntity, Task }. It is designed based on the following predicates extracted by the NLP pipeline: reduce,limit,confine,restrain,constrain,restrict,prevent" ;
    rdfs:domain cskg-ont:Material ;
    rdfs:range _:N6fbd7b79b82641238ccb201b4c0fc275 ;
    rdfs:subPropertyOf cskg-ont:limitedBy ;
    owl:inverseOf cskg-ont:limitsMaterial .

cskg-ont:materialLinkedBy a owl:ObjectProperty ;
    rdfs:comment "This relation indicates that an instance	 of class Material was linked by an instance belonging to one of the following classes { Method, Metric, Task }. It is designed based on the following predicates extracted by the NLP pipeline: fasten,strap,hook,lasso,leash,reeve,peg,rope,seal,clamp,latch,chain,band,trammel,shackle,clasp,knot,button,lock,moor,buckle,yoke,manacle,screw,link,string,pin,tether,paste,anchor,bond,wire,connect" ;
    rdfs:domain cskg-ont:Material ;
    rdfs:range _:Nc5e1db55c2f049efb0984d63efb8a66e ;
    rdfs:subPropertyOf cskg-ont:linkedBy ;
    owl:inverseOf cskg-ont:linksMaterial .

cskg-ont:materialManagedBy a owl:ObjectProperty ;
    rdfs:comment "This relation indicates that an instance	 of class Material was managed by an instance belonging to one of the following classes { Method, Task }. It is designed based on the following predicates extracted by the NLP pipeline: look_out,wait_on,look_after,care,manage,maintain,preserve,keep,handle,treat,deal,configure" ;
    rdfs:domain cskg-ont:Material ;
    rdfs:range _:N8a58b70d2de6491b9e2460616c6f8e88 ;
    rdfs:subPropertyOf cskg-ont:managedBy ;
    owl:inverseOf cskg-ont:managesMaterial .

cskg-ont:materialOutperformedBy a owl:ObjectProperty,
        owl:TransitiveProperty ;
    rdfs:comment "This relation indicates that an instance	 of class Material was outperformed by an instance belonging to one of the following classes { Material, Method, Metric, OtherEntity }. It is designed based on the following predicates extracted by the NLP pipeline: outperform" ;
    rdfs:domain cskg-ont:Material ;
    rdfs:range _:N8e228a8aba9841f88141006ed0d039c8 ;
    rdfs:subPropertyOf cskg-ont:outperformedBy ;
    owl:inverseOf cskg-ont:outperformsMaterial .

cskg-ont:materialPredictedBy a owl:ObjectProperty ;
    rdfs:comment "This relation indicates that an instance	 of class Material was predicted by an instance belonging to one of the following classes { Material, Method, OtherEntity, Task }. It is designed based on the following predicates extracted by the NLP pipeline: denote,corroborate,indicate,imply,predict,anticipate,forebode,say,expose,prognosticate,explain,forecast" ;
    rdfs:domain cskg-ont:Material ;
    rdfs:range _:N2a981ddad09442f3bbf2168fd92d119a ;
    rdfs:subPropertyOf cskg-ont:predictedBy ;
    owl:inverseOf cskg-ont:predictsMaterial .

cskg-ont:materialProcessedBy a owl:ObjectProperty ;
    rdfs:comment "This relation indicates that an instance	 of class Material was processed by an instance belonging to one of the following classes { Method, OtherEntity, Task }. It is designed based on the following predicates extracted by the NLP pipeline: process,proces" ;
    rdfs:domain cskg-ont:Material ;
    rdfs:range _:N7326ea397df347f1ab490fea703779f6 ;
    rdfs:subPropertyOf cskg-ont:processedBy ;
    owl:inverseOf cskg-ont:processesMaterial .

cskg-ont:materialProducedBy a owl:ObjectProperty ;
    rdfs:comment "This relation indicates that an instance	 of class Material was produced by an instance belonging to one of the following classes { Method, OtherEntity, Task }. It is designed based on the following predicates extracted by the NLP pipeline: author,coin,compose,compute,conoct,construct,contrive,cowrite,create,derive,draft,fabricate,form,formulate,invent,manufacture,model,organize,produce,rebuild,recreate,style,synthesize,write,generate,design,develop,implement,deploy,make,do" ;
    rdfs:domain cskg-ont:Material ;
    rdfs:range _:Na8f5f43e5b904317a7bbba3fbb34a41c ;
    rdfs:subPropertyOf cskg-ont:producedBy ;
    owl:inverseOf cskg-ont:producesMaterial .

cskg-ont:materialProposedBy a owl:ObjectProperty ;
    rdfs:comment "This relation indicates that an instance	 of class Material was proposed by an instance belonging to one of the following classes { Method, OtherEntity, Task }. It is designed based on the following predicates extracted by the NLP pipeline: propose,report,say,state,recommend,suggest,hint,introduce,outline,promise" ;
    rdfs:domain cskg-ont:Material ;
    rdfs:range _:Neada5e5673584d3b9a7f574d65dadc46 ;
    rdfs:subPropertyOf cskg-ont:proposedBy ;
    owl:inverseOf cskg-ont:proposesMaterial .

cskg-ont:materialProvidedBy a owl:ObjectProperty ;
    rdfs:comment "This relation indicates that an instance	 of class Material was provided by an instance belonging to one of the following classes { Method, OtherEntity, Task }. It is designed based on the following predicates extracted by the NLP pipeline: present,furnish,resupply,serve,supply,provide,yield,give,add,assign" ;
    rdfs:domain cskg-ont:Material ;
    rdfs:range _:N7b68838e3777448ab5f7047aa5a6120f ;
    rdfs:subPropertyOf cskg-ont:providedBy ;
    owl:inverseOf cskg-ont:providesMaterial .

cskg-ont:materialQueriedBy a owl:ObjectProperty ;
    rdfs:comment "This relation indicates that an instance	 of class Material was queried by an instance belonging to one of the following classes { Method, Task }. It is designed based on the following predicates extracted by the NLP pipeline: query" ;
    rdfs:domain cskg-ont:Material ;
    rdfs:range _:N1180ea8f3dc54e0d8b6efb545a5fd9fe ;
    rdfs:subPropertyOf cskg-ont:queriedBy ;
    owl:inverseOf cskg-ont:queriesMaterial .

cskg-ont:materialSolvedBy a owl:ObjectProperty ;
    rdfs:comment "This relation indicates that an instance	 of class Material was solved by an instance belonging to one of the following classes { Material, Method, Metric, OtherEntity, Task }. It is designed based on the following predicates extracted by the NLP pipeline: find,determine,see,rationalize,guess,deduce,solve,discover,pick_up,ascertain,realize,relearn,ascertain,realize,relearn,fix" ;
    rdfs:domain cskg-ont:Material ;
    rdfs:range _:Nfd15102f89754dcdb6b4cea4fe32762e ;
    rdfs:subPropertyOf cskg-ont:solvedBy ;
    owl:inverseOf cskg-ont:solvesMaterial .

cskg-ont:materialStandardizedBy a owl:ObjectProperty ;
    rdfs:comment "This relation indicates that an instance	 of class Material was standardized by an instance belonging to one of the following classes { Material, Method, Metric, OtherEntity, Task }. It is designed based on the following predicates extracted by the NLP pipeline: standardize,standardise" ;
    rdfs:domain cskg-ont:Material ;
    rdfs:range _:Nbc27e6b3f2f34bc39339daacb1b90191 ;
    rdfs:subPropertyOf cskg-ont:standardizedBy ;
    owl:inverseOf cskg-ont:standardizesMaterial .

cskg-ont:materialSupportedBy a owl:ObjectProperty ;
    rdfs:comment "This relation indicates that an instance	 of class Material was supported by an instance belonging to one of the following classes { Method, Task }. It is designed based on the following predicates extracted by the NLP pipeline: help,support,aid,assist,back,underlie,enable,promote,empower,facilitate,foster,facilitate,allow,hold,bear" ;
    rdfs:domain cskg-ont:Material ;
    rdfs:range _:N15a8080dcfdb43bf8d293acae48153f4 ;
    rdfs:subPropertyOf cskg-ont:supportedBy ;
    owl:inverseOf cskg-ont:supportsMaterial .

cskg-ont:materialTransferredBy a owl:ObjectProperty ;
    rdfs:comment "This relation indicates that an instance	 of class Material was transferred by an instance belonging to one of the following classes { Material, Method, Metric, OtherEntity, Task }. It is designed based on the following predicates extracted by the NLP pipeline: deliver,dispatch,shunt,airmail,import,forward,ship,send,transship,transmit,pass,hand,transport,shift,export,express,post,wire,transfer,drive,slip,port,return,convey,handdeliver,mail,answer" ;
    rdfs:domain cskg-ont:Material ;
    rdfs:range _:N9ca46b7d5ba948fb8d1bce22a5201cb9 ;
    rdfs:subPropertyOf cskg-ont:transferredBy ;
    owl:inverseOf cskg-ont:transfersMaterial .

cskg-ont:materialUsedBy a owl:ObjectProperty,
        owl:TransitiveProperty ;
    rdfs:comment "This relation indicates that an instance	 of class Material was used by an instance belonging to one of the following classes { Method, Metric, OtherEntity, Task }. It is designed by the Used-for relationships extracted by the DyGIE++. It is also designed based on the following predicates extracted by the NLP pipeline: apply,employ,exert,exploit,reuse,use,utilize,utilise,adopt,leverage,rely,access" ;
    rdfs:domain cskg-ont:Material ;
    rdfs:range _:N7737e44cf65944dc83e0afa0502ac699 ;
    rdfs:subPropertyOf cskg-ont:usedBy ;
    owl:inverseOf cskg-ont:usesMaterial .

cskg-ont:materialVisualizedBy a owl:ObjectProperty ;
    rdfs:comment "This relation indicates that an instance	 of class Material was visualized by an instance belonging to one of the following classes { Material, Method, OtherEntity }. It is designed based on the following predicates extracted by the NLP pipeline: visualize,disclose,reflect" ;
    rdfs:domain cskg-ont:Material ;
    rdfs:range _:N9651cd8605e0463690c4598807c85aca ;
    rdfs:subPropertyOf cskg-ont:visualizedBy ;
    owl:inverseOf cskg-ont:visualizesMaterial .

cskg-ont:methodAcquiredBy a owl:ObjectProperty,
        owl:TransitiveProperty ;
    rdfs:comment "This relation indicates that an instance	 of class Method was acquired by an instance belonging to one of the following classes { Method, OtherEntity, Task }. It is designed based on the following predicates extracted by the NLP pipeline: select,accumulate,recoup,source,receive,acquire,regain,retrieve,obtain,accrue,borrow,subselect,inherit,accept,collect,gather,store,attract,get,capture,record,achieve" ;
    rdfs:domain cskg-ont:Method ;
    rdfs:range _:Nb537d70acb5d4f7b83ce9774ba62ee76 ;
    rdfs:subPropertyOf cskg-ont:acquiredBy ;
    owl:inverseOf cskg-ont:acquiresMethod .

cskg-ont:methodAdaptedBy a owl:ObjectProperty,
        owl:TransitiveProperty ;
    rdfs:comment "This relation indicates that an instance	 of class Method was adapted by an instance belonging to one of the following classes { Method, OtherEntity, Task }. It is designed based on the following predicates extracted by the NLP pipeline: readapt,adjust,conform,adapt,gear,readjust,fit,assimilate,accommodate,personalize,customize,specialize,generalize,tailor,refine" ;
    rdfs:domain cskg-ont:Method ;
    rdfs:range _:N76f3d2c578754615a35c5ed25ed29481 ;
    rdfs:subPropertyOf cskg-ont:adaptedBy ;
    owl:inverseOf cskg-ont:adaptsMethod .

cskg-ont:methodAffectedBy a owl:ObjectProperty ;
    rdfs:comment "This relation indicates that an instance	 of class Method was affected by an instance belonging to one of the following classes { Method, Metric, OtherEntity, Task }. It is designed based on the following predicates extracted by the NLP pipeline: placate,provoke,engage,console,impair,repulse,shake,discombobulate,threaten,inflame,thrill,satisfy,unsettle,kill,enrapture,outrage,disgruntle,reassure,discompose,interest,alarm,engross,afflict,manipulate,edit,update,increase,replace,modify,fatigue,refresh,cut" ;
    rdfs:domain cskg-ont:Method ;
    rdfs:range _:N1bb86d25c9754b338b0a373bccca95bf ;
    rdfs:subPropertyOf cskg-ont:affectedBy ;
    owl:inverseOf cskg-ont:affectsMethod .

cskg-ont:methodAnalyzedBy a owl:ObjectProperty,
        owl:TransitiveProperty ;
    rdfs:comment "This relation indicates that an instance	 of class Method was analyzed by an instance belonging to one of the following classes { Method, Metric, OtherEntity, Task }. It is designed based on the following predicates extracted by the NLP pipeline: analyze,assess,study,try_on,scan,approximate,proofread,inspect,sample,research,check,appraise,analyse,examine,watch,audit,feel_out,go_over,consult,survey,test,assay,try,evaluate,investigate,monitor,regard,peruse,review,try_out,measure,calculate,address,estimate" ;
    rdfs:domain cskg-ont:Method ;
    rdfs:range _:N78e421076cfc4a1ea744c6a381116451 ;
    rdfs:subPropertyOf cskg-ont:analyzedBy ;
    owl:inverseOf cskg-ont:analyzesMethod .

cskg-ont:methodAnnotatedBy a owl:ObjectProperty ;
    rdfs:comment "This relation indicates that an instance	 of class Method was annotated by an instance belonging to one of the following classes { Method, Task }. It is designed based on the following predicates extracted by the NLP pipeline: scar,stipple,annotate,stamp,embroider,incise,inscribe,engrave,applique,imprint,paint,reinscribe,mark,sign,tag,label" ;
    rdfs:domain cskg-ont:Method ;
    rdfs:range _:N325b3b8c68e44ac286527bae7a46fc96 ;
    rdfs:subPropertyOf cskg-ont:annotatedBy ;
    owl:inverseOf cskg-ont:annotatesMethod .

cskg-ont:methodAutomatedBy a owl:ObjectProperty ;
    rdfs:comment "This relation indicates that an instance	 of class Method was automated by an instance belonging to one of the following classes { Method, Task }. It is designed based on the following predicates extracted by the NLP pipeline: automate" ;
    rdfs:domain cskg-ont:Method ;
    rdfs:range _:N8207716fbb6a4c14a67b17f93eb075d0 ;
    rdfs:subPropertyOf cskg-ont:automatedBy ;
    owl:inverseOf cskg-ont:automatesMethod .

cskg-ont:methodBases a owl:ObjectProperty,
        owl:TransitiveProperty ;
    rdfs:comment "This relation indicates that an instance	 of class Method was bases by an instance belonging to one of the following classes { Material, Method, Metric, OtherEntity, Task }. It is designed based on the following predicates extracted by the NLP pipeline: base,ground,found,construe,build,establish" ;
    rdfs:domain cskg-ont:Method ;
    rdfs:range _:N08fd05694b3f44ebb87a0f020839acee ;
    rdfs:subPropertyOf cskg-ont:bases ;
    owl:inverseOf cskg-ont:based-onMethod .

cskg-ont:methodCausedBy a owl:ObjectProperty ;
    rdfs:comment "This relation indicates that an instance	 of class Method was caused by an instance belonging to one of the following classes { Method, Metric, OtherEntity, Task }. It is designed based on the following predicates extracted by the NLP pipeline: cause,influence" ;
    rdfs:domain cskg-ont:Method ;
    rdfs:range _:Nbc785b4cd6cb4bcfa9eaa81652c25a8f ;
    rdfs:subPropertyOf cskg-ont:causedBy ;
    owl:inverseOf cskg-ont:causesMethod .

cskg-ont:methodClassifiedBy a owl:ObjectProperty ;
    rdfs:comment "This relation indicates that an instance	 of class Method was classified by an instance belonging to one of the following classes { Method, Metric, OtherEntity, Task }. It is designed based on the following predicates extracted by the NLP pipeline: regroup,bracket,categorize,recode,chunk,code,separate,group,sort,sort_out,catalogue,classify,class,number,seed,reclassify,grade" ;
    rdfs:domain cskg-ont:Method ;
    rdfs:range _:N96bcde7c4ac345708387678406877c6f ;
    rdfs:subPropertyOf cskg-ont:classifiedBy ;
    owl:inverseOf cskg-ont:classifiesMethod .

cskg-ont:methodContributedBy a owl:ObjectProperty ;
    rdfs:comment "This relation indicates that an instance	 of class Method was contributed by an instance belonging to one of the following classes { Method, Metric, OtherEntity, Task }. It is designed based on the following predicates extracted by the NLP pipeline: abnegate,gift,pass_out,turn-over,restore,turn-in,give-out,disburse,give-away,proffer,distribute,remit,transfer,extend,shell_out,give-up,hand_out,refer,disseminate,contribute" ;
    rdfs:domain cskg-ont:Method ;
    rdfs:range _:N0053e46091564bada9a0447722971667 ;
    rdfs:subPropertyOf cskg-ont:contributedBy ;
    owl:inverseOf cskg-ont:contributes-toMethod .

cskg-ont:methodDiscussedBy a owl:ObjectProperty ;
    rdfs:comment "This relation indicates that an instance	 of class Method was discussed by an instance belonging to one of the following classes { Method, Task }. It is designed based on the following predicates extracted by the NLP pipeline: debate,discuss,chatter,confer,converse,argue,discus" ;
    rdfs:domain cskg-ont:Method ;
    rdfs:range _:Nc6e13c900be140a09f05f8a8026e8bd1 ;
    rdfs:subPropertyOf cskg-ont:discussedBy ;
    owl:inverseOf cskg-ont:discussesMethod .

cskg-ont:methodExecutedBy a owl:ObjectProperty,
        owl:TransitiveProperty ;
    rdfs:comment "This relation indicates that an instance	 of class Method was executed by an instance belonging to one of the following classes { Method, Metric, OtherEntity, Task }. It is designed based on the following predicates extracted by the NLP pipeline: perform,execute,operate,run,simulate,play,work,train,action" ;
    rdfs:domain cskg-ont:Method ;
    rdfs:range _:N4aeafb7a405e4e7b91141051e25e7321 ;
    rdfs:subPropertyOf cskg-ont:executedBy ;
    owl:inverseOf cskg-ont:executesMethod .

cskg-ont:methodExtractedBy a owl:ObjectProperty,
        owl:TransitiveProperty ;
    rdfs:comment "This relation indicates that an instance	 of class Method was extracted by an instance belonging to one of the following classes { Material, Method, OtherEntity, Task }. It is designed based on the following predicates extracted by the NLP pipeline: extract,mine,induce,infer" ;
    rdfs:domain cskg-ont:Method ;
    rdfs:range _:Nbda0a556387e4fe5a06a56ee9bf2b863 ;
    rdfs:subPropertyOf cskg-ont:extractedBy ;
    owl:inverseOf cskg-ont:extractsMethod .

cskg-ont:methodGuidedBy a owl:ObjectProperty ;
    rdfs:comment "This relation indicates that an instance	 of class Method was guided by an instance belonging to one of the following classes { Method, Metric, OtherEntity, Task }. It is designed based on the following predicates extracted by the NLP pipeline: steer,conduct,guide,misdirect,lead,escort,accompany,direct" ;
    rdfs:domain cskg-ont:Method ;
    rdfs:range _:N51d8015b10504c6db235279c00bf373e ;
    rdfs:subPropertyOf cskg-ont:guidedBy ;
    owl:inverseOf cskg-ont:guidesMethod .

cskg-ont:methodHighlightedBy a owl:ObjectProperty ;
    rdfs:comment "This relation indicates that an instance	 of class Method was highlighted by an instance belonging to one of the following classes { Material, Method, Metric, OtherEntity, Task }. It is designed based on the following predicates extracted by the NLP pipeline: highlight,emphasize" ;
    rdfs:domain cskg-ont:Method ;
    rdfs:range _:N47b3eb8ba4ff46eeae0ebc5471a01be0 ;
    rdfs:subPropertyOf cskg-ont:highlightedBy ;
    owl:inverseOf cskg-ont:highlightsMethod .

cskg-ont:methodIdentifiedBy a owl:ObjectProperty ;
    rdfs:comment "This relation indicates that an instance	 of class Method was identified by an instance belonging to one of the following classes { Method, OtherEntity, Task }. It is designed based on the following predicates extracted by the NLP pipeline: identify,detect,filter,recognize,locate" ;
    rdfs:domain cskg-ont:Method ;
    rdfs:range _:N2824d69514f949f49091964a1b85a3a6 ;
    rdfs:subPropertyOf cskg-ont:identifiedBy ;
    owl:inverseOf cskg-ont:identifiesMethod .

cskg-ont:methodImprovedBy a owl:ObjectProperty ;
    rdfs:comment "This relation indicates that an instance	 of class Method was improved by an instance belonging to one of the following classes { Material, Method, Metric, OtherEntity, Task }. It is designed based on the following predicates extracted by the NLP pipeline: improve,evolve,grow,enrich,expand,augment,raise,enhance,advance,gain,optimize" ;
    rdfs:domain cskg-ont:Method ;
    rdfs:range _:Nf64606f7c1a94762924496d321d021f3 ;
    rdfs:subPropertyOf cskg-ont:improvedBy ;
    owl:inverseOf cskg-ont:improvesMethod .

cskg-ont:methodIncludedBy a owl:ObjectProperty,
        owl:TransitiveProperty ;
    rdfs:comment "This relation indicates that an instance	 of class Method was included by an instance belonging to one of the following classes { Method, OtherEntity, Task }. It is designed by the Feature-of and Part-of relationships extracted by the DyGIE++. It is also designed based on the following predicates extracted by the NLP pipeline: 'relate,include,involve,engage,enroll,embed,contain,comprise,carry,cover,consider,share,mount,have,equip,install" ;
    rdfs:domain cskg-ont:Method ;
    rdfs:range _:Nf653e74b64c64b5fb48fb838f3e9088c ;
    rdfs:subPropertyOf cskg-ont:includedBy ;
    owl:inverseOf cskg-ont:includesMethod .

cskg-ont:methodInteracts-With a owl:ObjectProperty ;
    rdfs:comment "This relation indicates that an instance	 of class Method was interacts-with by an instance belonging to one of the following classes { Material, Method, Metric, OtherEntity, Task }. It is designed based on the following predicates extracted by the NLP pipeline: renegotiate,compromise,agree,debate,interact,collaborate,disagree,communicate,haggle,interlink,participate" ;
    rdfs:domain cskg-ont:Method ;
    rdfs:range _:N30ac83d4034e493dbbf4dced9bfc0300 ;
    rdfs:subPropertyOf cskg-ont:interacts-with ;
    owl:inverseOf cskg-ont:interacts-withMethod .

cskg-ont:methodLackedof a owl:ObjectProperty ;
    rdfs:comment "This relation indicates that an instance	 of class Method was lackedof by an instance belonging to one of the following classes { Material, Method, Metric, OtherEntity, Task }. It is designed based on the following predicates extracted by the NLP pipeline: lack" ;
    rdfs:domain cskg-ont:Method ;
    rdfs:range _:N8fe46fa8ab734ea18a302a274498734c ;
    rdfs:subPropertyOf cskg-ont:lackedOf ;
    owl:inverseOf cskg-ont:lacksMethod .

cskg-ont:methodLearnedBy a owl:ObjectProperty ;
    rdfs:comment "This relation indicates that an instance	 of class Method was learned by an instance belonging to one of the following classes { Material, Method, OtherEntity, Task }. It is designed based on the following predicates extracted by the NLP pipeline: memorize,glean,learn,study,absorb,assimilate,cram,relearn,read" ;
    rdfs:domain cskg-ont:Method ;
    rdfs:range _:Nbcdeafe6bedf4949bb33dd323b560164 ;
    rdfs:subPropertyOf cskg-ont:learnedBy ;
    owl:inverseOf cskg-ont:learnsMethod .

cskg-ont:methodLimitedBy a owl:ObjectProperty ;
    rdfs:comment "This relation indicates that an instance	 of class Method was limited by an instance belonging to one of the following classes { Material, Method, OtherEntity, Task }. It is designed based on the following predicates extracted by the NLP pipeline: reduce,limit,confine,restrain,constrain,restrict,prevent" ;
    rdfs:domain cskg-ont:Method ;
    rdfs:range _:Nc935650e9b464fcc9855696059362122 ;
    rdfs:subPropertyOf cskg-ont:limitedBy ;
    owl:inverseOf cskg-ont:limitsMethod .

cskg-ont:methodLinkedBy a owl:ObjectProperty,
        owl:TransitiveProperty ;
    rdfs:comment "This relation indicates that an instance	 of class Method was linked by an instance belonging to one of the following classes { Method, OtherEntity, Task }. It is designed based on the following predicates extracted by the NLP pipeline: fasten,strap,hook,lasso,leash,reeve,peg,rope,seal,clamp,latch,chain,band,trammel,shackle,clasp,knot,button,lock,moor,buckle,yoke,manacle,screw,link,string,pin,tether,paste,anchor,bond,wire,connect" ;
    rdfs:domain cskg-ont:Method ;
    rdfs:range _:N33b475fad8e94666ab0c0d8f6bb77516 ;
    rdfs:subPropertyOf cskg-ont:linkedBy ;
    owl:inverseOf cskg-ont:linksMethod .

cskg-ont:methodManagedBy a owl:ObjectProperty,
        owl:TransitiveProperty ;
    rdfs:comment "This relation indicates that an instance	 of class Method was managed by an instance belonging to one of the following classes { Method, Task }. It is designed based on the following predicates extracted by the NLP pipeline: look_out,wait_on,look_after,care,manage,maintain,preserve,keep,handle,treat,deal,configure" ;
    rdfs:domain cskg-ont:Method ;
    rdfs:range _:Nebf399080e1a4380a2c8f1c7401f0c10 ;
    rdfs:subPropertyOf cskg-ont:managedBy ;
    owl:inverseOf cskg-ont:managesMethod .

cskg-ont:methodMatchedBy a owl:ObjectProperty ;
    rdfs:comment "This relation indicates that an instance	 of class Method was matched by an instance belonging to one of the following classes { Method, Task }. It is designed based on the following predicates extracted by the NLP pipeline: harmonize,go,square,dovetail,couple,pair,alternate,align,map,compare,match" ;
    rdfs:domain cskg-ont:Method ;
    rdfs:range _:N40a65d8582d6409cae8d3048379836d9 ;
    rdfs:subPropertyOf cskg-ont:matchedBy ;
    owl:inverseOf cskg-ont:matchesMethod .

cskg-ont:methodOutperformedBy a owl:ObjectProperty,
        owl:TransitiveProperty ;
    rdfs:comment "This relation indicates that an instance	 of class Method was outperformed by an instance belonging to one of the following classes { Material, Method, Metric, OtherEntity, Task }. It is designed based on the following predicates extracted by the NLP pipeline: outperform" ;
    rdfs:domain cskg-ont:Method ;
    rdfs:range _:N8018a76176324d59bbe6d65bbdb0c9e4 ;
    rdfs:subPropertyOf cskg-ont:outperformedBy ;
    owl:inverseOf cskg-ont:outperformsMethod .

cskg-ont:methodPredictedBy a owl:ObjectProperty ;
    rdfs:comment "This relation indicates that an instance	 of class Method was predicted by an instance belonging to one of the following classes { Material, Method, OtherEntity, Task }. It is designed based on the following predicates extracted by the NLP pipeline: denote,corroborate,indicate,imply,predict,anticipate,forebode,say,expose,prognosticate,explain,forecast" ;
    rdfs:domain cskg-ont:Method ;
    rdfs:range _:N1a90f39251084963a0e43a269d1c9d13 ;
    rdfs:subPropertyOf cskg-ont:predictedBy ;
    owl:inverseOf cskg-ont:predictsMethod .

cskg-ont:methodProcessedBy a owl:ObjectProperty ;
    rdfs:comment "This relation indicates that an instance	 of class Method was processed by an instance belonging to one of the following classes { Method, Task }. It is designed based on the following predicates extracted by the NLP pipeline: process,proces" ;
    rdfs:domain cskg-ont:Method ;
    rdfs:range _:N955dfd3e9c954207b4ffe0c9f2f9daf2 ;
    rdfs:subPropertyOf cskg-ont:processedBy ;
    owl:inverseOf cskg-ont:processesMethod .

cskg-ont:methodProducedBy a owl:ObjectProperty,
        owl:TransitiveProperty ;
    rdfs:comment "This relation indicates that an instance	 of class Method was produced by an instance belonging to one of the following classes { Method, OtherEntity, Task }. It is designed based on the following predicates extracted by the NLP pipeline: author,coin,compose,compute,conoct,construct,contrive,cowrite,create,derive,draft,fabricate,form,formulate,invent,manufacture,model,organize,produce,rebuild,recreate,style,synthesize,write,generate,design,develop,implement,deploy,make,do" ;
    rdfs:domain cskg-ont:Method ;
    rdfs:range _:Nd5ef3a6440db43dfb488042b013f990a ;
    rdfs:subPropertyOf cskg-ont:producedBy ;
    owl:inverseOf cskg-ont:producesMethod .

cskg-ont:methodProposedBy a owl:ObjectProperty ;
    rdfs:comment "This relation indicates that an instance	 of class Method was proposed by an instance belonging to one of the following classes { Method, OtherEntity, Task }. It is designed based on the following predicates extracted by the NLP pipeline: propose,report,say,state,recommend,suggest,hint,introduce,outline,promise" ;
    rdfs:domain cskg-ont:Method ;
    rdfs:range _:Ndfef39aead1d4430a1744fb242c62a0d ;
    rdfs:subPropertyOf cskg-ont:proposedBy ;
    owl:inverseOf cskg-ont:proposesMethod .

cskg-ont:methodProvidedBy a owl:ObjectProperty,
        owl:TransitiveProperty ;
    rdfs:comment "This relation indicates that an instance	 of class Method was provided by an instance belonging to one of the following classes { Method, OtherEntity, Task }. It is designed based on the following predicates extracted by the NLP pipeline: present,furnish,resupply,serve,supply,provide,yield,give,add,assign" ;
    rdfs:domain cskg-ont:Method ;
    rdfs:range _:N7ae089cecafe4d34ae8b2bb2964db95b ;
    rdfs:subPropertyOf cskg-ont:providedBy ;
    owl:inverseOf cskg-ont:providesMethod .

cskg-ont:methodSolvedBy a owl:ObjectProperty ;
    rdfs:comment "This relation indicates that an instance	 of class Method was solved by an instance belonging to one of the following classes { Material, Method, Metric, OtherEntity, Task }. It is designed based on the following predicates extracted by the NLP pipeline: find,determine,see,rationalize,guess,deduce,solve,discover,pick_up,ascertain,realize,relearn,ascertain,realize,relearn,fix" ;
    rdfs:domain cskg-ont:Method ;
    rdfs:range _:Nf9274a4f2b844ee292c2dc38853f9e4c ;
    rdfs:subPropertyOf cskg-ont:solvedBy ;
    owl:inverseOf cskg-ont:solvesMethod .

cskg-ont:methodStandardizedBy a owl:ObjectProperty ;
    rdfs:comment "This relation indicates that an instance	 of class Method was standardized by an instance belonging to one of the following classes { Material, Method, Metric, OtherEntity, Task }. It is designed based on the following predicates extracted by the NLP pipeline: standardize,standardise" ;
    rdfs:domain cskg-ont:Method ;
    rdfs:range _:N924787736fc3410a819e8c65bb11079a ;
    rdfs:subPropertyOf cskg-ont:standardizedBy ;
    owl:inverseOf cskg-ont:standardizesMethod .

cskg-ont:methodSupportedBy a owl:ObjectProperty ;
    rdfs:comment "This relation indicates that an instance	 of class Method was supported by an instance belonging to one of the following classes { Material, Method, Metric, OtherEntity, Task }. It is designed based on the following predicates extracted by the NLP pipeline: help,support,aid,assist,back,underlie,enable,promote,empower,facilitate,foster,facilitate,allow,hold,bear" ;
    rdfs:domain cskg-ont:Method ;
    rdfs:range _:N2a8dec03baeb4ec8b05703ac02a71e46 ;
    rdfs:subPropertyOf cskg-ont:supportedBy ;
    owl:inverseOf cskg-ont:supportsMethod .

cskg-ont:methodTransferredBy a owl:ObjectProperty ;
    rdfs:comment "This relation indicates that an instance	 of class Method was transferred by an instance belonging to one of the following classes { Material, Method, Metric, OtherEntity, Task }. It is designed based on the following predicates extracted by the NLP pipeline: deliver,dispatch,shunt,airmail,import,forward,ship,send,transship,transmit,pass,hand,transport,shift,export,express,post,wire,transfer,drive,slip,port,return,convey,handdeliver,mail,answer" ;
    rdfs:domain cskg-ont:Method ;
    rdfs:range _:N3a1bcb2947c843f1be540ff3d252bbe9 ;
    rdfs:subPropertyOf cskg-ont:transferredBy ;
    owl:inverseOf cskg-ont:transfersMethod .

cskg-ont:methodUsedBy a owl:ObjectProperty,
        owl:TransitiveProperty ;
    rdfs:comment "This relation indicates that an instance	 of class Method was used by an instance belonging to one of the following classes { Method, Metric, OtherEntity, Task }. It is designed by the Used-for relationships extracted by the DyGIE++. It is also designed based on the following predicates extracted by the NLP pipeline: apply,employ,exert,exploit,reuse,use,utilize,utilise,adopt,leverage,rely,access" ;
    rdfs:domain cskg-ont:Method ;
    rdfs:range _:Na1375b14902d42048768204c5ce0711f ;
    rdfs:subPropertyOf cskg-ont:usedBy ;
    owl:inverseOf cskg-ont:usesMethod .

cskg-ont:methodVisualizedBy a owl:ObjectProperty ;
    rdfs:comment "This relation indicates that an instance	 of class Method was visualized by an instance belonging to one of the following classes { Material, Method, OtherEntity, Task }. It is designed based on the following predicates extracted by the NLP pipeline: visualize,disclose,reflect" ;
    rdfs:domain cskg-ont:Method ;
    rdfs:range _:N6164b28feaa64c4c9bea7aaae8ca2c72 ;
    rdfs:subPropertyOf cskg-ont:visualizedBy ;
    owl:inverseOf cskg-ont:visualizesMethod .

cskg-ont:metricAcquiredBy a owl:ObjectProperty ;
    rdfs:comment "This relation indicates that an instance	 of class Metric was acquired by an instance belonging to one of the following classes { Method, OtherEntity, Task }. It is designed based on the following predicates extracted by the NLP pipeline: select,accumulate,recoup,source,receive,acquire,regain,retrieve,obtain,accrue,borrow,subselect,inherit,accept,collect,gather,store,attract,get,capture,record,achieve" ;
    rdfs:domain cskg-ont:Metric ;
    rdfs:range _:Ne250491a99094a61a35c8792c5f8c59c ;
    rdfs:subPropertyOf cskg-ont:acquiredBy ;
    owl:inverseOf cskg-ont:acquiresMetric .

cskg-ont:metricAdaptedBy a owl:ObjectProperty ;
    rdfs:comment "This relation indicates that an instance	 of class Metric was adapted by an instance belonging to one of the following classes { Method, OtherEntity, Task }. It is designed based on the following predicates extracted by the NLP pipeline: readapt,adjust,conform,adapt,gear,readjust,fit,assimilate,accommodate,personalize,customize,specialize,generalize,tailor,refine" ;
    rdfs:domain cskg-ont:Metric ;
    rdfs:range _:N1f6623cc3bef4f9e98932345e573de01 ;
    rdfs:subPropertyOf cskg-ont:adaptedBy ;
    owl:inverseOf cskg-ont:adaptsMetric .

cskg-ont:metricAffectedBy a owl:ObjectProperty ;
    rdfs:comment "This relation indicates that an instance	 of class Metric was affected by an instance belonging to one of the following classes { Method, Metric, OtherEntity, Task }. It is designed based on the following predicates extracted by the NLP pipeline: placate,provoke,engage,console,impair,repulse,shake,discombobulate,threaten,inflame,thrill,satisfy,unsettle,kill,enrapture,outrage,disgruntle,reassure,discompose,interest,alarm,engross,afflict,manipulate,edit,update,increase,replace,modify,fatigue,refresh,cut" ;
    rdfs:domain cskg-ont:Metric ;
    rdfs:range _:N1802d0de86f3405b9653a79f47cac09e ;
    rdfs:subPropertyOf cskg-ont:affectedBy ;
    owl:inverseOf cskg-ont:affectsMetric .

cskg-ont:metricAnalyzedBy a owl:ObjectProperty ;
    rdfs:comment "This relation indicates that an instance	 of class Metric was analyzed by an instance belonging to one of the following classes { Method, Metric, OtherEntity, Task }. It is designed based on the following predicates extracted by the NLP pipeline: analyze,assess,study,try_on,scan,approximate,proofread,inspect,sample,research,check,appraise,analyse,examine,watch,audit,feel_out,go_over,consult,survey,test,assay,try,evaluate,investigate,monitor,regard,peruse,review,try_out,measure,calculate,address,estimate" ;
    rdfs:domain cskg-ont:Metric ;
    rdfs:range _:N58074e7205704ced9fcc9e9a6a38b145 ;
    rdfs:subPropertyOf cskg-ont:analyzedBy ;
    owl:inverseOf cskg-ont:analyzesMetric .

cskg-ont:metricBases a owl:ObjectProperty,
        owl:TransitiveProperty ;
    rdfs:comment "This relation indicates that an instance	 of class Metric was bases by an instance belonging to one of the following classes { Material, Method, Metric, OtherEntity, Task }. It is designed based on the following predicates extracted by the NLP pipeline: base,ground,found,construe,build,establish" ;
    rdfs:domain cskg-ont:Metric ;
    rdfs:range _:N3affbed2bf194787b6196c968430d26c ;
    rdfs:subPropertyOf cskg-ont:bases ;
    owl:inverseOf cskg-ont:based-onMetric .

cskg-ont:metricCausedBy a owl:ObjectProperty ;
    rdfs:comment "This relation indicates that an instance	 of class Metric was caused by an instance belonging to one of the following classes { Method, Metric, OtherEntity }. It is designed based on the following predicates extracted by the NLP pipeline: cause,influence" ;
    rdfs:domain cskg-ont:Metric ;
    rdfs:range _:Na5876f2af4d34f668446c417e896ca6f ;
    rdfs:subPropertyOf cskg-ont:causedBy ;
    owl:inverseOf cskg-ont:causesMetric .

cskg-ont:metricClassifiedBy a owl:ObjectProperty ;
    rdfs:comment "This relation indicates that an instance	 of class Metric was classified by an instance belonging to one of the following classes { Method, Metric, OtherEntity }. It is designed based on the following predicates extracted by the NLP pipeline: regroup,bracket,categorize,recode,chunk,code,separate,group,sort,sort_out,catalogue,classify,class,number,seed,reclassify,grade" ;
    rdfs:domain cskg-ont:Metric ;
    rdfs:range _:N5454fd48e8d24c3ba6385a8dbd5c286e ;
    rdfs:subPropertyOf cskg-ont:classifiedBy ;
    owl:inverseOf cskg-ont:classifiesMetric .

cskg-ont:metricContributedBy a owl:ObjectProperty ;
    rdfs:comment "This relation indicates that an instance	 of class Metric was contributed by an instance belonging to one of the following classes { Method, Metric, OtherEntity, Task }. It is designed based on the following predicates extracted by the NLP pipeline: abnegate,gift,pass_out,turn-over,restore,turn-in,give-out,disburse,give-away,proffer,distribute,remit,transfer,extend,shell_out,give-up,hand_out,refer,disseminate,contribute" ;
    rdfs:domain cskg-ont:Metric ;
    rdfs:range _:N689f07c9e0f04b3d90b900367988b31d ;
    rdfs:subPropertyOf cskg-ont:contributedBy ;
    owl:inverseOf cskg-ont:contributes-toMetric .

cskg-ont:metricDiscussedBy a owl:ObjectProperty ;
    rdfs:comment "This relation indicates that an instance	 of class Metric was discussed by an instance belonging to one of the following classes { Task }. It is designed based on the following predicates extracted by the NLP pipeline: debate,discuss,chatter,confer,converse,argue,discus" ;
    rdfs:domain cskg-ont:Metric ;
    rdfs:range _:Nbdede62bcfd74bcd89207501aff28ae0 ;
    rdfs:subPropertyOf cskg-ont:discussedBy ;
    owl:inverseOf cskg-ont:discussesMetric .

cskg-ont:metricExtractedBy a owl:ObjectProperty,
        owl:TransitiveProperty ;
    rdfs:comment "This relation indicates that an instance	 of class Metric was extracted by an instance belonging to one of the following classes { Material, Method, OtherEntity, Task }. It is designed based on the following predicates extracted by the NLP pipeline: extract,mine,induce,infer" ;
    rdfs:domain cskg-ont:Metric ;
    rdfs:range _:N3104c110b5ba4b969038f41603f6014c ;
    rdfs:subPropertyOf cskg-ont:extractedBy ;
    owl:inverseOf cskg-ont:extractsMetric .

cskg-ont:metricGuidedBy a owl:ObjectProperty ;
    rdfs:comment "This relation indicates that an instance	 of class Metric was guided by an instance belonging to one of the following classes { Method, Metric, OtherEntity, Task }. It is designed based on the following predicates extracted by the NLP pipeline: steer,conduct,guide,misdirect,lead,escort,accompany,direct" ;
    rdfs:domain cskg-ont:Metric ;
    rdfs:range _:Na18faff524ce44c3a7bd793776599add ;
    rdfs:subPropertyOf cskg-ont:guidedBy ;
    owl:inverseOf cskg-ont:guidesMetric .

cskg-ont:metricHighlightedBy a owl:ObjectProperty ;
    rdfs:comment "This relation indicates that an instance	 of class Metric was highlighted by an instance belonging to one of the following classes { Material, Method, Metric, OtherEntity, Task }. It is designed based on the following predicates extracted by the NLP pipeline: highlight,emphasize" ;
    rdfs:domain cskg-ont:Metric ;
    rdfs:range _:N7d3fce177c8d4cb5af61d158778e6aee ;
    rdfs:subPropertyOf cskg-ont:highlightedBy ;
    owl:inverseOf cskg-ont:highlightsMetric .

cskg-ont:metricIdentifiedBy a owl:ObjectProperty ;
    rdfs:comment "This relation indicates that an instance	 of class Metric was identified by an instance belonging to one of the following classes { Method, OtherEntity, Task }. It is designed based on the following predicates extracted by the NLP pipeline: identify,detect,filter,recognize,locate" ;
    rdfs:domain cskg-ont:Metric ;
    rdfs:range _:N14089d541ce349aaaa4fd1b63fd36a00 ;
    rdfs:subPropertyOf cskg-ont:identifiedBy ;
    owl:inverseOf cskg-ont:identifiesMetric .

cskg-ont:metricImprovedBy a owl:ObjectProperty ;
    rdfs:comment "This relation indicates that an instance	 of class Metric was improved by an instance belonging to one of the following classes { Method, Metric, OtherEntity, Task }. It is designed based on the following predicates extracted by the NLP pipeline: improve,evolve,grow,enrich,expand,augment,raise,enhance,advance,gain,optimize" ;
    rdfs:domain cskg-ont:Metric ;
    rdfs:range _:Na29cd5ad9ddc439d8d35a10b6625d264 ;
    rdfs:subPropertyOf cskg-ont:improvedBy ;
    owl:inverseOf cskg-ont:improvesMetric .

cskg-ont:metricIncludedBy a owl:ObjectProperty ;
    rdfs:comment "This relation indicates that an instance	 of class Metric was included by an instance belonging to one of the following classes { Material, Method, OtherEntity, Task }. It is designed by the Feature-of and Part-of relationships extracted by the DyGIE++. It is also designed based on the following predicates extracted by the NLP pipeline: 'relate,include,involve,engage,enroll,embed,contain,comprise,carry,cover,consider,share,mount,have,equip,install" ;
    rdfs:domain cskg-ont:Metric ;
    rdfs:range _:N1b7fcb3709b14ff3b9f3959d221e3dca ;
    rdfs:subPropertyOf cskg-ont:includedBy ;
    owl:inverseOf cskg-ont:includesMetric .

cskg-ont:metricInteracts-With a owl:ObjectProperty ;
    rdfs:comment "This relation indicates that an instance	 of class Metric was interacts-with by an instance belonging to one of the following classes { Material, Method, Metric, OtherEntity, Task }. It is designed based on the following predicates extracted by the NLP pipeline: renegotiate,compromise,agree,debate,interact,collaborate,disagree,communicate,haggle,interlink,participate" ;
    rdfs:domain cskg-ont:Metric ;
    rdfs:range _:N4f8cc36c01214c6ba562824bbde43bd2 ;
    rdfs:subPropertyOf cskg-ont:interacts-with ;
    owl:inverseOf cskg-ont:interacts-withMetric .

cskg-ont:metricLackedof a owl:ObjectProperty ;
    rdfs:comment "This relation indicates that an instance	 of class Metric was lackedof by an instance belonging to one of the following classes { Material, Method, OtherEntity, Task }. It is designed based on the following predicates extracted by the NLP pipeline: lack" ;
    rdfs:domain cskg-ont:Metric ;
    rdfs:range _:N4d1a78f54cdb41009c4456a977760171 ;
    rdfs:subPropertyOf cskg-ont:lackedOf ;
    owl:inverseOf cskg-ont:lacksMetric .

cskg-ont:metricLimitedBy a owl:ObjectProperty ;
    rdfs:comment "This relation indicates that an instance	 of class Metric was limited by an instance belonging to one of the following classes { Material, Method, Metric, OtherEntity }. It is designed based on the following predicates extracted by the NLP pipeline: reduce,limit,confine,restrain,constrain,restrict,prevent" ;
    rdfs:domain cskg-ont:Metric ;
    rdfs:range _:N3002f74f0b844bec8d66e889c133c828 ;
    rdfs:subPropertyOf cskg-ont:limitedBy ;
    owl:inverseOf cskg-ont:limitsMetric .

cskg-ont:metricManagedBy a owl:ObjectProperty ;
    rdfs:comment "This relation indicates that an instance	 of class Metric was managed by an instance belonging to one of the following classes { Method, Task }. It is designed based on the following predicates extracted by the NLP pipeline: look_out,wait_on,look_after,care,manage,maintain,preserve,keep,handle,treat,deal,configure" ;
    rdfs:domain cskg-ont:Metric ;
    rdfs:range _:Nf70066e61f4d46c1993c8d54a7fc726c ;
    rdfs:subPropertyOf cskg-ont:managedBy ;
    owl:inverseOf cskg-ont:managesMetric .

cskg-ont:metricMatchedBy a owl:ObjectProperty ;
    rdfs:comment "This relation indicates that an instance	 of class Metric was matched by an instance belonging to one of the following classes { Method }. It is designed based on the following predicates extracted by the NLP pipeline: harmonize,go,square,dovetail,couple,pair,alternate,align,map,compare,match" ;
    rdfs:domain cskg-ont:Metric ;
    rdfs:range _:N3e79eb16e49543fe827090de5929a49d ;
    rdfs:subPropertyOf cskg-ont:matchedBy ;
    owl:inverseOf cskg-ont:matchesMetric .

cskg-ont:metricOutperformedBy a owl:ObjectProperty,
        owl:TransitiveProperty ;
    rdfs:comment "This relation indicates that an instance	 of class Metric was outperformed by an instance belonging to one of the following classes { Metric }. It is designed based on the following predicates extracted by the NLP pipeline: outperform" ;
    rdfs:domain cskg-ont:Metric ;
    rdfs:range _:Nb4d555962720432b9706eed1174a7f35 ;
    rdfs:subPropertyOf cskg-ont:outperformedBy ;
    owl:inverseOf cskg-ont:outperformsMetric .

cskg-ont:metricPredictedBy a owl:ObjectProperty ;
    rdfs:comment "This relation indicates that an instance	 of class Metric was predicted by an instance belonging to one of the following classes { Method, Task }. It is designed based on the following predicates extracted by the NLP pipeline: denote,corroborate,indicate,imply,predict,anticipate,forebode,say,expose,prognosticate,explain,forecast" ;
    rdfs:domain cskg-ont:Metric ;
    rdfs:range _:N0bd7083d9bbc422f92e266e47b20363d ;
    rdfs:subPropertyOf cskg-ont:predictedBy ;
    owl:inverseOf cskg-ont:predictsMetric .

cskg-ont:metricProcessedBy a owl:ObjectProperty ;
    rdfs:comment "This relation indicates that an instance	 of class Metric was processed by an instance belonging to one of the following classes { Method, Task }. It is designed based on the following predicates extracted by the NLP pipeline: process,proces" ;
    rdfs:domain cskg-ont:Metric ;
    rdfs:range _:N988dc0f7e5f6414780c74ecda82f8bcb ;
    rdfs:subPropertyOf cskg-ont:processedBy ;
    owl:inverseOf cskg-ont:processesMetric .

cskg-ont:metricProducedBy a owl:ObjectProperty ;
    rdfs:comment "This relation indicates that an instance	 of class Metric was produced by an instance belonging to one of the following classes { Method, OtherEntity, Task }. It is designed based on the following predicates extracted by the NLP pipeline: author,coin,compose,compute,conoct,construct,contrive,cowrite,create,derive,draft,fabricate,form,formulate,invent,manufacture,model,organize,produce,rebuild,recreate,style,synthesize,write,generate,design,develop,implement,deploy,make,do" ;
    rdfs:domain cskg-ont:Metric ;
    rdfs:range _:Ne16adafdc323491d984944c180663627 ;
    rdfs:subPropertyOf cskg-ont:producedBy ;
    owl:inverseOf cskg-ont:producesMetric .

cskg-ont:metricProposedBy a owl:ObjectProperty ;
    rdfs:comment "This relation indicates that an instance	 of class Metric was proposed by an instance belonging to one of the following classes { Method, OtherEntity, Task }. It is designed based on the following predicates extracted by the NLP pipeline: propose,report,say,state,recommend,suggest,hint,introduce,outline,promise" ;
    rdfs:domain cskg-ont:Metric ;
    rdfs:range _:N2af9352be5834a908acd7941b06493e3 ;
    rdfs:subPropertyOf cskg-ont:proposedBy ;
    owl:inverseOf cskg-ont:proposesMetric .

cskg-ont:metricProvidedBy a owl:ObjectProperty ;
    rdfs:comment "This relation indicates that an instance	 of class Metric was provided by an instance belonging to one of the following classes { Method, OtherEntity, Task }. It is designed based on the following predicates extracted by the NLP pipeline: present,furnish,resupply,serve,supply,provide,yield,give,add,assign" ;
    rdfs:domain cskg-ont:Metric ;
    rdfs:range _:N497f9c02321348b5a5460e2adbe2e14d ;
    rdfs:subPropertyOf cskg-ont:providedBy ;
    owl:inverseOf cskg-ont:providesMetric .

cskg-ont:metricSolvedBy a owl:ObjectProperty ;
    rdfs:comment "This relation indicates that an instance	 of class Metric was solved by an instance belonging to one of the following classes { Material, Method, Metric, OtherEntity, Task }. It is designed based on the following predicates extracted by the NLP pipeline: find,determine,see,rationalize,guess,deduce,solve,discover,pick_up,ascertain,realize,relearn,ascertain,realize,relearn,fix" ;
    rdfs:domain cskg-ont:Metric ;
    rdfs:range _:N49ce4eca3edd4cc78b03a189cc38cd71 ;
    rdfs:subPropertyOf cskg-ont:solvedBy ;
    owl:inverseOf cskg-ont:solvesMetric .

cskg-ont:metricStandardizedBy a owl:ObjectProperty ;
    rdfs:comment "This relation indicates that an instance	 of class Metric was standardized by an instance belonging to one of the following classes { Material, Method, Metric, OtherEntity, Task }. It is designed based on the following predicates extracted by the NLP pipeline: standardize,standardise" ;
    rdfs:domain cskg-ont:Metric ;
    rdfs:range _:N05fff169cc7b47d38569f88b88d8e23f ;
    rdfs:subPropertyOf cskg-ont:standardizedBy ;
    owl:inverseOf cskg-ont:standardizesMetric .

cskg-ont:metricSupportedBy a owl:ObjectProperty ;
    rdfs:comment "This relation indicates that an instance	 of class Metric was supported by an instance belonging to one of the following classes { Method, Task }. It is designed based on the following predicates extracted by the NLP pipeline: help,support,aid,assist,back,underlie,enable,promote,empower,facilitate,foster,facilitate,allow,hold,bear" ;
    rdfs:domain cskg-ont:Metric ;
    rdfs:range _:N858c8dd2315f4e72a9b242c8785d8099 ;
    rdfs:subPropertyOf cskg-ont:supportedBy ;
    owl:inverseOf cskg-ont:supportsMetric .

cskg-ont:metricTransferredBy a owl:ObjectProperty ;
    rdfs:comment "This relation indicates that an instance	 of class Metric was transferred by an instance belonging to one of the following classes { Material, OtherEntity, Task }. It is designed based on the following predicates extracted by the NLP pipeline: deliver,dispatch,shunt,airmail,import,forward,ship,send,transship,transmit,pass,hand,transport,shift,export,express,post,wire,transfer,drive,slip,port,return,convey,handdeliver,mail,answer" ;
    rdfs:domain cskg-ont:Metric ;
    rdfs:range _:N74f6d56423f346dc8b3f8d870cfd2926 ;
    rdfs:subPropertyOf cskg-ont:transferredBy ;
    owl:inverseOf cskg-ont:transfersMetric .

cskg-ont:metricUsedBy a owl:ObjectProperty,
        owl:TransitiveProperty ;
    rdfs:comment "This relation indicates that an instance	 of class Metric was used by an instance belonging to one of the following classes { Method, Metric, OtherEntity, Task }. It is designed by the Used-for relationships extracted by the DyGIE++. It is also designed based on the following predicates extracted by the NLP pipeline: apply,employ,exert,exploit,reuse,use,utilize,utilise,adopt,leverage,rely,access" ;
    rdfs:domain cskg-ont:Metric ;
    rdfs:range _:N729c182289a44f1cb3a3d8590f8f879c ;
    rdfs:subPropertyOf cskg-ont:usedBy ;
    owl:inverseOf cskg-ont:usesMetric .

cskg-ont:metricVisualizedBy a owl:ObjectProperty ;
    rdfs:comment "This relation indicates that an instance	 of class Metric was visualized by an instance belonging to one of the following classes { OtherEntity }. It is designed based on the following predicates extracted by the NLP pipeline: visualize,disclose,reflect" ;
    rdfs:domain cskg-ont:Metric ;
    rdfs:range _:N0efe5afe2d9d443882349b3cf85ecb78 ;
    rdfs:subPropertyOf cskg-ont:visualizedBy ;
    owl:inverseOf cskg-ont:visualizesMetric .

cskg-ont:otherentityAcquiredBy a owl:ObjectProperty,
        owl:TransitiveProperty ;
    rdfs:comment "This relation indicates that an instance	 of class OtherEntity was acquired by an instance belonging to one of the following classes { Method, OtherEntity, Task }. It is designed based on the following predicates extracted by the NLP pipeline: select,accumulate,recoup,source,receive,acquire,regain,retrieve,obtain,accrue,borrow,subselect,inherit,accept,collect,gather,store,attract,get,capture,record,achieve" ;
    rdfs:domain cskg-ont:OtherEntity ;
    rdfs:range _:N1457e755bb5841c594cfec96662ad8f6 ;
    rdfs:subPropertyOf cskg-ont:acquiredBy ;
    owl:inverseOf cskg-ont:acquiresOtherEntity .

cskg-ont:otherentityAdaptedBy a owl:ObjectProperty,
        owl:TransitiveProperty ;
    rdfs:comment "This relation indicates that an instance	 of class OtherEntity was adapted by an instance belonging to one of the following classes { Method, OtherEntity, Task }. It is designed based on the following predicates extracted by the NLP pipeline: readapt,adjust,conform,adapt,gear,readjust,fit,assimilate,accommodate,personalize,customize,specialize,generalize,tailor,refine" ;
    rdfs:domain cskg-ont:OtherEntity ;
    rdfs:range _:Na677c9cf1eec4b199058fa4c7497de9a ;
    rdfs:subPropertyOf cskg-ont:adaptedBy ;
    owl:inverseOf cskg-ont:adaptsOtherEntity .

cskg-ont:otherentityAffectedBy a owl:ObjectProperty ;
    rdfs:comment "This relation indicates that an instance	 of class OtherEntity was affected by an instance belonging to one of the following classes { Material, Method, Metric, OtherEntity, Task }. It is designed based on the following predicates extracted by the NLP pipeline: placate,provoke,engage,console,impair,repulse,shake,discombobulate,threaten,inflame,thrill,satisfy,unsettle,kill,enrapture,outrage,disgruntle,reassure,discompose,interest,alarm,engross,afflict,manipulate,edit,update,increase,replace,modify,fatigue,refresh,cut" ;
    rdfs:domain cskg-ont:OtherEntity ;
    rdfs:range _:Nc42629e2ebbf4afd9c50c37db59f9d93 ;
    rdfs:subPropertyOf cskg-ont:affectedBy ;
    owl:inverseOf cskg-ont:affectsOtherEntity .

cskg-ont:otherentityAnalyzedBy a owl:ObjectProperty,
        owl:TransitiveProperty ;
    rdfs:comment "This relation indicates that an instance	 of class OtherEntity was analyzed by an instance belonging to one of the following classes { Method, Metric, OtherEntity, Task }. It is designed based on the following predicates extracted by the NLP pipeline: analyze,assess,study,try_on,scan,approximate,proofread,inspect,sample,research,check,appraise,analyse,examine,watch,audit,feel_out,go_over,consult,survey,test,assay,try,evaluate,investigate,monitor,regard,peruse,review,try_out,measure,calculate,address,estimate" ;
    rdfs:domain cskg-ont:OtherEntity ;
    rdfs:range _:N4546f13a64de4f31ae43d05836a73544 ;
    rdfs:subPropertyOf cskg-ont:analyzedBy ;
    owl:inverseOf cskg-ont:analyzesOtherEntity .

cskg-ont:otherentityAnnotatedBy a owl:ObjectProperty ;
    rdfs:comment "This relation indicates that an instance	 of class OtherEntity was annotated by an instance belonging to one of the following classes { Method, OtherEntity }. It is designed based on the following predicates extracted by the NLP pipeline: scar,stipple,annotate,stamp,embroider,incise,inscribe,engrave,applique,imprint,paint,reinscribe,mark,sign,tag,label" ;
    rdfs:domain cskg-ont:OtherEntity ;
    rdfs:range _:Na3b25ebacb6c48179625b2df35224994 ;
    rdfs:subPropertyOf cskg-ont:annotatedBy ;
    owl:inverseOf cskg-ont:annotatesOtherEntity .

cskg-ont:otherentityAutomatedBy a owl:ObjectProperty ;
    rdfs:comment "This relation indicates that an instance	 of class OtherEntity was automated by an instance belonging to one of the following classes { Method, OtherEntity }. It is designed based on the following predicates extracted by the NLP pipeline: automate" ;
    rdfs:domain cskg-ont:OtherEntity ;
    rdfs:range _:N0dfe945b3ba44539b8d155270cf03b90 ;
    rdfs:subPropertyOf cskg-ont:automatedBy ;
    owl:inverseOf cskg-ont:automatesOtherEntity .

cskg-ont:otherentityBases a owl:ObjectProperty,
        owl:TransitiveProperty ;
    rdfs:comment "This relation indicates that an instance	 of class OtherEntity was bases by an instance belonging to one of the following classes { Material, Method, Metric, OtherEntity, Task }. It is designed based on the following predicates extracted by the NLP pipeline: base,ground,found,construe,build,establish" ;
    rdfs:domain cskg-ont:OtherEntity ;
    rdfs:range _:Ndc503fa6ad354569a9c6b9e17e337ef8 ;
    rdfs:subPropertyOf cskg-ont:bases ;
    owl:inverseOf cskg-ont:based-onOtherEntity .

cskg-ont:otherentityCausedBy a owl:ObjectProperty ;
    rdfs:comment "This relation indicates that an instance	 of class OtherEntity was caused by an instance belonging to one of the following classes { Material, Method, Metric, OtherEntity, Task }. It is designed based on the following predicates extracted by the NLP pipeline: cause,influence" ;
    rdfs:domain cskg-ont:OtherEntity ;
    rdfs:range _:N834f5e422e534f37a004eeed1df1d02a ;
    rdfs:subPropertyOf cskg-ont:causedBy ;
    owl:inverseOf cskg-ont:causesOtherEntity .

cskg-ont:otherentityClassifiedBy a owl:ObjectProperty ;
    rdfs:comment "This relation indicates that an instance	 of class OtherEntity was classified by an instance belonging to one of the following classes { Method, Metric, OtherEntity }. It is designed based on the following predicates extracted by the NLP pipeline: regroup,bracket,categorize,recode,chunk,code,separate,group,sort,sort_out,catalogue,classify,class,number,seed,reclassify,grade" ;
    rdfs:domain cskg-ont:OtherEntity ;
    rdfs:range _:N0b7d5a96f896460586a5c3412f211a2f ;
    rdfs:subPropertyOf cskg-ont:classifiedBy ;
    owl:inverseOf cskg-ont:classifiesOtherEntity .

cskg-ont:otherentityContributedBy a owl:ObjectProperty ;
    rdfs:comment "This relation indicates that an instance	 of class OtherEntity was contributed by an instance belonging to one of the following classes { Method, Metric, OtherEntity, Task }. It is designed based on the following predicates extracted by the NLP pipeline: abnegate,gift,pass_out,turn-over,restore,turn-in,give-out,disburse,give-away,proffer,distribute,remit,transfer,extend,shell_out,give-up,hand_out,refer,disseminate,contribute" ;
    rdfs:domain cskg-ont:OtherEntity ;
    rdfs:range _:N69404871f6734e52a230c04a387f8ba5 ;
    rdfs:subPropertyOf cskg-ont:contributedBy ;
    owl:inverseOf cskg-ont:contributes-toOtherEntity .

cskg-ont:otherentityDiscussedBy a owl:ObjectProperty ;
    rdfs:comment "This relation indicates that an instance	 of class OtherEntity was discussed by an instance belonging to one of the following classes { Task }. It is designed based on the following predicates extracted by the NLP pipeline: debate,discuss,chatter,confer,converse,argue,discus" ;
    rdfs:domain cskg-ont:OtherEntity ;
    rdfs:range _:N500da0682b05415fbc855afa0ad3b3de ;
    rdfs:subPropertyOf cskg-ont:discussedBy ;
    owl:inverseOf cskg-ont:discussesOtherEntity .

cskg-ont:otherentityExecutedBy a owl:ObjectProperty,
        owl:TransitiveProperty ;
    rdfs:comment "This relation indicates that an instance	 of class OtherEntity was executed by an instance belonging to one of the following classes { Method, Metric, OtherEntity, Task }. It is designed based on the following predicates extracted by the NLP pipeline: perform,execute,operate,run,simulate,play,work,train,action" ;
    rdfs:domain cskg-ont:OtherEntity ;
    rdfs:range _:Ne749f6d04ff04b2cbee667ec125f6efb ;
    rdfs:subPropertyOf cskg-ont:executedBy ;
    owl:inverseOf cskg-ont:executesOtherEntity .

cskg-ont:otherentityExtractedBy a owl:ObjectProperty,
        owl:TransitiveProperty ;
    rdfs:comment "This relation indicates that an instance	 of class OtherEntity was extracted by an instance belonging to one of the following classes { Material, Method, OtherEntity, Task }. It is designed based on the following predicates extracted by the NLP pipeline: extract,mine,induce,infer" ;
    rdfs:domain cskg-ont:OtherEntity ;
    rdfs:range _:N9f08bcc4907946cfb720f28808183be3 ;
    rdfs:subPropertyOf cskg-ont:extractedBy ;
    owl:inverseOf cskg-ont:extractsOtherEntity .

cskg-ont:otherentityGuidedBy a owl:ObjectProperty ;
    rdfs:comment "This relation indicates that an instance	 of class OtherEntity was guided by an instance belonging to one of the following classes { Method, Metric, OtherEntity, Task }. It is designed based on the following predicates extracted by the NLP pipeline: steer,conduct,guide,misdirect,lead,escort,accompany,direct" ;
    rdfs:domain cskg-ont:OtherEntity ;
    rdfs:range _:Naa71c951c7094ee78260e723b1581218 ;
    rdfs:subPropertyOf cskg-ont:guidedBy ;
    owl:inverseOf cskg-ont:guidesOtherEntity .

cskg-ont:otherentityHighlightedBy a owl:ObjectProperty ;
    rdfs:comment "This relation indicates that an instance	 of class OtherEntity was highlighted by an instance belonging to one of the following classes { Material, Method, Metric, OtherEntity, Task }. It is designed based on the following predicates extracted by the NLP pipeline: highlight,emphasize" ;
    rdfs:domain cskg-ont:OtherEntity ;
    rdfs:range _:N546ebba2acea45c98854bbcd3e5e186c ;
    rdfs:subPropertyOf cskg-ont:highlightedBy ;
    owl:inverseOf cskg-ont:highlightsOtherEntity .

cskg-ont:otherentityIdentifiedBy a owl:ObjectProperty ;
    rdfs:comment "This relation indicates that an instance	 of class OtherEntity was identified by an instance belonging to one of the following classes { Method, OtherEntity, Task }. It is designed based on the following predicates extracted by the NLP pipeline: identify,detect,filter,recognize,locate" ;
    rdfs:domain cskg-ont:OtherEntity ;
    rdfs:range _:N32d7ae61b2634b3fa1855613b102b731 ;
    rdfs:subPropertyOf cskg-ont:identifiedBy ;
    owl:inverseOf cskg-ont:identifiesOtherEntity .

cskg-ont:otherentityImprovedBy a owl:ObjectProperty ;
    rdfs:comment "This relation indicates that an instance	 of class OtherEntity was improved by an instance belonging to one of the following classes { Method, Metric, OtherEntity, Task }. It is designed based on the following predicates extracted by the NLP pipeline: improve,evolve,grow,enrich,expand,augment,raise,enhance,advance,gain,optimize" ;
    rdfs:domain cskg-ont:OtherEntity ;
    rdfs:range _:N5b30fa28b8f649bc95dba7dbc8229030 ;
    rdfs:subPropertyOf cskg-ont:improvedBy ;
    owl:inverseOf cskg-ont:improvesOtherEntity .

cskg-ont:otherentityIncludedBy a owl:ObjectProperty,
        owl:TransitiveProperty ;
    rdfs:comment "This relation indicates that an instance	 of class OtherEntity was included by an instance belonging to one of the following classes { Material, Method, OtherEntity, Task }. It is designed by the Feature-of and Part-of relationships extracted by the DyGIE++. It is also designed based on the following predicates extracted by the NLP pipeline: 'relate,include,involve,engage,enroll,embed,contain,comprise,carry,cover,consider,share,mount,have,equip,install" ;
    rdfs:domain cskg-ont:OtherEntity ;
    rdfs:range _:N9c7a820d81f24625baa100d6ee6bbd5e ;
    rdfs:subPropertyOf cskg-ont:includedBy ;
    owl:inverseOf cskg-ont:includesOtherEntity .

cskg-ont:otherentityInteracts-With a owl:ObjectProperty ;
    rdfs:comment "This relation indicates that an instance	 of class OtherEntity was interacts-with by an instance belonging to one of the following classes { Material, Method, Metric, OtherEntity, Task }. It is designed based on the following predicates extracted by the NLP pipeline: renegotiate,compromise,agree,debate,interact,collaborate,disagree,communicate,haggle,interlink,participate" ;
    rdfs:domain cskg-ont:OtherEntity ;
    rdfs:range _:N0c6045d04e2d4fb698e46d314ee9ca52 ;
    rdfs:subPropertyOf cskg-ont:interacts-with ;
    owl:inverseOf cskg-ont:interacts-withOtherEntity .

cskg-ont:otherentityLackedof a owl:ObjectProperty ;
    rdfs:comment "This relation indicates that an instance	 of class OtherEntity was lackedof by an instance belonging to one of the following classes { Material, Method, Metric, OtherEntity, Task }. It is designed based on the following predicates extracted by the NLP pipeline: lack" ;
    rdfs:domain cskg-ont:OtherEntity ;
    rdfs:range _:N5c7e8edce3d54f2e84a531e2b82c0fb4 ;
    rdfs:subPropertyOf cskg-ont:lackedOf ;
    owl:inverseOf cskg-ont:lacksOtherEntity .

cskg-ont:otherentityLearnedBy a owl:ObjectProperty ;
    rdfs:comment "This relation indicates that an instance	 of class OtherEntity was learned by an instance belonging to one of the following classes { Material, Method, OtherEntity, Task }. It is designed based on the following predicates extracted by the NLP pipeline: memorize,glean,learn,study,absorb,assimilate,cram,relearn,read" ;
    rdfs:domain cskg-ont:OtherEntity ;
    rdfs:range _:N266241773fb747198e8cee8f7c80f0ce ;
    rdfs:subPropertyOf cskg-ont:learnedBy ;
    owl:inverseOf cskg-ont:learnsOtherEntity .

cskg-ont:otherentityLimitedBy a owl:ObjectProperty ;
    rdfs:comment "This relation indicates that an instance	 of class OtherEntity was limited by an instance belonging to one of the following classes { Material, Method, Metric, OtherEntity, Task }. It is designed based on the following predicates extracted by the NLP pipeline: reduce,limit,confine,restrain,constrain,restrict,prevent" ;
    rdfs:domain cskg-ont:OtherEntity ;
    rdfs:range _:N041d55ebb2344a4c821fed0b93a96c07 ;
    rdfs:subPropertyOf cskg-ont:limitedBy ;
    owl:inverseOf cskg-ont:limitsOtherEntity .

cskg-ont:otherentityLinkedBy a owl:ObjectProperty,
        owl:TransitiveProperty ;
    rdfs:comment "This relation indicates that an instance	 of class OtherEntity was linked by an instance belonging to one of the following classes { Method, OtherEntity, Task }. It is designed based on the following predicates extracted by the NLP pipeline: fasten,strap,hook,lasso,leash,reeve,peg,rope,seal,clamp,latch,chain,band,trammel,shackle,clasp,knot,button,lock,moor,buckle,yoke,manacle,screw,link,string,pin,tether,paste,anchor,bond,wire,connect" ;
    rdfs:domain cskg-ont:OtherEntity ;
    rdfs:range _:Naca3ac89fa7b4a57ae86bcc28519a296 ;
    rdfs:subPropertyOf cskg-ont:linkedBy ;
    owl:inverseOf cskg-ont:linksOtherEntity .

cskg-ont:otherentityManagedBy a owl:ObjectProperty,
        owl:TransitiveProperty ;
    rdfs:comment "This relation indicates that an instance	 of class OtherEntity was managed by an instance belonging to one of the following classes { Method, Task }. It is designed based on the following predicates extracted by the NLP pipeline: look_out,wait_on,look_after,care,manage,maintain,preserve,keep,handle,treat,deal,configure" ;
    rdfs:domain cskg-ont:OtherEntity ;
    rdfs:range _:N3c0397721de747b089088a59bba638b3 ;
    rdfs:subPropertyOf cskg-ont:managedBy ;
    owl:inverseOf cskg-ont:managesOtherEntity .

cskg-ont:otherentityOutperformedBy a owl:ObjectProperty,
        owl:TransitiveProperty ;
    rdfs:comment "This relation indicates that an instance	 of class OtherEntity was outperformed by an instance belonging to one of the following classes { Material, Method, Metric, OtherEntity, Task }. It is designed based on the following predicates extracted by the NLP pipeline: outperform" ;
    rdfs:domain cskg-ont:OtherEntity ;
    rdfs:range _:N2a9dfb5c771247ff9bbfac03e665e224 ;
    rdfs:subPropertyOf cskg-ont:outperformedBy ;
    owl:inverseOf cskg-ont:outperformsOtherEntity .

cskg-ont:otherentityPredictedBy a owl:ObjectProperty ;
    rdfs:comment "This relation indicates that an instance	 of class OtherEntity was predicted by an instance belonging to one of the following classes { Material, Method, OtherEntity, Task }. It is designed based on the following predicates extracted by the NLP pipeline: denote,corroborate,indicate,imply,predict,anticipate,forebode,say,expose,prognosticate,explain,forecast" ;
    rdfs:domain cskg-ont:OtherEntity ;
    rdfs:range _:N0e4608619db046fd8645d33a9c58429f ;
    rdfs:subPropertyOf cskg-ont:predictedBy ;
    owl:inverseOf cskg-ont:predictsOtherEntity .

cskg-ont:otherentityProcessedBy a owl:ObjectProperty ;
    rdfs:comment "This relation indicates that an instance	 of class OtherEntity was processed by an instance belonging to one of the following classes { Method, OtherEntity, Task }. It is designed based on the following predicates extracted by the NLP pipeline: process,proces" ;
    rdfs:domain cskg-ont:OtherEntity ;
    rdfs:range _:Nf6875e68b52748d698406e26489862c3 ;
    rdfs:subPropertyOf cskg-ont:processedBy ;
    owl:inverseOf cskg-ont:processesOtherEntity .

cskg-ont:otherentityProducedBy a owl:ObjectProperty,
        owl:TransitiveProperty ;
    rdfs:comment "This relation indicates that an instance	 of class OtherEntity was produced by an instance belonging to one of the following classes { Method, OtherEntity, Task }. It is designed based on the following predicates extracted by the NLP pipeline: author,coin,compose,compute,conoct,construct,contrive,cowrite,create,derive,draft,fabricate,form,formulate,invent,manufacture,model,organize,produce,rebuild,recreate,style,synthesize,write,generate,design,develop,implement,deploy,make,do" ;
    rdfs:domain cskg-ont:OtherEntity ;
    rdfs:range _:Nd728889fde2d409ea84799397b8adbbb ;
    rdfs:subPropertyOf cskg-ont:producedBy ;
    owl:inverseOf cskg-ont:producesOtherEntity .

cskg-ont:otherentityProposedBy a owl:ObjectProperty ;
    rdfs:comment "This relation indicates that an instance	 of class OtherEntity was proposed by an instance belonging to one of the following classes { Method, OtherEntity, Task }. It is designed based on the following predicates extracted by the NLP pipeline: propose,report,say,state,recommend,suggest,hint,introduce,outline,promise" ;
    rdfs:domain cskg-ont:OtherEntity ;
    rdfs:range _:N6c9bffc4afb84f59b54c806a405408b6 ;
    rdfs:subPropertyOf cskg-ont:proposedBy ;
    owl:inverseOf cskg-ont:proposesOtherEntity .

cskg-ont:otherentityProvidedBy a owl:ObjectProperty,
        owl:TransitiveProperty ;
    rdfs:comment "This relation indicates that an instance	 of class OtherEntity was provided by an instance belonging to one of the following classes { Method, Metric, OtherEntity, Task }. It is designed based on the following predicates extracted by the NLP pipeline: present,furnish,resupply,serve,supply,provide,yield,give,add,assign" ;
    rdfs:domain cskg-ont:OtherEntity ;
    rdfs:range _:Nf911d4c28edc48f1bb6ec24f81c0a277 ;
    rdfs:subPropertyOf cskg-ont:providedBy ;
    owl:inverseOf cskg-ont:providesOtherEntity .

cskg-ont:otherentityQueriedBy a owl:ObjectProperty ;
    rdfs:comment "This relation indicates that an instance	 of class OtherEntity was queried by an instance belonging to one of the following classes { Method, Task }. It is designed based on the following predicates extracted by the NLP pipeline: query" ;
    rdfs:domain cskg-ont:OtherEntity ;
    rdfs:range _:N643c09c87dac4699a09b44bac23ba7db ;
    rdfs:subPropertyOf cskg-ont:queriedBy ;
    owl:inverseOf cskg-ont:queriesOtherEntity .

cskg-ont:otherentitySolvedBy a owl:ObjectProperty ;
    rdfs:comment "This relation indicates that an instance	 of class OtherEntity was solved by an instance belonging to one of the following classes { Material, Method, Metric, OtherEntity, Task }. It is designed based on the following predicates extracted by the NLP pipeline: find,determine,see,rationalize,guess,deduce,solve,discover,pick_up,ascertain,realize,relearn,ascertain,realize,relearn,fix" ;
    rdfs:domain cskg-ont:OtherEntity ;
    rdfs:range _:N1d89778f5eee4becb135ae54ea6ac098 ;
    rdfs:subPropertyOf cskg-ont:solvedBy ;
    owl:inverseOf cskg-ont:solvesOtherEntity .

cskg-ont:otherentityStandardizedBy a owl:ObjectProperty ;
    rdfs:comment "This relation indicates that an instance	 of class OtherEntity was standardized by an instance belonging to one of the following classes { Material, Method, Metric, OtherEntity, Task }. It is designed based on the following predicates extracted by the NLP pipeline: standardize,standardise" ;
    rdfs:domain cskg-ont:OtherEntity ;
    rdfs:range _:N5d064c0a456041dea42da6099d2c09a5 ;
    rdfs:subPropertyOf cskg-ont:standardizedBy ;
    owl:inverseOf cskg-ont:standardizesOtherEntity .

cskg-ont:otherentitySupportedBy a owl:ObjectProperty ;
    rdfs:comment "This relation indicates that an instance	 of class OtherEntity was supported by an instance belonging to one of the following classes { Material, Method, Metric, OtherEntity, Task }. It is designed based on the following predicates extracted by the NLP pipeline: help,support,aid,assist,back,underlie,enable,promote,empower,facilitate,foster,facilitate,allow,hold,bear" ;
    rdfs:domain cskg-ont:OtherEntity ;
    rdfs:range _:N77f97df3763b4e5380481a85960e8fd2 ;
    rdfs:subPropertyOf cskg-ont:supportedBy ;
    owl:inverseOf cskg-ont:supportsOtherEntity .

cskg-ont:otherentityTransferredBy a owl:ObjectProperty ;
    rdfs:comment "This relation indicates that an instance	 of class OtherEntity was transferred by an instance belonging to one of the following classes { Material, Method, Metric, OtherEntity, Task }. It is designed based on the following predicates extracted by the NLP pipeline: deliver,dispatch,shunt,airmail,import,forward,ship,send,transship,transmit,pass,hand,transport,shift,export,express,post,wire,transfer,drive,slip,port,return,convey,handdeliver,mail,answer" ;
    rdfs:domain cskg-ont:OtherEntity ;
    rdfs:range _:N8ed691a078b54c38be50433903e66463 ;
    rdfs:subPropertyOf cskg-ont:transferredBy ;
    owl:inverseOf cskg-ont:transfersOtherEntity .

cskg-ont:otherentityUsedBy a owl:ObjectProperty,
        owl:TransitiveProperty ;
    rdfs:comment "This relation indicates that an instance	 of class OtherEntity was used by an instance belonging to one of the following classes { Method, Metric, OtherEntity, Task }. It is designed by the Used-for relationships extracted by the DyGIE++. It is also designed based on the following predicates extracted by the NLP pipeline: apply,employ,exert,exploit,reuse,use,utilize,utilise,adopt,leverage,rely,access" ;
    rdfs:domain cskg-ont:OtherEntity ;
    rdfs:range _:N849ae1a9a93447adb97c0b77a0f8eb8e ;
    rdfs:subPropertyOf cskg-ont:usedBy ;
    owl:inverseOf cskg-ont:usesOtherEntity .

cskg-ont:otherentityVisualizedBy a owl:ObjectProperty ;
    rdfs:comment "This relation indicates that an instance	 of class OtherEntity was visualized by an instance belonging to one of the following classes { Material, Method, Metric, OtherEntity }. It is designed based on the following predicates extracted by the NLP pipeline: visualize,disclose,reflect" ;
    rdfs:domain cskg-ont:OtherEntity ;
    rdfs:range _:N75eaaf8f7d944145995cee9c2dc4b1f4 ;
    rdfs:subPropertyOf cskg-ont:visualizedBy ;
    owl:inverseOf cskg-ont:visualizesOtherEntity .

cskg-ont:outperformsMaterial a owl:ObjectProperty,
        owl:TransitiveProperty ;
    rdfs:comment "This relation indicates that an instance belonging to one class in { Material, Method, Metric, OtherEntity } outperforms an instance of  Material. It is designed based on the following predicates extracted by the NLP pipeline: outperform" ;
    rdfs:domain _:N8e228a8aba9841f88141006ed0d039c8 ;
    rdfs:range cskg-ont:Material ;
    rdfs:subPropertyOf cskg-ont:outperforms ;
    owl:inverseOf cskg-ont:materialOutperformedBy .

cskg-ont:outperformsMethod a owl:ObjectProperty,
        owl:TransitiveProperty ;
    rdfs:comment "This relation indicates that an instance belonging to one class in { Material, Method, Metric, OtherEntity, Task } outperforms an instance of  Method. It is designed based on the following predicates extracted by the NLP pipeline: outperform" ;
    rdfs:domain _:N8018a76176324d59bbe6d65bbdb0c9e4 ;
    rdfs:range cskg-ont:Method ;
    rdfs:subPropertyOf cskg-ont:outperforms ;
    owl:inverseOf cskg-ont:methodOutperformedBy .

cskg-ont:outperformsMetric a owl:ObjectProperty,
        owl:TransitiveProperty ;
    rdfs:comment "This relation indicates that an instance belonging to one class in { Metric } outperforms an instance of  Metric. It is designed based on the following predicates extracted by the NLP pipeline: outperform" ;
    rdfs:domain _:Nb4d555962720432b9706eed1174a7f35 ;
    rdfs:range cskg-ont:Metric ;
    rdfs:subPropertyOf cskg-ont:outperforms ;
    owl:inverseOf cskg-ont:metricOutperformedBy .

cskg-ont:outperformsOtherEntity a owl:ObjectProperty,
        owl:TransitiveProperty ;
    rdfs:comment "This relation indicates that an instance belonging to one class in { Material, Method, Metric, OtherEntity, Task } outperforms an instance of  OtherEntity. It is designed based on the following predicates extracted by the NLP pipeline: outperform" ;
    rdfs:domain _:N2a9dfb5c771247ff9bbfac03e665e224 ;
    rdfs:range cskg-ont:OtherEntity ;
    rdfs:subPropertyOf cskg-ont:outperforms ;
    owl:inverseOf cskg-ont:otherentityOutperformedBy .

cskg-ont:outperformsTask a owl:ObjectProperty,
        owl:TransitiveProperty ;
    rdfs:comment "This relation indicates that an instance belonging to one class in { Method, Task } outperforms an instance of  Task. It is designed based on the following predicates extracted by the NLP pipeline: outperform" ;
    rdfs:domain _:Ne820e56ea37d4cc8b0b1e18266d61899 ;
    rdfs:range cskg-ont:Task ;
    rdfs:subPropertyOf cskg-ont:outperforms ;
    owl:inverseOf cskg-ont:taskOutperformedBy .

cskg-ont:predictsMaterial a owl:ObjectProperty ;
    rdfs:comment "This relation indicates that an instance belonging to one class in { Material, Method, OtherEntity, Task } predicts an instance of  Material. It is designed based on the following predicates extracted by the NLP pipeline: denote,corroborate,indicate,imply,predict,anticipate,forebode,say,expose,prognosticate,explain,forecast" ;
    rdfs:domain _:N2a981ddad09442f3bbf2168fd92d119a ;
    rdfs:range cskg-ont:Material ;
    rdfs:subPropertyOf cskg-ont:predicts ;
    owl:inverseOf cskg-ont:materialPredictedBy .

cskg-ont:predictsMethod a owl:ObjectProperty ;
    rdfs:comment "This relation indicates that an instance belonging to one class in { Material, Method, OtherEntity, Task } predicts an instance of  Method. It is designed based on the following predicates extracted by the NLP pipeline: denote,corroborate,indicate,imply,predict,anticipate,forebode,say,expose,prognosticate,explain,forecast" ;
    rdfs:domain _:N1a90f39251084963a0e43a269d1c9d13 ;
    rdfs:range cskg-ont:Method ;
    rdfs:subPropertyOf cskg-ont:predicts ;
    owl:inverseOf cskg-ont:methodPredictedBy .

cskg-ont:predictsMetric a owl:ObjectProperty ;
    rdfs:comment "This relation indicates that an instance belonging to one class in { Method, Task } predicts an instance of  Metric. It is designed based on the following predicates extracted by the NLP pipeline: denote,corroborate,indicate,imply,predict,anticipate,forebode,say,expose,prognosticate,explain,forecast" ;
    rdfs:domain _:N0bd7083d9bbc422f92e266e47b20363d ;
    rdfs:range cskg-ont:Metric ;
    rdfs:subPropertyOf cskg-ont:predicts ;
    owl:inverseOf cskg-ont:metricPredictedBy .

cskg-ont:predictsOtherEntity a owl:ObjectProperty ;
    rdfs:comment "This relation indicates that an instance belonging to one class in { Material, Method, OtherEntity, Task } predicts an instance of  OtherEntity. It is designed based on the following predicates extracted by the NLP pipeline: denote,corroborate,indicate,imply,predict,anticipate,forebode,say,expose,prognosticate,explain,forecast" ;
    rdfs:domain _:N0e4608619db046fd8645d33a9c58429f ;
    rdfs:range cskg-ont:OtherEntity ;
    rdfs:subPropertyOf cskg-ont:predicts ;
    owl:inverseOf cskg-ont:otherentityPredictedBy .

cskg-ont:predictsTask a owl:ObjectProperty ;
    rdfs:comment "This relation indicates that an instance belonging to one class in { Material, Method, OtherEntity, Task } predicts an instance of  Task. It is designed based on the following predicates extracted by the NLP pipeline: denote,corroborate,indicate,imply,predict,anticipate,forebode,say,expose,prognosticate,explain,forecast" ;
    rdfs:domain _:N0b422da05d3c4d2293fa30de0b98d6e1 ;
    rdfs:range cskg-ont:Task ;
    rdfs:subPropertyOf cskg-ont:predicts ;
    owl:inverseOf cskg-ont:taskPredictedBy .

cskg-ont:processesMaterial a owl:ObjectProperty ;
    rdfs:comment "This relation indicates that an instance belonging to one class in { Method, OtherEntity, Task } processes an instance of  Material. It is designed based on the following predicates extracted by the NLP pipeline: process,proces" ;
    rdfs:domain _:N7326ea397df347f1ab490fea703779f6 ;
    rdfs:range cskg-ont:Material ;
    rdfs:subPropertyOf cskg-ont:processes ;
    owl:inverseOf cskg-ont:materialProcessedBy .

cskg-ont:processesMethod a owl:ObjectProperty ;
    rdfs:comment "This relation indicates that an instance belonging to one class in { Method, Task } processes an instance of  Method. It is designed based on the following predicates extracted by the NLP pipeline: process,proces" ;
    rdfs:domain _:N955dfd3e9c954207b4ffe0c9f2f9daf2 ;
    rdfs:range cskg-ont:Method ;
    rdfs:subPropertyOf cskg-ont:processes ;
    owl:inverseOf cskg-ont:methodProcessedBy .

cskg-ont:processesMetric a owl:ObjectProperty ;
    rdfs:comment "This relation indicates that an instance belonging to one class in { Method, Task } processes an instance of  Metric. It is designed based on the following predicates extracted by the NLP pipeline: process,proces" ;
    rdfs:domain _:N988dc0f7e5f6414780c74ecda82f8bcb ;
    rdfs:range cskg-ont:Metric ;
    rdfs:subPropertyOf cskg-ont:processes ;
    owl:inverseOf cskg-ont:metricProcessedBy .

cskg-ont:processesOtherEntity a owl:ObjectProperty ;
    rdfs:comment "This relation indicates that an instance belonging to one class in { Method, OtherEntity, Task } processes an instance of  OtherEntity. It is designed based on the following predicates extracted by the NLP pipeline: process,proces" ;
    rdfs:domain _:Nf6875e68b52748d698406e26489862c3 ;
    rdfs:range cskg-ont:OtherEntity ;
    rdfs:subPropertyOf cskg-ont:processes ;
    owl:inverseOf cskg-ont:otherentityProcessedBy .

cskg-ont:processesTask a owl:ObjectProperty ;
    rdfs:comment "This relation indicates that an instance belonging to one class in { Method, OtherEntity, Task } processes an instance of  Task. It is designed based on the following predicates extracted by the NLP pipeline: process,proces" ;
    rdfs:domain _:N66dc74126f5c44409fda43db68f1be57 ;
    rdfs:range cskg-ont:Task ;
    rdfs:subPropertyOf cskg-ont:processes ;
    owl:inverseOf cskg-ont:taskProcessedBy .

cskg-ont:producesMaterial a owl:ObjectProperty ;
    rdfs:comment "This relation indicates that an instance belonging to one class in { Method, OtherEntity, Task } produces an instance of  Material. It is designed based on the following predicates extracted by the NLP pipeline: author,coin,compose,compute,conoct,construct,contrive,cowrite,create,derive,draft,fabricate,form,formulate,invent,manufacture,model,organize,produce,rebuild,recreate,style,synthesize,write,generate,design,develop,implement,deploy,make,do" ;
    rdfs:domain _:Na8f5f43e5b904317a7bbba3fbb34a41c ;
    rdfs:range cskg-ont:Material ;
    rdfs:subPropertyOf cskg-ont:produces ;
    owl:inverseOf cskg-ont:materialProducedBy .

cskg-ont:producesMethod a owl:ObjectProperty,
        owl:TransitiveProperty ;
    rdfs:comment "This relation indicates that an instance belonging to one class in { Method, OtherEntity, Task } produces an instance of  Method. It is designed based on the following predicates extracted by the NLP pipeline: author,coin,compose,compute,conoct,construct,contrive,cowrite,create,derive,draft,fabricate,form,formulate,invent,manufacture,model,organize,produce,rebuild,recreate,style,synthesize,write,generate,design,develop,implement,deploy,make,do" ;
    rdfs:domain _:Nd5ef3a6440db43dfb488042b013f990a ;
    rdfs:range cskg-ont:Method ;
    rdfs:subPropertyOf cskg-ont:produces ;
    owl:inverseOf cskg-ont:methodProducedBy .

cskg-ont:producesMetric a owl:ObjectProperty ;
    rdfs:comment "This relation indicates that an instance belonging to one class in { Method, OtherEntity, Task } produces an instance of  Metric. It is designed based on the following predicates extracted by the NLP pipeline: author,coin,compose,compute,conoct,construct,contrive,cowrite,create,derive,draft,fabricate,form,formulate,invent,manufacture,model,organize,produce,rebuild,recreate,style,synthesize,write,generate,design,develop,implement,deploy,make,do" ;
    rdfs:domain _:Ne16adafdc323491d984944c180663627 ;
    rdfs:range cskg-ont:Metric ;
    rdfs:subPropertyOf cskg-ont:produces ;
    owl:inverseOf cskg-ont:metricProducedBy .

cskg-ont:producesOtherEntity a owl:ObjectProperty,
        owl:TransitiveProperty ;
    rdfs:comment "This relation indicates that an instance belonging to one class in { Method, OtherEntity, Task } produces an instance of  OtherEntity. It is designed based on the following predicates extracted by the NLP pipeline: author,coin,compose,compute,conoct,construct,contrive,cowrite,create,derive,draft,fabricate,form,formulate,invent,manufacture,model,organize,produce,rebuild,recreate,style,synthesize,write,generate,design,develop,implement,deploy,make,do" ;
    rdfs:domain _:Nd728889fde2d409ea84799397b8adbbb ;
    rdfs:range cskg-ont:OtherEntity ;
    rdfs:subPropertyOf cskg-ont:produces ;
    owl:inverseOf cskg-ont:otherentityProducedBy .

cskg-ont:producesTask a owl:ObjectProperty,
        owl:TransitiveProperty ;
    rdfs:comment "This relation indicates that an instance belonging to one class in { Method, Task } produces an instance of  Task. It is designed based on the following predicates extracted by the NLP pipeline: author,coin,compose,compute,conoct,construct,contrive,cowrite,create,derive,draft,fabricate,form,formulate,invent,manufacture,model,organize,produce,rebuild,recreate,style,synthesize,write,generate,design,develop,implement,deploy,make,do" ;
    rdfs:domain _:N11e01c48cf0b41f8a07ab64da28f89b3 ;
    rdfs:range cskg-ont:Task ;
    rdfs:subPropertyOf cskg-ont:produces ;
    owl:inverseOf cskg-ont:taskProducedBy .

cskg-ont:proposesMaterial a owl:ObjectProperty ;
    rdfs:comment "This relation indicates that an instance belonging to one class in { Method, OtherEntity, Task } proposes an instance of  Material. It is designed based on the following predicates extracted by the NLP pipeline: propose,report,say,state,recommend,suggest,hint,introduce,outline,promise" ;
    rdfs:domain _:Neada5e5673584d3b9a7f574d65dadc46 ;
    rdfs:range cskg-ont:Material ;
    rdfs:subPropertyOf cskg-ont:proposes ;
    owl:inverseOf cskg-ont:materialProposedBy .

cskg-ont:proposesMethod a owl:ObjectProperty ;
    rdfs:comment "This relation indicates that an instance belonging to one class in { Method, OtherEntity, Task } proposes an instance of  Method. It is designed based on the following predicates extracted by the NLP pipeline: propose,report,say,state,recommend,suggest,hint,introduce,outline,promise" ;
    rdfs:domain _:Ndfef39aead1d4430a1744fb242c62a0d ;
    rdfs:range cskg-ont:Method ;
    rdfs:subPropertyOf cskg-ont:proposes ;
    owl:inverseOf cskg-ont:methodProposedBy .

cskg-ont:proposesMetric a owl:ObjectProperty ;
    rdfs:comment "This relation indicates that an instance belonging to one class in { Method, OtherEntity, Task } proposes an instance of  Metric. It is designed based on the following predicates extracted by the NLP pipeline: propose,report,say,state,recommend,suggest,hint,introduce,outline,promise" ;
    rdfs:domain _:N2af9352be5834a908acd7941b06493e3 ;
    rdfs:range cskg-ont:Metric ;
    rdfs:subPropertyOf cskg-ont:proposes ;
    owl:inverseOf cskg-ont:metricProposedBy .

cskg-ont:proposesOtherEntity a owl:ObjectProperty ;
    rdfs:comment "This relation indicates that an instance belonging to one class in { Method, OtherEntity, Task } proposes an instance of  OtherEntity. It is designed based on the following predicates extracted by the NLP pipeline: propose,report,say,state,recommend,suggest,hint,introduce,outline,promise" ;
    rdfs:domain _:N6c9bffc4afb84f59b54c806a405408b6 ;
    rdfs:range cskg-ont:OtherEntity ;
    rdfs:subPropertyOf cskg-ont:proposes ;
    owl:inverseOf cskg-ont:otherentityProposedBy .

cskg-ont:proposesTask a owl:ObjectProperty ;
    rdfs:comment "This relation indicates that an instance belonging to one class in { Method, OtherEntity, Task } proposes an instance of  Task. It is designed based on the following predicates extracted by the NLP pipeline: propose,report,say,state,recommend,suggest,hint,introduce,outline,promise" ;
    rdfs:domain _:N67712a1fb05f4cd4bd69c7bc8c6b53fb ;
    rdfs:range cskg-ont:Task ;
    rdfs:subPropertyOf cskg-ont:proposes ;
    owl:inverseOf cskg-ont:taskProposedBy .

cskg-ont:providesMaterial a owl:ObjectProperty ;
    rdfs:comment "This relation indicates that an instance belonging to one class in { Method, OtherEntity, Task } provides an instance of  Material. It is designed based on the following predicates extracted by the NLP pipeline: present,furnish,resupply,serve,supply,provide,yield,give,add,assign" ;
    rdfs:domain _:N7b68838e3777448ab5f7047aa5a6120f ;
    rdfs:range cskg-ont:Material ;
    rdfs:subPropertyOf cskg-ont:provides ;
    owl:inverseOf cskg-ont:materialProvidedBy .

cskg-ont:providesMethod a owl:ObjectProperty,
        owl:TransitiveProperty ;
    rdfs:comment "This relation indicates that an instance belonging to one class in { Method, OtherEntity, Task } provides an instance of  Method. It is designed based on the following predicates extracted by the NLP pipeline: present,furnish,resupply,serve,supply,provide,yield,give,add,assign" ;
    rdfs:domain _:N7ae089cecafe4d34ae8b2bb2964db95b ;
    rdfs:range cskg-ont:Method ;
    rdfs:subPropertyOf cskg-ont:provides ;
    owl:inverseOf cskg-ont:methodProvidedBy .

cskg-ont:providesMetric a owl:ObjectProperty ;
    rdfs:comment "This relation indicates that an instance belonging to one class in { Method, OtherEntity, Task } provides an instance of  Metric. It is designed based on the following predicates extracted by the NLP pipeline: present,furnish,resupply,serve,supply,provide,yield,give,add,assign" ;
    rdfs:domain _:N497f9c02321348b5a5460e2adbe2e14d ;
    rdfs:range cskg-ont:Metric ;
    rdfs:subPropertyOf cskg-ont:provides ;
    owl:inverseOf cskg-ont:metricProvidedBy .

cskg-ont:providesOtherEntity a owl:ObjectProperty,
        owl:TransitiveProperty ;
    rdfs:comment "This relation indicates that an instance belonging to one class in { Method, Metric, OtherEntity, Task } provides an instance of  OtherEntity. It is designed based on the following predicates extracted by the NLP pipeline: present,furnish,resupply,serve,supply,provide,yield,give,add,assign" ;
    rdfs:domain _:Nf911d4c28edc48f1bb6ec24f81c0a277 ;
    rdfs:range cskg-ont:OtherEntity ;
    rdfs:subPropertyOf cskg-ont:provides ;
    owl:inverseOf cskg-ont:otherentityProvidedBy .

cskg-ont:providesTask a owl:ObjectProperty,
        owl:TransitiveProperty ;
    rdfs:comment "This relation indicates that an instance belonging to one class in { Method, Task } provides an instance of  Task. It is designed based on the following predicates extracted by the NLP pipeline: present,furnish,resupply,serve,supply,provide,yield,give,add,assign" ;
    rdfs:domain _:N238d5b5ca3454fa5bc4c9fa1a192c826 ;
    rdfs:range cskg-ont:Task ;
    rdfs:subPropertyOf cskg-ont:provides ;
    owl:inverseOf cskg-ont:taskProvidedBy .

cskg-ont:queriesMaterial a owl:ObjectProperty ;
    rdfs:comment "This relation indicates that an instance belonging to one class in { Method, Task } queries an instance of  Material. It is designed based on the following predicates extracted by the NLP pipeline: query" ;
    rdfs:domain _:N1180ea8f3dc54e0d8b6efb545a5fd9fe ;
    rdfs:range cskg-ont:Material ;
    rdfs:subPropertyOf cskg-ont:queries ;
    owl:inverseOf cskg-ont:materialQueriedBy .

cskg-ont:queriesOtherEntity a owl:ObjectProperty ;
    rdfs:comment "This relation indicates that an instance belonging to one class in { Method, Task } queries an instance of  OtherEntity. It is designed based on the following predicates extracted by the NLP pipeline: query" ;
    rdfs:domain _:N643c09c87dac4699a09b44bac23ba7db ;
    rdfs:range cskg-ont:OtherEntity ;
    rdfs:subPropertyOf cskg-ont:queries ;
    owl:inverseOf cskg-ont:otherentityQueriedBy .

cskg-ont:solvesMaterial a owl:ObjectProperty ;
    rdfs:comment "This relation indicates that an instance belonging to one class in { Material, Method, Metric, OtherEntity, Task } solves an instance of  Material. It is designed based on the following predicates extracted by the NLP pipeline: find,determine,see,rationalize,guess,deduce,solve,discover,pick_up,ascertain,realize,relearn,ascertain,realize,relearn,fix" ;
    rdfs:domain _:Nfd15102f89754dcdb6b4cea4fe32762e ;
    rdfs:range cskg-ont:Material ;
    rdfs:subPropertyOf cskg-ont:solves ;
    owl:inverseOf cskg-ont:materialSolvedBy .

cskg-ont:solvesMethod a owl:ObjectProperty ;
    rdfs:comment "This relation indicates that an instance belonging to one class in { Material, Method, Metric, OtherEntity, Task } solves an instance of  Method. It is designed based on the following predicates extracted by the NLP pipeline: find,determine,see,rationalize,guess,deduce,solve,discover,pick_up,ascertain,realize,relearn,ascertain,realize,relearn,fix" ;
    rdfs:domain _:Nf9274a4f2b844ee292c2dc38853f9e4c ;
    rdfs:range cskg-ont:Method ;
    rdfs:subPropertyOf cskg-ont:solves ;
    owl:inverseOf cskg-ont:methodSolvedBy .

cskg-ont:solvesMetric a owl:ObjectProperty ;
    rdfs:comment "This relation indicates that an instance belonging to one class in { Material, Method, Metric, OtherEntity, Task } solves an instance of  Metric. It is designed based on the following predicates extracted by the NLP pipeline: find,determine,see,rationalize,guess,deduce,solve,discover,pick_up,ascertain,realize,relearn,ascertain,realize,relearn,fix" ;
    rdfs:domain _:N49ce4eca3edd4cc78b03a189cc38cd71 ;
    rdfs:range cskg-ont:Metric ;
    rdfs:subPropertyOf cskg-ont:solves ;
    owl:inverseOf cskg-ont:metricSolvedBy .

cskg-ont:solvesOtherEntity a owl:ObjectProperty ;
    rdfs:comment "This relation indicates that an instance belonging to one class in { Material, Method, Metric, OtherEntity, Task } solves an instance of  OtherEntity. It is designed based on the following predicates extracted by the NLP pipeline: find,determine,see,rationalize,guess,deduce,solve,discover,pick_up,ascertain,realize,relearn,ascertain,realize,relearn,fix" ;
    rdfs:domain _:N1d89778f5eee4becb135ae54ea6ac098 ;
    rdfs:range cskg-ont:OtherEntity ;
    rdfs:subPropertyOf cskg-ont:solves ;
    owl:inverseOf cskg-ont:otherentitySolvedBy .

cskg-ont:solvesTask a owl:ObjectProperty ;
    rdfs:comment "This relation indicates that an instance belonging to one class in { Material, Method, Metric, OtherEntity, Task } solves an instance of  Task. It is designed based on the following predicates extracted by the NLP pipeline: find,determine,see,rationalize,guess,deduce,solve,discover,pick_up,ascertain,realize,relearn,ascertain,realize,relearn,fix" ;
    rdfs:domain _:Ne84f44c11bdf4d58a6f9736f48b3ae13 ;
    rdfs:range cskg-ont:Task ;
    rdfs:subPropertyOf cskg-ont:solves ;
    owl:inverseOf cskg-ont:taskSolvedBy .

cskg-ont:standardizesMaterial a owl:ObjectProperty ;
    rdfs:comment "This relation indicates that an instance belonging to one class in { Material, Method, Metric, OtherEntity, Task } standardizes an instance of  Material. It is designed based on the following predicates extracted by the NLP pipeline: standardize,standardise" ;
    rdfs:domain _:Nbc27e6b3f2f34bc39339daacb1b90191 ;
    rdfs:range cskg-ont:Material ;
    rdfs:subPropertyOf cskg-ont:standardizes ;
    owl:inverseOf cskg-ont:materialStandardizedBy .

cskg-ont:standardizesMethod a owl:ObjectProperty ;
    rdfs:comment "This relation indicates that an instance belonging to one class in { Material, Method, Metric, OtherEntity, Task } standardizes an instance of  Method. It is designed based on the following predicates extracted by the NLP pipeline: standardize,standardise" ;
    rdfs:domain _:N924787736fc3410a819e8c65bb11079a ;
    rdfs:range cskg-ont:Method ;
    rdfs:subPropertyOf cskg-ont:standardizes ;
    owl:inverseOf cskg-ont:methodStandardizedBy .

cskg-ont:standardizesMetric a owl:ObjectProperty ;
    rdfs:comment "This relation indicates that an instance belonging to one class in { Material, Method, Metric, OtherEntity, Task } standardizes an instance of  Metric. It is designed based on the following predicates extracted by the NLP pipeline: standardize,standardise" ;
    rdfs:domain _:N05fff169cc7b47d38569f88b88d8e23f ;
    rdfs:range cskg-ont:Metric ;
    rdfs:subPropertyOf cskg-ont:standardizes ;
    owl:inverseOf cskg-ont:metricStandardizedBy .

cskg-ont:standardizesOtherEntity a owl:ObjectProperty ;
    rdfs:comment "This relation indicates that an instance belonging to one class in { Material, Method, Metric, OtherEntity, Task } standardizes an instance of  OtherEntity. It is designed based on the following predicates extracted by the NLP pipeline: standardize,standardise" ;
    rdfs:domain _:N5d064c0a456041dea42da6099d2c09a5 ;
    rdfs:range cskg-ont:OtherEntity ;
    rdfs:subPropertyOf cskg-ont:standardizes ;
    owl:inverseOf cskg-ont:otherentityStandardizedBy .

cskg-ont:standardizesTask a owl:ObjectProperty ;
    rdfs:comment "This relation indicates that an instance belonging to one class in { Material, Method, Metric, OtherEntity, Task } standardizes an instance of  Task. It is designed based on the following predicates extracted by the NLP pipeline: standardize,standardise" ;
    rdfs:domain _:N65a40cf82d8c4baaaa10dd77428da2b4 ;
    rdfs:range cskg-ont:Task ;
    rdfs:subPropertyOf cskg-ont:standardizes ;
    owl:inverseOf cskg-ont:taskStandardizedBy .

cskg-ont:supportsMaterial a owl:ObjectProperty ;
    rdfs:comment "This relation indicates that an instance belonging to one class in { Method, Task } supports an instance of  Material. It is designed based on the following predicates extracted by the NLP pipeline: help,support,aid,assist,back,underlie,enable,promote,empower,facilitate,foster,facilitate,allow,hold,bear" ;
    rdfs:domain _:N15a8080dcfdb43bf8d293acae48153f4 ;
    rdfs:range cskg-ont:Material ;
    rdfs:subPropertyOf cskg-ont:supports ;
    owl:inverseOf cskg-ont:materialSupportedBy .

cskg-ont:supportsMethod a owl:ObjectProperty ;
    rdfs:comment "This relation indicates that an instance belonging to one class in { Material, Method, Metric, OtherEntity, Task } supports an instance of  Method. It is designed based on the following predicates extracted by the NLP pipeline: help,support,aid,assist,back,underlie,enable,promote,empower,facilitate,foster,facilitate,allow,hold,bear" ;
    rdfs:domain _:N2a8dec03baeb4ec8b05703ac02a71e46 ;
    rdfs:range cskg-ont:Method ;
    rdfs:subPropertyOf cskg-ont:supports ;
    owl:inverseOf cskg-ont:methodSupportedBy .

cskg-ont:supportsMetric a owl:ObjectProperty ;
    rdfs:comment "This relation indicates that an instance belonging to one class in { Method, Task } supports an instance of  Metric. It is designed based on the following predicates extracted by the NLP pipeline: help,support,aid,assist,back,underlie,enable,promote,empower,facilitate,foster,facilitate,allow,hold,bear" ;
    rdfs:domain _:N858c8dd2315f4e72a9b242c8785d8099 ;
    rdfs:range cskg-ont:Metric ;
    rdfs:subPropertyOf cskg-ont:supports ;
    owl:inverseOf cskg-ont:metricSupportedBy .

cskg-ont:supportsOtherEntity a owl:ObjectProperty ;
    rdfs:comment "This relation indicates that an instance belonging to one class in { Material, Method, Metric, OtherEntity, Task } supports an instance of  OtherEntity. It is designed based on the following predicates extracted by the NLP pipeline: help,support,aid,assist,back,underlie,enable,promote,empower,facilitate,foster,facilitate,allow,hold,bear" ;
    rdfs:domain _:N77f97df3763b4e5380481a85960e8fd2 ;
    rdfs:range cskg-ont:OtherEntity ;
    rdfs:subPropertyOf cskg-ont:supports ;
    owl:inverseOf cskg-ont:otherentitySupportedBy .

cskg-ont:supportsTask a owl:ObjectProperty ;
    rdfs:comment "This relation indicates that an instance belonging to one class in { Material, Method, Metric, OtherEntity, Task } supports an instance of  Task. It is designed based on the following predicates extracted by the NLP pipeline: help,support,aid,assist,back,underlie,enable,promote,empower,facilitate,foster,facilitate,allow,hold,bear" ;
    rdfs:domain _:N99f8dc357c4f4b7da81b5653cc759ff7 ;
    rdfs:range cskg-ont:Task ;
    rdfs:subPropertyOf cskg-ont:supports ;
    owl:inverseOf cskg-ont:taskSupportedBy .

cskg-ont:taskAcquiredBy a owl:ObjectProperty,
        owl:TransitiveProperty ;
    rdfs:comment "This relation indicates that an instance	 of class Task was acquired by an instance belonging to one of the following classes { Method, Task }. It is designed based on the following predicates extracted by the NLP pipeline: select,accumulate,recoup,source,receive,acquire,regain,retrieve,obtain,accrue,borrow,subselect,inherit,accept,collect,gather,store,attract,get,capture,record,achieve" ;
    rdfs:domain cskg-ont:Task ;
    rdfs:range _:N35e6671791614fab9c31cbb63e75adba ;
    rdfs:subPropertyOf cskg-ont:acquiredBy ;
    owl:inverseOf cskg-ont:acquiresTask .

cskg-ont:taskAdaptedBy a owl:ObjectProperty,
        owl:TransitiveProperty ;
    rdfs:comment "This relation indicates that an instance	 of class Task was adapted by an instance belonging to one of the following classes { Method, OtherEntity, Task }. It is designed based on the following predicates extracted by the NLP pipeline: readapt,adjust,conform,adapt,gear,readjust,fit,assimilate,accommodate,personalize,customize,specialize,generalize,tailor,refine" ;
    rdfs:domain cskg-ont:Task ;
    rdfs:range _:Nbad3c5cc49e541bcab922a7e6e1576e7 ;
    rdfs:subPropertyOf cskg-ont:adaptedBy ;
    owl:inverseOf cskg-ont:adaptsTask .

cskg-ont:taskAffectedBy a owl:ObjectProperty ;
    rdfs:comment "This relation indicates that an instance	 of class Task was affected by an instance belonging to one of the following classes { Method, Metric, OtherEntity, Task }. It is designed based on the following predicates extracted by the NLP pipeline: placate,provoke,engage,console,impair,repulse,shake,discombobulate,threaten,inflame,thrill,satisfy,unsettle,kill,enrapture,outrage,disgruntle,reassure,discompose,interest,alarm,engross,afflict,manipulate,edit,update,increase,replace,modify,fatigue,refresh,cut" ;
    rdfs:domain cskg-ont:Task ;
    rdfs:range _:N1067ae94682b42c18653eadaac85deff ;
    rdfs:subPropertyOf cskg-ont:affectedBy ;
    owl:inverseOf cskg-ont:affectsTask .

cskg-ont:taskAnalyzedBy a owl:ObjectProperty,
        owl:TransitiveProperty ;
    rdfs:comment "This relation indicates that an instance	 of class Task was analyzed by an instance belonging to one of the following classes { Method, Metric, Task }. It is designed based on the following predicates extracted by the NLP pipeline: analyze,assess,study,try_on,scan,approximate,proofread,inspect,sample,research,check,appraise,analyse,examine,watch,audit,feel_out,go_over,consult,survey,test,assay,try,evaluate,investigate,monitor,regard,peruse,review,try_out,measure,calculate,address,estimate" ;
    rdfs:domain cskg-ont:Task ;
    rdfs:range _:N7b2ed255dc74415284c07048e5bd44cf ;
    rdfs:subPropertyOf cskg-ont:analyzedBy ;
    owl:inverseOf cskg-ont:analyzesTask .

cskg-ont:taskAnnotatedBy a owl:ObjectProperty ;
    rdfs:comment "This relation indicates that an instance	 of class Task was annotated by an instance belonging to one of the following classes { Method, Task }. It is designed based on the following predicates extracted by the NLP pipeline: scar,stipple,annotate,stamp,embroider,incise,inscribe,engrave,applique,imprint,paint,reinscribe,mark,sign,tag,label" ;
    rdfs:domain cskg-ont:Task ;
    rdfs:range _:Nf0d2aa6e99b04ae6944e92df8712aec0 ;
    rdfs:subPropertyOf cskg-ont:annotatedBy ;
    owl:inverseOf cskg-ont:annotatesTask .

cskg-ont:taskAutomatedBy a owl:ObjectProperty ;
    rdfs:comment "This relation indicates that an instance	 of class Task was automated by an instance belonging to one of the following classes { Method, OtherEntity }. It is designed based on the following predicates extracted by the NLP pipeline: automate" ;
    rdfs:domain cskg-ont:Task ;
    rdfs:range _:N2aa6a5f8122f449185ed52bbf0a15b7f ;
    rdfs:subPropertyOf cskg-ont:automatedBy ;
    owl:inverseOf cskg-ont:automatesTask .

cskg-ont:taskBases a owl:ObjectProperty,
        owl:TransitiveProperty ;
    rdfs:comment "This relation indicates that an instance	 of class Task was bases by an instance belonging to one of the following classes { Material, Method, Metric, OtherEntity, Task }. It is designed based on the following predicates extracted by the NLP pipeline: base,ground,found,construe,build,establish" ;
    rdfs:domain cskg-ont:Task ;
    rdfs:range _:Ne8dc2f8964064602885a66d293f855e5 ;
    rdfs:subPropertyOf cskg-ont:bases ;
    owl:inverseOf cskg-ont:based-onTask .

cskg-ont:taskCausedBy a owl:ObjectProperty ;
    rdfs:comment "This relation indicates that an instance	 of class Task was caused by an instance belonging to one of the following classes { Method, Metric, OtherEntity, Task }. It is designed based on the following predicates extracted by the NLP pipeline: cause,influence" ;
    rdfs:domain cskg-ont:Task ;
    rdfs:range _:N0e7780581a8a4d36a89b991aa4e88270 ;
    rdfs:subPropertyOf cskg-ont:causedBy ;
    owl:inverseOf cskg-ont:causesTask .

cskg-ont:taskClassifiedBy a owl:ObjectProperty ;
    rdfs:comment "This relation indicates that an instance	 of class Task was classified by an instance belonging to one of the following classes { Method, Metric, OtherEntity, Task }. It is designed based on the following predicates extracted by the NLP pipeline: regroup,bracket,categorize,recode,chunk,code,separate,group,sort,sort_out,catalogue,classify,class,number,seed,reclassify,grade" ;
    rdfs:domain cskg-ont:Task ;
    rdfs:range _:N2ef7f44fc61b4c279d0516a584ce1183 ;
    rdfs:subPropertyOf cskg-ont:classifiedBy ;
    owl:inverseOf cskg-ont:classifiesTask .

cskg-ont:taskContributedBy a owl:ObjectProperty ;
    rdfs:comment "This relation indicates that an instance	 of class Task was contributed by an instance belonging to one of the following classes { Method, OtherEntity, Task }. It is designed based on the following predicates extracted by the NLP pipeline: abnegate,gift,pass_out,turn-over,restore,turn-in,give-out,disburse,give-away,proffer,distribute,remit,transfer,extend,shell_out,give-up,hand_out,refer,disseminate,contribute" ;
    rdfs:domain cskg-ont:Task ;
    rdfs:range _:N05212fdb40c2415597e72a670c36a9cb ;
    rdfs:subPropertyOf cskg-ont:contributedBy ;
    owl:inverseOf cskg-ont:contributes-toTask .

cskg-ont:taskDiscussedBy a owl:ObjectProperty ;
    rdfs:comment "This relation indicates that an instance	 of class Task was discussed by an instance belonging to one of the following classes { Task }. It is designed based on the following predicates extracted by the NLP pipeline: debate,discuss,chatter,confer,converse,argue,discus" ;
    rdfs:domain cskg-ont:Task ;
    rdfs:range _:Na4e8e1ac70ae44409f0bd9176f121197 ;
    rdfs:subPropertyOf cskg-ont:discussedBy ;
    owl:inverseOf cskg-ont:discussesTask .

cskg-ont:taskExecutedBy a owl:ObjectProperty,
        owl:TransitiveProperty ;
    rdfs:comment "This relation indicates that an instance	 of class Task was executed by an instance belonging to one of the following classes { Method, Task }. It is designed based on the following predicates extracted by the NLP pipeline: perform,execute,operate,run,simulate,play,work,train,action" ;
    rdfs:domain cskg-ont:Task ;
    rdfs:range _:Na8087c12038741179751d08d18e7e3bc ;
    rdfs:subPropertyOf cskg-ont:executedBy ;
    owl:inverseOf cskg-ont:executesTask .

cskg-ont:taskExtractedBy a owl:ObjectProperty,
        owl:TransitiveProperty ;
    rdfs:comment "This relation indicates that an instance	 of class Task was extracted by an instance belonging to one of the following classes { Material, Method, Task }. It is designed based on the following predicates extracted by the NLP pipeline: extract,mine,induce,infer" ;
    rdfs:domain cskg-ont:Task ;
    rdfs:range _:N2cbdf4d21ad247858a139a0db3288bb9 ;
    rdfs:subPropertyOf cskg-ont:extractedBy ;
    owl:inverseOf cskg-ont:extractsTask .

cskg-ont:taskGuidedBy a owl:ObjectProperty ;
    rdfs:comment "This relation indicates that an instance	 of class Task was guided by an instance belonging to one of the following classes { Method, OtherEntity, Task }. It is designed based on the following predicates extracted by the NLP pipeline: steer,conduct,guide,misdirect,lead,escort,accompany,direct" ;
    rdfs:domain cskg-ont:Task ;
    rdfs:range _:N5ae634f65eac4fedb488fffb891db558 ;
    rdfs:subPropertyOf cskg-ont:guidedBy ;
    owl:inverseOf cskg-ont:guidesTask .

cskg-ont:taskHighlightedBy a owl:ObjectProperty ;
    rdfs:comment "This relation indicates that an instance	 of class Task was highlighted by an instance belonging to one of the following classes { Material, Method, OtherEntity, Task }. It is designed based on the following predicates extracted by the NLP pipeline: highlight,emphasize" ;
    rdfs:domain cskg-ont:Task ;
    rdfs:range _:Nd3ca8cbb75dc405ca9d7fef969d2dc40 ;
    rdfs:subPropertyOf cskg-ont:highlightedBy ;
    owl:inverseOf cskg-ont:highlightsTask .

cskg-ont:taskIdentifiedBy a owl:ObjectProperty ;
    rdfs:comment "This relation indicates that an instance	 of class Task was identified by an instance belonging to one of the following classes { Method, OtherEntity, Task }. It is designed based on the following predicates extracted by the NLP pipeline: identify,detect,filter,recognize,locate" ;
    rdfs:domain cskg-ont:Task ;
    rdfs:range _:N6fc28ae3bc614aa5a75fd033d634fbf2 ;
    rdfs:subPropertyOf cskg-ont:identifiedBy ;
    owl:inverseOf cskg-ont:identifiesTask .

cskg-ont:taskImprovedBy a owl:ObjectProperty ;
    rdfs:comment "This relation indicates that an instance	 of class Task was improved by an instance belonging to one of the following classes { Material, Method, Metric, Task }. It is designed based on the following predicates extracted by the NLP pipeline: improve,evolve,grow,enrich,expand,augment,raise,enhance,advance,gain,optimize" ;
    rdfs:domain cskg-ont:Task ;
    rdfs:range _:Nc386a051f3e9404782512bb5046e9df6 ;
    rdfs:subPropertyOf cskg-ont:improvedBy ;
    owl:inverseOf cskg-ont:improvesTask .

cskg-ont:taskIncludedBy a owl:ObjectProperty,
        owl:TransitiveProperty ;
    rdfs:comment "This relation indicates that an instance	 of class Task was included by an instance belonging to one of the following classes { Method, Task }. It is designed by the Feature-of and Part-of relationships extracted by the DyGIE++. It is also designed based on the following predicates extracted by the NLP pipeline: 'relate,include,involve,engage,enroll,embed,contain,comprise,carry,cover,consider,share,mount,have,equip,install" ;
    rdfs:domain cskg-ont:Task ;
    rdfs:range _:Nfe8a492d8bc446d6badfb8ef747c73f5 ;
    rdfs:subPropertyOf cskg-ont:includedBy ;
    owl:inverseOf cskg-ont:includesTask .

cskg-ont:taskInteracts-With a owl:ObjectProperty ;
    rdfs:comment "This relation indicates that an instance	 of class Task was interacts-with by an instance belonging to one of the following classes { Material, Method, Metric, OtherEntity, Task }. It is designed based on the following predicates extracted by the NLP pipeline: renegotiate,compromise,agree,debate,interact,collaborate,disagree,communicate,haggle,interlink,participate" ;
    rdfs:domain cskg-ont:Task ;
    rdfs:range _:N60a43915fb6c4bd483370f770935a5b9 ;
    rdfs:subPropertyOf cskg-ont:interacts-with ;
    owl:inverseOf cskg-ont:interacts-withTask .

cskg-ont:taskLackedof a owl:ObjectProperty ;
    rdfs:comment "This relation indicates that an instance	 of class Task was lackedof by an instance belonging to one of the following classes { Material, Method, Task }. It is designed based on the following predicates extracted by the NLP pipeline: lack" ;
    rdfs:domain cskg-ont:Task ;
    rdfs:range _:N1199cb3160fd4657961cd60acea9c881 ;
    rdfs:subPropertyOf cskg-ont:lackedOf ;
    owl:inverseOf cskg-ont:lacksTask .

cskg-ont:taskLearnedBy a owl:ObjectProperty ;
    rdfs:comment "This relation indicates that an instance	 of class Task was learned by an instance belonging to one of the following classes { Material, Method, OtherEntity, Task }. It is designed based on the following predicates extracted by the NLP pipeline: memorize,glean,learn,study,absorb,assimilate,cram,relearn,read" ;
    rdfs:domain cskg-ont:Task ;
    rdfs:range _:N9ee201229f954e9cb0c1d007f3277890 ;
    rdfs:subPropertyOf cskg-ont:learnedBy ;
    owl:inverseOf cskg-ont:learnsTask .

cskg-ont:taskLimitedBy a owl:ObjectProperty ;
    rdfs:comment "This relation indicates that an instance	 of class Task was limited by an instance belonging to one of the following classes { Material, Method, Metric, OtherEntity, Task }. It is designed based on the following predicates extracted by the NLP pipeline: reduce,limit,confine,restrain,constrain,restrict,prevent" ;
    rdfs:domain cskg-ont:Task ;
    rdfs:range _:N1b0212194ffc4a3eae84da8bbd9c1a17 ;
    rdfs:subPropertyOf cskg-ont:limitedBy ;
    owl:inverseOf cskg-ont:limitsTask .

cskg-ont:taskLinkedBy a owl:ObjectProperty,
        owl:TransitiveProperty ;
    rdfs:comment "This relation indicates that an instance	 of class Task was linked by an instance belonging to one of the following classes { Method, OtherEntity, Task }. It is designed based on the following predicates extracted by the NLP pipeline: fasten,strap,hook,lasso,leash,reeve,peg,rope,seal,clamp,latch,chain,band,trammel,shackle,clasp,knot,button,lock,moor,buckle,yoke,manacle,screw,link,string,pin,tether,paste,anchor,bond,wire,connect" ;
    rdfs:domain cskg-ont:Task ;
    rdfs:range _:N20e3c93bde28431db37c1313ed671e6e ;
    rdfs:subPropertyOf cskg-ont:linkedBy ;
    owl:inverseOf cskg-ont:linksTask .

cskg-ont:taskManagedBy a owl:ObjectProperty,
        owl:TransitiveProperty ;
    rdfs:comment "This relation indicates that an instance	 of class Task was managed by an instance belonging to one of the following classes { Method, Task }. It is designed based on the following predicates extracted by the NLP pipeline: look_out,wait_on,look_after,care,manage,maintain,preserve,keep,handle,treat,deal,configure" ;
    rdfs:domain cskg-ont:Task ;
    rdfs:range _:N618060df18e6473e9d6a6ba16882c462 ;
    rdfs:subPropertyOf cskg-ont:managedBy ;
    owl:inverseOf cskg-ont:managesTask .

cskg-ont:taskMatchedBy a owl:ObjectProperty ;
    rdfs:comment "This relation indicates that an instance	 of class Task was matched by an instance belonging to one of the following classes { Method, Task }. It is designed based on the following predicates extracted by the NLP pipeline: harmonize,go,square,dovetail,couple,pair,alternate,align,map,compare,match" ;
    rdfs:domain cskg-ont:Task ;
    rdfs:range _:Nf29389327a4f4441a7638e9b87845ca2 ;
    rdfs:subPropertyOf cskg-ont:matchedBy ;
    owl:inverseOf cskg-ont:matchesTask .

cskg-ont:taskOutperformedBy a owl:ObjectProperty,
        owl:TransitiveProperty ;
    rdfs:comment "This relation indicates that an instance	 of class Task was outperformed by an instance belonging to one of the following classes { Method, Task }. It is designed based on the following predicates extracted by the NLP pipeline: outperform" ;
    rdfs:domain cskg-ont:Task ;
    rdfs:range _:Ne820e56ea37d4cc8b0b1e18266d61899 ;
    rdfs:subPropertyOf cskg-ont:outperformedBy ;
    owl:inverseOf cskg-ont:outperformsTask .

cskg-ont:taskPredictedBy a owl:ObjectProperty ;
    rdfs:comment "This relation indicates that an instance	 of class Task was predicted by an instance belonging to one of the following classes { Material, Method, OtherEntity, Task }. It is designed based on the following predicates extracted by the NLP pipeline: denote,corroborate,indicate,imply,predict,anticipate,forebode,say,expose,prognosticate,explain,forecast" ;
    rdfs:domain cskg-ont:Task ;
    rdfs:range _:N0b422da05d3c4d2293fa30de0b98d6e1 ;
    rdfs:subPropertyOf cskg-ont:predictedBy ;
    owl:inverseOf cskg-ont:predictsTask .

cskg-ont:taskProcessedBy a owl:ObjectProperty ;
    rdfs:comment "This relation indicates that an instance	 of class Task was processed by an instance belonging to one of the following classes { Method, OtherEntity, Task }. It is designed based on the following predicates extracted by the NLP pipeline: process,proces" ;
    rdfs:domain cskg-ont:Task ;
    rdfs:range _:N66dc74126f5c44409fda43db68f1be57 ;
    rdfs:subPropertyOf cskg-ont:processedBy ;
    owl:inverseOf cskg-ont:processesTask .

cskg-ont:taskProducedBy a owl:ObjectProperty,
        owl:TransitiveProperty ;
    rdfs:comment "This relation indicates that an instance	 of class Task was produced by an instance belonging to one of the following classes { Method, Task }. It is designed based on the following predicates extracted by the NLP pipeline: author,coin,compose,compute,conoct,construct,contrive,cowrite,create,derive,draft,fabricate,form,formulate,invent,manufacture,model,organize,produce,rebuild,recreate,style,synthesize,write,generate,design,develop,implement,deploy,make,do" ;
    rdfs:domain cskg-ont:Task ;
    rdfs:range _:N11e01c48cf0b41f8a07ab64da28f89b3 ;
    rdfs:subPropertyOf cskg-ont:producedBy ;
    owl:inverseOf cskg-ont:producesTask .

cskg-ont:taskProposedBy a owl:ObjectProperty ;
    rdfs:comment "This relation indicates that an instance	 of class Task was proposed by an instance belonging to one of the following classes { Method, OtherEntity, Task }. It is designed based on the following predicates extracted by the NLP pipeline: propose,report,say,state,recommend,suggest,hint,introduce,outline,promise" ;
    rdfs:domain cskg-ont:Task ;
    rdfs:range _:N67712a1fb05f4cd4bd69c7bc8c6b53fb ;
    rdfs:subPropertyOf cskg-ont:proposedBy ;
    owl:inverseOf cskg-ont:proposesTask .

cskg-ont:taskProvidedBy a owl:ObjectProperty,
        owl:TransitiveProperty ;
    rdfs:comment "This relation indicates that an instance	 of class Task was provided by an instance belonging to one of the following classes { Method, Task }. It is designed based on the following predicates extracted by the NLP pipeline: present,furnish,resupply,serve,supply,provide,yield,give,add,assign" ;
    rdfs:domain cskg-ont:Task ;
    rdfs:range _:N238d5b5ca3454fa5bc4c9fa1a192c826 ;
    rdfs:subPropertyOf cskg-ont:providedBy ;
    owl:inverseOf cskg-ont:providesTask .

cskg-ont:taskSolvedBy a owl:ObjectProperty ;
    rdfs:comment "This relation indicates that an instance	 of class Task was solved by an instance belonging to one of the following classes { Material, Method, Metric, OtherEntity, Task }. It is designed based on the following predicates extracted by the NLP pipeline: find,determine,see,rationalize,guess,deduce,solve,discover,pick_up,ascertain,realize,relearn,ascertain,realize,relearn,fix" ;
    rdfs:domain cskg-ont:Task ;
    rdfs:range _:Ne84f44c11bdf4d58a6f9736f48b3ae13 ;
    rdfs:subPropertyOf cskg-ont:solvedBy ;
    owl:inverseOf cskg-ont:solvesTask .

cskg-ont:taskStandardizedBy a owl:ObjectProperty ;
    rdfs:comment "This relation indicates that an instance	 of class Task was standardized by an instance belonging to one of the following classes { Material, Method, Metric, OtherEntity, Task }. It is designed based on the following predicates extracted by the NLP pipeline: standardize,standardise" ;
    rdfs:domain cskg-ont:Task ;
    rdfs:range _:N65a40cf82d8c4baaaa10dd77428da2b4 ;
    rdfs:subPropertyOf cskg-ont:standardizedBy ;
    owl:inverseOf cskg-ont:standardizesTask .

cskg-ont:taskSupportedBy a owl:ObjectProperty ;
    rdfs:comment "This relation indicates that an instance	 of class Task was supported by an instance belonging to one of the following classes { Material, Method, Metric, OtherEntity, Task }. It is designed based on the following predicates extracted by the NLP pipeline: help,support,aid,assist,back,underlie,enable,promote,empower,facilitate,foster,facilitate,allow,hold,bear" ;
    rdfs:domain cskg-ont:Task ;
    rdfs:range _:N99f8dc357c4f4b7da81b5653cc759ff7 ;
    rdfs:subPropertyOf cskg-ont:supportedBy ;
    owl:inverseOf cskg-ont:supportsTask .

cskg-ont:taskTransferredBy a owl:ObjectProperty ;
    rdfs:comment "This relation indicates that an instance	 of class Task was transferred by an instance belonging to one of the following classes { Material, Method, OtherEntity, Task }. It is designed based on the following predicates extracted by the NLP pipeline: deliver,dispatch,shunt,airmail,import,forward,ship,send,transship,transmit,pass,hand,transport,shift,export,express,post,wire,transfer,drive,slip,port,return,convey,handdeliver,mail,answer" ;
    rdfs:domain cskg-ont:Task ;
    rdfs:range _:N4cb06259f0a746d599629e4aa410af9d ;
    rdfs:subPropertyOf cskg-ont:transferredBy ;
    owl:inverseOf cskg-ont:transfersTask .

cskg-ont:taskUsedBy a owl:ObjectProperty,
        owl:TransitiveProperty ;
    rdfs:comment "This relation indicates that an instance	 of class Task was used by an instance belonging to one of the following classes { Method, Metric, Task }. It is designed by the Used-for relationships extracted by the DyGIE++. It is also designed based on the following predicates extracted by the NLP pipeline: apply,employ,exert,exploit,reuse,use,utilize,utilise,adopt,leverage,rely,access" ;
    rdfs:domain cskg-ont:Task ;
    rdfs:range _:Nbaa39987224f457e8b27f689c11db5c6 ;
    rdfs:subPropertyOf cskg-ont:usedBy ;
    owl:inverseOf cskg-ont:usesTask .

cskg-ont:taskVisualizedBy a owl:ObjectProperty ;
    rdfs:comment "This relation indicates that an instance	 of class Task was visualized by an instance belonging to one of the following classes { OtherEntity }. It is designed based on the following predicates extracted by the NLP pipeline: visualize,disclose,reflect" ;
    rdfs:domain cskg-ont:Task ;
    rdfs:range _:N587d559e54b447ee9b6a96be613707c2 ;
    rdfs:subPropertyOf cskg-ont:visualizedBy ;
    owl:inverseOf cskg-ont:visualizesTask .

cskg-ont:transfersMaterial a owl:ObjectProperty ;
    rdfs:comment "This relation indicates that an instance belonging to one class in { Material, Method, Metric, OtherEntity, Task } transfers an instance of  Material. It is designed based on the following predicates extracted by the NLP pipeline: deliver,dispatch,shunt,airmail,import,forward,ship,send,transship,transmit,pass,hand,transport,shift,export,express,post,wire,transfer,drive,slip,port,return,convey,handdeliver,mail,answer" ;
    rdfs:domain _:N9ca46b7d5ba948fb8d1bce22a5201cb9 ;
    rdfs:range cskg-ont:Material ;
    rdfs:subPropertyOf cskg-ont:transfers ;
    owl:inverseOf cskg-ont:materialTransferredBy .

cskg-ont:transfersMethod a owl:ObjectProperty ;
    rdfs:comment "This relation indicates that an instance belonging to one class in { Material, Method, Metric, OtherEntity, Task } transfers an instance of  Method. It is designed based on the following predicates extracted by the NLP pipeline: deliver,dispatch,shunt,airmail,import,forward,ship,send,transship,transmit,pass,hand,transport,shift,export,express,post,wire,transfer,drive,slip,port,return,convey,handdeliver,mail,answer" ;
    rdfs:domain _:N3a1bcb2947c843f1be540ff3d252bbe9 ;
    rdfs:range cskg-ont:Method ;
    rdfs:subPropertyOf cskg-ont:transfers ;
    owl:inverseOf cskg-ont:methodTransferredBy .

cskg-ont:transfersMetric a owl:ObjectProperty ;
    rdfs:comment "This relation indicates that an instance belonging to one class in { Material, OtherEntity, Task } transfers an instance of  Metric. It is designed based on the following predicates extracted by the NLP pipeline: deliver,dispatch,shunt,airmail,import,forward,ship,send,transship,transmit,pass,hand,transport,shift,export,express,post,wire,transfer,drive,slip,port,return,convey,handdeliver,mail,answer" ;
    rdfs:domain _:N74f6d56423f346dc8b3f8d870cfd2926 ;
    rdfs:range cskg-ont:Metric ;
    rdfs:subPropertyOf cskg-ont:transfers ;
    owl:inverseOf cskg-ont:metricTransferredBy .

cskg-ont:transfersOtherEntity a owl:ObjectProperty ;
    rdfs:comment "This relation indicates that an instance belonging to one class in { Material, Method, Metric, OtherEntity, Task } transfers an instance of  OtherEntity. It is designed based on the following predicates extracted by the NLP pipeline: deliver,dispatch,shunt,airmail,import,forward,ship,send,transship,transmit,pass,hand,transport,shift,export,express,post,wire,transfer,drive,slip,port,return,convey,handdeliver,mail,answer" ;
    rdfs:domain _:N8ed691a078b54c38be50433903e66463 ;
    rdfs:range cskg-ont:OtherEntity ;
    rdfs:subPropertyOf cskg-ont:transfers ;
    owl:inverseOf cskg-ont:otherentityTransferredBy .

cskg-ont:transfersTask a owl:ObjectProperty ;
    rdfs:comment "This relation indicates that an instance belonging to one class in { Material, Method, OtherEntity, Task } transfers an instance of  Task. It is designed based on the following predicates extracted by the NLP pipeline: deliver,dispatch,shunt,airmail,import,forward,ship,send,transship,transmit,pass,hand,transport,shift,export,express,post,wire,transfer,drive,slip,port,return,convey,handdeliver,mail,answer" ;
    rdfs:domain _:N4cb06259f0a746d599629e4aa410af9d ;
    rdfs:range cskg-ont:Task ;
    rdfs:subPropertyOf cskg-ont:transfers ;
    owl:inverseOf cskg-ont:taskTransferredBy .

cskg-ont:usesMaterial a owl:ObjectProperty,
        owl:TransitiveProperty ;
    rdfs:comment "This relation indicates that an instance belonging to one class in { Method, Metric, OtherEntity, Task } uses an instance of  Material. It is designed by the Used-for relationships extracted by the DyGIE++. It is also designed based on the following predicates extracted by the NLP pipeline: apply,employ,exert,exploit,reuse,use,utilize,utilise,adopt,leverage,rely,access" ;
    rdfs:domain _:N7737e44cf65944dc83e0afa0502ac699 ;
    rdfs:range cskg-ont:Material ;
    rdfs:subPropertyOf cskg-ont:uses ;
    owl:inverseOf cskg-ont:materialUsedBy .

cskg-ont:usesMethod a owl:ObjectProperty,
        owl:TransitiveProperty ;
    rdfs:comment "This relation indicates that an instance belonging to one class in { Method, Metric, OtherEntity, Task } uses an instance of  Method. It is designed by the Used-for relationships extracted by the DyGIE++. It is also designed based on the following predicates extracted by the NLP pipeline: apply,employ,exert,exploit,reuse,use,utilize,utilise,adopt,leverage,rely,access" ;
    rdfs:domain _:Na1375b14902d42048768204c5ce0711f ;
    rdfs:range cskg-ont:Method ;
    rdfs:subPropertyOf cskg-ont:uses ;
    owl:inverseOf cskg-ont:methodUsedBy .

cskg-ont:usesMetric a owl:ObjectProperty,
        owl:TransitiveProperty ;
    rdfs:comment "This relation indicates that an instance belonging to one class in { Method, Metric, OtherEntity, Task } uses an instance of  Metric. It is designed by the Used-for relationships extracted by the DyGIE++. It is also designed based on the following predicates extracted by the NLP pipeline: apply,employ,exert,exploit,reuse,use,utilize,utilise,adopt,leverage,rely,access" ;
    rdfs:domain _:N729c182289a44f1cb3a3d8590f8f879c ;
    rdfs:range cskg-ont:Metric ;
    rdfs:subPropertyOf cskg-ont:uses ;
    owl:inverseOf cskg-ont:metricUsedBy .

cskg-ont:usesOtherEntity a owl:ObjectProperty,
        owl:TransitiveProperty ;
    rdfs:comment "This relation indicates that an instance belonging to one class in { Method, Metric, OtherEntity, Task } uses an instance of  OtherEntity. It is designed by the Used-for relationships extracted by the DyGIE++. It is also designed based on the following predicates extracted by the NLP pipeline: apply,employ,exert,exploit,reuse,use,utilize,utilise,adopt,leverage,rely,access" ;
    rdfs:domain _:N849ae1a9a93447adb97c0b77a0f8eb8e ;
    rdfs:range cskg-ont:OtherEntity ;
    rdfs:subPropertyOf cskg-ont:uses ;
    owl:inverseOf cskg-ont:otherentityUsedBy .

cskg-ont:usesTask a owl:ObjectProperty,
        owl:TransitiveProperty ;
    rdfs:comment "This relation indicates that an instance belonging to one class in { Method, Metric, Task } uses an instance of  Task. It is designed by the Used-for relationships extracted by the DyGIE++. It is also designed based on the following predicates extracted by the NLP pipeline: apply,employ,exert,exploit,reuse,use,utilize,utilise,adopt,leverage,rely,access" ;
    rdfs:domain _:Nbaa39987224f457e8b27f689c11db5c6 ;
    rdfs:range cskg-ont:Task ;
    rdfs:subPropertyOf cskg-ont:uses ;
    owl:inverseOf cskg-ont:taskUsedBy .

cskg-ont:visualizesMaterial a owl:ObjectProperty ;
    rdfs:comment "This relation indicates that an instance belonging to one class in { Material, Method, OtherEntity } visualizes an instance of  Material. It is designed based on the following predicates extracted by the NLP pipeline: visualize,disclose,reflect" ;
    rdfs:domain _:N9651cd8605e0463690c4598807c85aca ;
    rdfs:range cskg-ont:Material ;
    rdfs:subPropertyOf cskg-ont:visualizes ;
    owl:inverseOf cskg-ont:materialVisualizedBy .

cskg-ont:visualizesMethod a owl:ObjectProperty ;
    rdfs:comment "This relation indicates that an instance belonging to one class in { Material, Method, OtherEntity, Task } visualizes an instance of  Method. It is designed based on the following predicates extracted by the NLP pipeline: visualize,disclose,reflect" ;
    rdfs:domain _:N6164b28feaa64c4c9bea7aaae8ca2c72 ;
    rdfs:range cskg-ont:Method ;
    rdfs:subPropertyOf cskg-ont:visualizes ;
    owl:inverseOf cskg-ont:methodVisualizedBy .

cskg-ont:visualizesMetric a owl:ObjectProperty ;
    rdfs:comment "This relation indicates that an instance belonging to one class in { OtherEntity } visualizes an instance of  Metric. It is designed based on the following predicates extracted by the NLP pipeline: visualize,disclose,reflect" ;
    rdfs:domain _:N0efe5afe2d9d443882349b3cf85ecb78 ;
    rdfs:range cskg-ont:Metric ;
    rdfs:subPropertyOf cskg-ont:visualizes ;
    owl:inverseOf cskg-ont:metricVisualizedBy .

cskg-ont:visualizesOtherEntity a owl:ObjectProperty ;
    rdfs:comment "This relation indicates that an instance belonging to one class in { Material, Method, Metric, OtherEntity } visualizes an instance of  OtherEntity. It is designed based on the following predicates extracted by the NLP pipeline: visualize,disclose,reflect" ;
    rdfs:domain _:N75eaaf8f7d944145995cee9c2dc4b1f4 ;
    rdfs:range cskg-ont:OtherEntity ;
    rdfs:subPropertyOf cskg-ont:visualizes ;
    owl:inverseOf cskg-ont:otherentityVisualizedBy .

cskg-ont:visualizesTask a owl:ObjectProperty ;
    rdfs:comment "This relation indicates that an instance belonging to one class in { OtherEntity } visualizes an instance of  Task. It is designed based on the following predicates extracted by the NLP pipeline: visualize,disclose,reflect" ;
    rdfs:domain _:N587d559e54b447ee9b6a96be613707c2 ;
    rdfs:range cskg-ont:Task ;
    rdfs:subPropertyOf cskg-ont:visualizes ;
    owl:inverseOf cskg-ont:taskVisualizedBy .

cskg-ont:queriedBy a owl:ObjectProperty ;
    owl:inverseOf cskg-ont:queries .

cskg-ont:Statement rdfs:subClassOf rdf:Statement .

cskg-ont:automatedBy a owl:ObjectProperty ;
    owl:inverseOf cskg-ont:automates .

cskg-ont:matchedBy a owl:ObjectProperty ;
    owl:inverseOf cskg-ont:matches .

cskg-ont:queries a owl:ObjectProperty .

cskg-ont:annotatedBy a owl:ObjectProperty ;
    owl:inverseOf cskg-ont:annotates .

cskg-ont:automates a owl:ObjectProperty .

cskg-ont:executedBy a owl:ObjectProperty ;
    owl:inverseOf cskg-ont:executes .

cskg-ont:learnedBy a owl:ObjectProperty ;
    owl:inverseOf cskg-ont:learns .

cskg-ont:linkedBy a owl:ObjectProperty ;
    owl:inverseOf cskg-ont:links .

cskg-ont:matches a owl:ObjectProperty .

cskg-ont:ResearchEntity a owl:Class .

cskg-ont:acquiredBy a owl:ObjectProperty ;
    owl:inverseOf cskg-ont:acquires .

cskg-ont:adaptedBy a owl:ObjectProperty ;
    owl:inverseOf cskg-ont:adapts .

cskg-ont:affectedBy a owl:ObjectProperty ;
    owl:inverseOf cskg-ont:affects .

cskg-ont:analyzedBy a owl:ObjectProperty ;
    owl:inverseOf cskg-ont:analyzes .

cskg-ont:annotates a owl:ObjectProperty .

cskg-ont:bases a owl:ObjectProperty ;
    owl:inverseOf cskg-ont:based-on .

cskg-ont:causedBy a owl:ObjectProperty ;
    owl:inverseOf cskg-ont:causes .

cskg-ont:classifiedBy a owl:ObjectProperty ;
    owl:inverseOf cskg-ont:classifies .

cskg-ont:contributedBy a owl:ObjectProperty ;
    owl:inverseOf cskg-ont:contributes-to .

cskg-ont:discussedBy a owl:ObjectProperty ;
    owl:inverseOf cskg-ont:discusses .

cskg-ont:executes a owl:ObjectProperty .

cskg-ont:extractedBy a owl:ObjectProperty ;
    owl:inverseOf cskg-ont:extracts .

cskg-ont:guidedBy a owl:ObjectProperty ;
    owl:inverseOf cskg-ont:guides .

cskg-ont:highlightedBy a owl:ObjectProperty ;
    owl:inverseOf cskg-ont:highlights .

cskg-ont:identifiedBy a owl:ObjectProperty ;
    owl:inverseOf cskg-ont:identifies .

cskg-ont:improvedBy a owl:ObjectProperty ;
    owl:inverseOf cskg-ont:improves .

cskg-ont:includedBy a owl:ObjectProperty ;
    owl:inverseOf cskg-ont:includes .

cskg-ont:lackedOf a owl:ObjectProperty ;
    owl:inverseOf cskg-ont:lacks .

cskg-ont:learns a owl:ObjectProperty .

cskg-ont:limitedBy a owl:ObjectProperty ;
    owl:inverseOf cskg-ont:limits .

cskg-ont:links a owl:ObjectProperty .

cskg-ont:managedBy a owl:ObjectProperty ;
    owl:inverseOf cskg-ont:manages .

cskg-ont:outperformedBy a owl:ObjectProperty ;
    owl:inverseOf cskg-ont:outperforms .

cskg-ont:predictedBy a owl:ObjectProperty ;
    owl:inverseOf cskg-ont:predicts .

cskg-ont:processedBy a owl:ObjectProperty ;
    owl:inverseOf cskg-ont:processes .

cskg-ont:producedBy a owl:ObjectProperty ;
    owl:inverseOf cskg-ont:produces .

cskg-ont:proposedBy a owl:ObjectProperty ;
    owl:inverseOf cskg-ont:proposes .

cskg-ont:providedBy a owl:ObjectProperty ;
    owl:inverseOf cskg-ont:provides .

cskg-ont:solvedBy a owl:ObjectProperty ;
    owl:inverseOf cskg-ont:solves .

cskg-ont:standardizedBy a owl:ObjectProperty ;
    owl:inverseOf cskg-ont:standardizes .

cskg-ont:supportedBy a owl:ObjectProperty ;
    owl:inverseOf cskg-ont:supports .

cskg-ont:transferredBy a owl:ObjectProperty ;
    owl:inverseOf cskg-ont:transfers .

cskg-ont:usedBy a owl:ObjectProperty ;
    owl:inverseOf cskg-ont:uses .

cskg-ont:visualizedBy a owl:ObjectProperty ;
    owl:inverseOf cskg-ont:visualizes .

cskg-ont:acquires a owl:ObjectProperty .

cskg-ont:adapts a owl:ObjectProperty .

cskg-ont:affects a owl:ObjectProperty .

cskg-ont:analyzes a owl:ObjectProperty .

cskg-ont:based-on a owl:ObjectProperty .

cskg-ont:causes a owl:ObjectProperty .

cskg-ont:classifies a owl:ObjectProperty .

cskg-ont:contributes-to a owl:ObjectProperty .

cskg-ont:discusses a owl:ObjectProperty .

cskg-ont:extracts a owl:ObjectProperty .

cskg-ont:guides a owl:ObjectProperty .

cskg-ont:highlights a owl:ObjectProperty .

cskg-ont:identifies a owl:ObjectProperty .

cskg-ont:improves a owl:ObjectProperty .

cskg-ont:includes a owl:ObjectProperty .

cskg-ont:lacks a owl:ObjectProperty .

cskg-ont:limits a owl:ObjectProperty .

cskg-ont:manages a owl:ObjectProperty .

cskg-ont:outperforms a owl:ObjectProperty .

cskg-ont:predicts a owl:ObjectProperty .

cskg-ont:processes a owl:ObjectProperty .

cskg-ont:produces a owl:ObjectProperty .

cskg-ont:proposes a owl:ObjectProperty .

cskg-ont:provides a owl:ObjectProperty .

cskg-ont:solves a owl:ObjectProperty .

cskg-ont:standardizes a owl:ObjectProperty .

cskg-ont:supports a owl:ObjectProperty .

cskg-ont:transfers a owl:ObjectProperty .

cskg-ont:uses a owl:ObjectProperty .

cskg-ont:visualizes a owl:ObjectProperty .

cskg-ont:interacts-with a owl:ObjectProperty ;
    owl:inverseOf cskg-ont:interacts-with .

cskg-ont:Material a owl:Class ;
    rdfs:comment "An object that is processed, used, or returned by methods in order to pursue a task. In computer science it is typically  a data set, a knowledge base, or a system. Some examples include ‘vocabulary', 'biometric data', 'Wordnet', and 'social network'." ;
    rdfs:subClassOf cskg-ont:ResearchEntity .

cskg-ont:Metric a owl:Class ;
    rdfs:comment "A measure of quantitative assessment, commonly used for comparing or assessing the performance of a method.  Some examples include ‘word error rate', 'minimum classification error', 'normalized mutual information', and 'fault exposure ratio'." ;
    rdfs:subClassOf cskg-ont:ResearchEntity .

cskg-ont:OtherEntity a owl:Class ;
    rdfs:comment "A significant entity that we were unable to classify as task, method, metric, or material. It usually refers to real world entities that are used by or affect tasks and methods. Some examples include ‘password’, ‘keyboard’, ‘fingerprint’, and ‘pixel’." ;
    rdfs:subClassOf cskg-ont:ResearchEntity .

cskg-ont:Task a owl:Class ;
    rdfs:comment "A piece of work to carry out, usually to solve a specific challenge. Some examples include ‘knowledge discovery’, ‘dimensionality reduction’, ‘computer vision’, and ‘authentication’." ;
    rdfs:subClassOf cskg-ont:ResearchEntity .

cskg-ont:Method a owl:Class ;
    rdfs:comment "A specific approach, usually adopted to address a task.  Some examples include ‘neural networks’, decision trees’, ‘principal component analysis’, ‘support vector machine’, and ‘fuzzy logic’." ;
    rdfs:subClassOf cskg-ont:ResearchEntity .

_:N00d71bc8dd4e4517a1c5280c66fd5727 rdf:first cskg-ont:Method ;
    rdf:rest ( cskg-ont:OtherEntity cskg-ont:Task ) .

_:N011a954ff1454870859edc81c98e13c6 rdf:first cskg-ont:Method ;
    rdf:rest ( cskg-ont:OtherEntity ) .

_:N011bd47746d04fc5b98754f3e568b573 rdf:first cskg-ont:Method ;
    rdf:rest ( cskg-ont:OtherEntity cskg-ont:Task ) .

_:N0129a28476bc4a44b69b62e01577102a rdf:first cskg-ont:OtherEntity .

_:N023503d98460488bbdd07ce517757a57 rdf:first cskg-ont:Method ;
    rdf:rest ( cskg-ont:OtherEntity cskg-ont:Task ) .

_:N02f202bd4a5346329bfd3dcee6be5571 rdf:first cskg-ont:Task ;
    rdf:rest () .

_:N034c522acc1f43e79cfa096a60a5a4bf rdf:first cskg-ont:OtherEntity ;
    rdf:rest ( cskg-ont:Task ) .

_:N0397c30dde4b4106a21be38c6f394ca8 rdf:first cskg-ont:OtherEntity ;
    rdf:rest ( cskg-ont:Task ) .

_:N03db5811abeb473ebcfb21d29ef1e54f rdf:first cskg-ont:Method ;
    rdf:rest ( cskg-ont:Metric cskg-ont:OtherEntity cskg-ont:Task ) .

_:N0456c28cc753463a9889c94521a23f1f rdf:first cskg-ont:Material ;
    rdf:rest ( cskg-ont:Method cskg-ont:Metric cskg-ont:OtherEntity cskg-ont:Task ) .

_:N06059a52615a4604abc1bdb2667387d5 rdf:first cskg-ont:Metric ;
    rdf:rest ( cskg-ont:OtherEntity cskg-ont:Task ) .

_:N0688b207b0ed49b7abf6072dc7423721 rdf:first cskg-ont:OtherEntity ;
    rdf:rest ( cskg-ont:Task ) .

_:N07485d7939cb4ee58dd55d622647e23b rdf:first cskg-ont:Task ;
    rdf:rest () .

_:N075a3987b8854f719d98d1afb8b9091e rdf:first cskg-ont:Material ;
    rdf:rest ( cskg-ont:Method cskg-ont:OtherEntity cskg-ont:Task ) .

_:N09a86850c1a84248bef86a1280c03fab rdf:first cskg-ont:Method ;
    rdf:rest ( cskg-ont:Metric cskg-ont:OtherEntity cskg-ont:Task ) .

_:N09face0f27f44b09928bdb466a779e0c rdf:first cskg-ont:Method ;
    rdf:rest ( cskg-ont:Task ) .

_:N0a0b2f6df94849bcb13992dd496ab284 rdf:first cskg-ont:OtherEntity ;
    rdf:rest ( cskg-ont:Task ) .

_:N0b81f8e9173b4da7af9fd434760c39ec rdf:first cskg-ont:Method ;
    rdf:rest ( cskg-ont:Task ) .

_:N0babd092f4c140e18b0709bfcfbd29be rdf:first cskg-ont:Material ;
    rdf:rest ( cskg-ont:Method cskg-ont:OtherEntity cskg-ont:Task ) .

_:N0c2d09c5355849abaea05586d6696eca rdf:first cskg-ont:OtherEntity ;
    rdf:rest ( cskg-ont:Task ) .

_:N0c3daaf334284e53926d5f0664ac68cc rdf:first cskg-ont:Method ;
    rdf:rest _:N07485d7939cb4ee58dd55d622647e23b .

_:N0d17d2e9665f44e598089a1898c44b34 rdf:first cskg-ont:Method ;
    rdf:rest ( cskg-ont:Metric cskg-ont:OtherEntity cskg-ont:Task ) .

_:N0d2c6055aa72491b8d2e66cc61d07483 rdf:first cskg-ont:Method ;
    rdf:rest ( cskg-ont:Metric cskg-ont:OtherEntity cskg-ont:Task ) .

_:N0db2af1f81d343e58a846864fb771463 rdf:first cskg-ont:OtherEntity ;
    rdf:rest ( cskg-ont:Task ) .

_:N0e144eb248954797adce68c1c075fdc1 rdf:first cskg-ont:Task ;
    rdf:rest () .

_:N0ee15839e545403a8684f2493e10f215 rdf:first cskg-ont:Method ;
    rdf:rest ( cskg-ont:Metric cskg-ont:Task ) .

_:N0f57f9c0fb574da6b4d8eeddfb7e140f rdf:first cskg-ont:Method ;
    rdf:rest ( cskg-ont:Metric cskg-ont:OtherEntity cskg-ont:Task ) .

_:N0ff64bc263ec4d9683811082a85d894d rdf:first cskg-ont:Task ;
    rdf:rest () .

_:N10c75405423145ad9b67500e6227edb8 rdf:first cskg-ont:Material ;
    rdf:rest ( cskg-ont:Method cskg-ont:Metric cskg-ont:OtherEntity cskg-ont:Task ) .

_:N118f61bc94274d738cc61e8251fd7937 rdf:first cskg-ont:Method ;
    rdf:rest ( cskg-ont:Task ) .

_:N119eaaa881924fb9a1c53daee8fb8aad rdf:first cskg-ont:Metric ;
    rdf:rest ( cskg-ont:OtherEntity cskg-ont:Task ) .

_:N11e9f14108554d7089f86ba543666fc1 rdf:first cskg-ont:Method ;
    rdf:rest ( cskg-ont:Metric cskg-ont:OtherEntity cskg-ont:Task ) .

_:N120815489be6482e80d47cbe4598bd44 rdf:first cskg-ont:Material ;
    rdf:rest ( cskg-ont:Method cskg-ont:Metric cskg-ont:OtherEntity ) .

_:N12251e1a74404f3ab76a34b31c80e154 rdf:first cskg-ont:OtherEntity ;
    rdf:rest ( cskg-ont:Task ) .

_:N128ef342859e4746b8a22629e8c4ccec rdf:first cskg-ont:OtherEntity ;
    rdf:rest ( cskg-ont:Task ) .

_:N12e5703ab1594f90b691772a72c291ca rdf:first cskg-ont:OtherEntity ;
    rdf:rest ( cskg-ont:Task ) .

_:N13c3be75b19f4ebfb9af0b26c873ff57 rdf:first cskg-ont:OtherEntity ;
    rdf:rest ( cskg-ont:Task ) .

_:N13d0851218794eb08543e3e81ee73917 rdf:first cskg-ont:OtherEntity ;
    rdf:rest ( cskg-ont:Task ) .

_:N1413d27637dd4dc58047ee00d272c5e5 rdf:first cskg-ont:Material ;
    rdf:rest ( cskg-ont:Method cskg-ont:Metric cskg-ont:OtherEntity cskg-ont:Task ) .

_:N1553508c847c4d9883f924d768d7d093 rdf:first cskg-ont:Task .

_:N1561912a81c847a48e37f8fe62ea8da9 rdf:first cskg-ont:Method ;
    rdf:rest ( cskg-ont:Metric cskg-ont:OtherEntity cskg-ont:Task ) .

_:N158d800c52db43ec9d4bbae00cf1a709 rdf:first cskg-ont:Task ;
    rdf:rest () .

_:N173843268c8744f28c796601363886fd rdf:first cskg-ont:Task ;
    rdf:rest () .

_:N17adef71aba64a9c9b1e8fe56da8ed1d rdf:first cskg-ont:Task ;
    rdf:rest () .

_:N1802ca24d379455ab2fcd75aeddafda0 rdf:first cskg-ont:Metric ;
    rdf:rest ( cskg-ont:OtherEntity cskg-ont:Task ) .

_:N184b8af6cf6646c387f1c3f1362a9653 rdf:first cskg-ont:Task ;
    rdf:rest () .

_:N186045bc966a430cb34e5a3f35a0a02b rdf:first cskg-ont:OtherEntity ;
    rdf:rest ( cskg-ont:Task ) .

_:N19530fc6ad3244698314dbeee21e6d01 rdf:first cskg-ont:Task ;
    rdf:rest () .

_:N19894926da5f445c802f7f78a4941b57 rdf:first cskg-ont:Method ;
    rdf:rest ( cskg-ont:OtherEntity cskg-ont:Task ) .

_:N19b09e56a7074f239b7b775977ee484e rdf:first cskg-ont:OtherEntity ;
    rdf:rest ( cskg-ont:Task ) .

_:N1aa0cca5719e4b449cc2bcca395d2b9f rdf:first cskg-ont:Metric ;
    rdf:rest ( cskg-ont:OtherEntity ) .

_:N1ae773c663d34c3f86c42bdd4c2c07e8 rdf:first cskg-ont:Task ;
    rdf:rest () .

_:N1b3b49f603664825990870d68a672ae1 rdf:first cskg-ont:Method .

_:N1cdab02fbcc34d56b8fc06487398d9ec rdf:first cskg-ont:Metric ;
    rdf:rest ( cskg-ont:OtherEntity cskg-ont:Task ) .

_:N1cf57b2877cd4a7cb61eef8b52700525 rdf:first cskg-ont:Method ;
    rdf:rest ( cskg-ont:Metric cskg-ont:OtherEntity cskg-ont:Task ) .

_:N1d5f5d52827344d1ba7861eb2fa29724 rdf:first cskg-ont:Task ;
    rdf:rest () .

_:N1dc22a3b12d248a2aa1fb13c6e1cc216 rdf:first cskg-ont:Task ;
    rdf:rest () .

_:N1dc8fb95861e4fc6bed44e38610589e8 rdf:first cskg-ont:Method ;
    rdf:rest ( cskg-ont:OtherEntity cskg-ont:Task ) .

_:N1e054c22cd58420aa2d9929a5700c7da rdf:first cskg-ont:Task ;
    rdf:rest () .

_:N1eea0d6602294242a602aa68a749c1c4 rdf:first cskg-ont:Material ;
    rdf:rest ( cskg-ont:Method cskg-ont:Metric cskg-ont:OtherEntity cskg-ont:Task ) .

_:N1f1a6ed4cf0c458f85eff301046f538c rdf:first cskg-ont:Method ;
    rdf:rest ( cskg-ont:OtherEntity cskg-ont:Task ) .

_:N1f6ce42b5c8e4b8abf63d1980ed56df8 rdf:first cskg-ont:Method ;
    rdf:rest ( cskg-ont:OtherEntity cskg-ont:Task ) .

_:N1f8586395f3f44df965285eae6f0d62f rdf:first cskg-ont:Method ;
    rdf:rest ( cskg-ont:Metric cskg-ont:OtherEntity cskg-ont:Task ) .

_:N1f8ce8aaf1e74ea8a1fb96b371455890 rdf:first cskg-ont:Method ;
    rdf:rest ( cskg-ont:Metric cskg-ont:OtherEntity cskg-ont:Task ) .

_:N1fe56bc13c4a4995a64686f65948fa21 rdf:first cskg-ont:Material ;
    rdf:rest _:N0c3daaf334284e53926d5f0664ac68cc .

_:N21d9b923903a48b19be22b0d4b532307 rdf:first cskg-ont:Material ;
    rdf:rest ( cskg-ont:Method cskg-ont:OtherEntity cskg-ont:Task ) .

_:N2373b14852e941a6ab5afe3b9d88f739 rdf:first cskg-ont:Method ;
    rdf:rest ( cskg-ont:OtherEntity cskg-ont:Task ) .

_:N240edaabfc2c4e91893560f4141a176a rdf:first cskg-ont:Method ;
    rdf:rest ( cskg-ont:OtherEntity cskg-ont:Task ) .

_:N24fb30e7071b427b81e35556f82eeb57 rdf:first cskg-ont:Material ;
    rdf:rest ( cskg-ont:Method cskg-ont:Metric cskg-ont:OtherEntity ) .

_:N257d067e1430474bb72e44c59338b853 rdf:first cskg-ont:OtherEntity ;
    rdf:rest ( cskg-ont:Task ) .

_:N25d94618a13b4839a4f5a2f78bd05536 rdf:first cskg-ont:Task ;
    rdf:rest () .

_:N2606774712b44682b46747720846da33 rdf:first cskg-ont:Metric ;
    rdf:rest ( cskg-ont:OtherEntity cskg-ont:Task ) .

_:N276cc8fb9c2043e9b654815a45cc12f3 rdf:first cskg-ont:OtherEntity ;
    rdf:rest ( cskg-ont:Task ) .

_:N277b38525a4e42e3aa5bb8e3ac5cdef2 rdf:first cskg-ont:OtherEntity ;
    rdf:rest ( cskg-ont:Task ) .

_:N28eccecc71414264839ba5c5ba34e054 rdf:first cskg-ont:Task ;
    rdf:rest () .

_:N2963f894553f49a59d7243ac245e0225 rdf:first cskg-ont:Metric ;
    rdf:rest ( cskg-ont:OtherEntity ) .

_:N296b488a91d44016ac622d7b01c0bc4f rdf:first cskg-ont:Metric ;
    rdf:rest ( cskg-ont:OtherEntity cskg-ont:Task ) .

_:N299af42e149844dab7f464259f954041 rdf:first cskg-ont:Metric ;
    rdf:rest ( cskg-ont:OtherEntity cskg-ont:Task ) .

_:N29a9c9f01cfe4fe1b1fd134242cb1c5e rdf:first cskg-ont:OtherEntity ;
    rdf:rest ( cskg-ont:Task ) .

_:N29ab5816c51a475e8a7054f629b8f26b rdf:first cskg-ont:Material ;
    rdf:rest _:N1f1a6ed4cf0c458f85eff301046f538c .

_:N2a286d19a6ef4645937787365e744938 rdf:first cskg-ont:Task ;
    rdf:rest () .

_:N2a835df8a4064aa0940d3658f9a88740 rdf:first cskg-ont:OtherEntity ;
    rdf:rest ( cskg-ont:Task ) .

_:N2a9751b860f74144a42cc41042e14948 rdf:first cskg-ont:Method ;
    rdf:rest _:N0688b207b0ed49b7abf6072dc7423721 .

_:N2ab0f845007840f2817dbbf1e7f09161 rdf:first cskg-ont:Metric ;
    rdf:rest ( cskg-ont:OtherEntity cskg-ont:Task ) .

_:N2b8deef03b8041459b09cbac8445885e rdf:first cskg-ont:Material ;
    rdf:rest ( cskg-ont:Method cskg-ont:OtherEntity cskg-ont:Task ) .

_:N2c2431c8e504473780f7e6ca4e34df88 rdf:first cskg-ont:Metric ;
    rdf:rest ( cskg-ont:OtherEntity cskg-ont:Task ) .

_:N2c35b28be3a84d698e6f1a34ce3a4f2e rdf:first cskg-ont:Method ;
    rdf:rest ( cskg-ont:OtherEntity cskg-ont:Task ) .

_:N2c81e927804a4ff4884f1b82083fc89d rdf:first cskg-ont:Material ;
    rdf:rest ( cskg-ont:Method cskg-ont:OtherEntity cskg-ont:Task ) .

_:N2d18cf49b3c04cc9a4ea4eede90ef669 rdf:first cskg-ont:Metric ;
    rdf:rest _:N0a0b2f6df94849bcb13992dd496ab284 .

_:N2deedadb5afa4736a373dfd38fa42c07 rdf:first cskg-ont:Task ;
    rdf:rest () .

_:N2df8a031a69a43f0bd3609acb13a8391 rdf:first cskg-ont:Method ;
    rdf:rest _:N06059a52615a4604abc1bdb2667387d5 .

_:N2e107529b2064bf0b902dc8bb3a3591f rdf:first cskg-ont:Method ;
    rdf:rest ( cskg-ont:OtherEntity cskg-ont:Task ) .

_:N2e148bde616249df9f9ea506b71853f7 rdf:first cskg-ont:Material ;
    rdf:rest ( cskg-ont:Method cskg-ont:Metric cskg-ont:OtherEntity cskg-ont:Task ) .

_:N2e9e6ef1333640e589ea584ea643f646 rdf:first cskg-ont:Method ;
    rdf:rest ( cskg-ont:Metric cskg-ont:OtherEntity cskg-ont:Task ) .

_:N2f2477af535f4973a4992e55524e1571 rdf:first cskg-ont:OtherEntity ;
    rdf:rest ( cskg-ont:Task ) .

_:N3098c2da615e44acb3a2f900cca7bdcb rdf:first cskg-ont:Method ;
    rdf:rest ( cskg-ont:Metric cskg-ont:OtherEntity cskg-ont:Task ) .

_:N30c7008c8e70495a94138f1cd2b1ec6f rdf:first cskg-ont:Metric ;
    rdf:rest ( cskg-ont:OtherEntity cskg-ont:Task ) .

_:N30f20e84880c4aaeb54c0b1c2e64f348 rdf:first cskg-ont:OtherEntity ;
    rdf:rest ( cskg-ont:Task ) .

_:N31aac8e62dcf413f9c5f65de23987062 rdf:first cskg-ont:Method ;
    rdf:rest _:N1e054c22cd58420aa2d9929a5700c7da .

_:N31eb3fb93aef492d9b692da6cf5d6b79 rdf:first cskg-ont:OtherEntity ;
    rdf:rest ( cskg-ont:Task ) .

_:N32316297f097451a85fcbccadb8f80aa rdf:first cskg-ont:Task ;
    rdf:rest () .

_:N3434b435995a4420b4d116058085dc7c rdf:first cskg-ont:Material ;
    rdf:rest _:N0d2c6055aa72491b8d2e66cc61d07483 .

_:N34cf4ac27cd14acc8a9e5c86f40b77c4 rdf:first cskg-ont:Material ;
    rdf:rest ( cskg-ont:Method cskg-ont:Metric cskg-ont:OtherEntity cskg-ont:Task ) .

_:N350fe24abc3d428590192eb6697b7977 rdf:first cskg-ont:Method ;
    rdf:rest ( cskg-ont:OtherEntity cskg-ont:Task ) .

_:N35114d9912c945a0bc02981db32295a0 rdf:first cskg-ont:OtherEntity ;
    rdf:rest ( cskg-ont:Task ) .

_:N359bfb2314e54cf38785144b00784db0 rdf:first cskg-ont:Metric ;
    rdf:rest ( cskg-ont:OtherEntity cskg-ont:Task ) .

_:N361a34ee78c04d41815578223f4c6713 rdf:first cskg-ont:Material ;
    rdf:rest ( cskg-ont:Method cskg-ont:OtherEntity cskg-ont:Task ) .

_:N367e19eb79e2485886a26583cbdbe537 rdf:first cskg-ont:Method ;
    rdf:rest _:N0397c30dde4b4106a21be38c6f394ca8 .

_:N36fd6c05bd2648eaa38898752e4b4433 rdf:first cskg-ont:Metric ;
    rdf:rest ( cskg-ont:OtherEntity cskg-ont:Task ) .

_:N3723b329235e49c8a5b7258b6c711b1f rdf:first cskg-ont:Metric ;
    rdf:rest _:N0c2d09c5355849abaea05586d6696eca .

_:N3a09effe5ff64429b58e4623de9425be rdf:first cskg-ont:Task ;
    rdf:rest () .

_:N3aba3bf8fd7842f18b83804c7274fd83 rdf:first cskg-ont:Material ;
    rdf:rest ( cskg-ont:Method cskg-ont:Metric cskg-ont:OtherEntity cskg-ont:Task ) .

_:N3af777630a734bb4a15be2322e3541a5 rdf:first cskg-ont:Metric ;
    rdf:rest ( cskg-ont:OtherEntity cskg-ont:Task ) .

_:N3b05a6ea85294f1181f21aed93bb963d rdf:first cskg-ont:Task ;
    rdf:rest () .

_:N3b33710a9caf4f83b1414fc8c6323b6d rdf:first cskg-ont:Metric ;
    rdf:rest ( cskg-ont:OtherEntity cskg-ont:Task ) .

_:N3b8a3884fb07482ea066c60f81fdb2bb rdf:first cskg-ont:Material ;
    rdf:rest ( cskg-ont:Method cskg-ont:OtherEntity cskg-ont:Task ) .

_:N3c127ee7063649d7a4eac3d45175a79c rdf:first cskg-ont:OtherEntity ;
    rdf:rest ( cskg-ont:Task ) .

_:N3c6bb5052f0e4113b86c3397056dd720 rdf:first cskg-ont:Material ;
    rdf:rest ( cskg-ont:Method cskg-ont:Metric cskg-ont:OtherEntity cskg-ont:Task ) .

_:N3d2760c7b94d46f8988b575814731e67 rdf:first cskg-ont:OtherEntity ;
    rdf:rest ( cskg-ont:Task ) .

_:N3d2f8cadfc9c4f5ba45ed135df7cb414 rdf:first cskg-ont:Method ;
    rdf:rest ( cskg-ont:OtherEntity cskg-ont:Task ) .

_:N3db65a9894334b438c7228eddd38ab15 rdf:first cskg-ont:OtherEntity ;
    rdf:rest ( cskg-ont:Task ) .

_:N3dc5fbb8d3084826b9ea8be6c864477e rdf:first cskg-ont:Task ;
    rdf:rest () .

_:N40158b88d967434a97def16bcb94cd5d rdf:first cskg-ont:OtherEntity ;
    rdf:rest _:N25d94618a13b4839a4f5a2f78bd05536 .

_:N4066263359ba4b68b671418497961b7f rdf:first cskg-ont:OtherEntity .

_:N407d7f57fc85445b9a32144c59267441 rdf:first cskg-ont:Material ;
    rdf:rest ( cskg-ont:Method cskg-ont:Metric cskg-ont:OtherEntity cskg-ont:Task ) .

_:N40cb30f91d0a4e95ba56ec763023fdd1 rdf:first cskg-ont:Task ;
    rdf:rest () .

_:N40e77d4153664c4eb14598c39d3ee18d rdf:first cskg-ont:OtherEntity ;
    rdf:rest _:N32316297f097451a85fcbccadb8f80aa .

_:N40f02d1ecc854b74a70ec37d32c4bf90 rdf:first cskg-ont:OtherEntity ;
    rdf:rest ( cskg-ont:Task ) .

_:N4144a6f05b134161b1b3b1111a4a6172 rdf:first cskg-ont:OtherEntity ;
    rdf:rest ( cskg-ont:Task ) .

_:N4200428de3004e1b9f8159d40a616358 rdf:first cskg-ont:Method ;
    rdf:rest _:N276cc8fb9c2043e9b654815a45cc12f3 .

_:N4292e225ac6a43a8873173d3288395e2 rdf:first cskg-ont:Material ;
    rdf:rest ( cskg-ont:Method cskg-ont:OtherEntity ) .

_:N42a23b6e361949fa8910023566ec7e61 rdf:first cskg-ont:Method ;
    rdf:rest _:N1aa0cca5719e4b449cc2bcca395d2b9f .

_:N4308eed296ca492584eb19c2b2c42f72 rdf:first cskg-ont:Material ;
    rdf:rest ( cskg-ont:Method cskg-ont:Metric cskg-ont:Task ) .

_:N430f73b793f64a308b8ecaf12589c9d4 rdf:first cskg-ont:Metric ;
    rdf:rest _:N12e5703ab1594f90b691772a72c291ca .

_:N4415d9965ef94e40bc097f3f8845482a rdf:first cskg-ont:Method ;
    rdf:rest _:N30f20e84880c4aaeb54c0b1c2e64f348 .

_:N4456b2e148ff43f782c96833687ceb36 rdf:first cskg-ont:Task ;
    rdf:rest () .

_:N44d36ec5564b413e8952eaf0e393e64f rdf:first cskg-ont:OtherEntity ;
    rdf:rest ( cskg-ont:Task ) .

_:N453d8652f626420f94382d540d75ebdd rdf:first cskg-ont:Method ;
    rdf:rest _:N36fd6c05bd2648eaa38898752e4b4433 .

_:N45cc845b31eb46ef95f5286ab3897d82 rdf:first cskg-ont:Metric ;
    rdf:rest ( cskg-ont:OtherEntity cskg-ont:Task ) .

_:N45e4b0c46cf4411194e41d6476691ae3 rdf:first cskg-ont:Material ;
    rdf:rest ( cskg-ont:Method cskg-ont:OtherEntity cskg-ont:Task ) .

_:N47f35a29d79543cbaa0e5cab36b29893 rdf:first cskg-ont:Material ;
    rdf:rest ( cskg-ont:Method cskg-ont:Metric cskg-ont:OtherEntity cskg-ont:Task ) .

_:N480f83d24a1c45de83a40e973ba3956a rdf:first cskg-ont:Task ;
    rdf:rest () .

_:N4907e29ab3de44b0b301768d30338480 rdf:first cskg-ont:Material ;
    rdf:rest _:N453d8652f626420f94382d540d75ebdd .

_:N4a029d256e3f4ccabd5dfedd3f8f799b rdf:first cskg-ont:Method ;
    rdf:rest _:N2f2477af535f4973a4992e55524e1571 .

_:N4a155d6abd7f4d4c8660cd91c540b4df rdf:first cskg-ont:Task ;
    rdf:rest () .

_:N4a9f24282a744be9ab82ea96076d3b84 rdf:first cskg-ont:Task .

_:N4b5346c25d774880b44f01831511c94c rdf:first cskg-ont:Method ;
    rdf:rest ( cskg-ont:Task ) .

_:N4b7e598d1a17492eb3a9dcd8bada3f84 rdf:first cskg-ont:Task ;
    rdf:rest () .

_:N4c1c437c7b444582aa4c2f72c6b74e4f rdf:first cskg-ont:Task ;
    rdf:rest () .

_:N4d166115d0904303917bd04b25b3f738 rdf:first cskg-ont:Task ;
    rdf:rest () .

_:N4e05af78719542ad89be8ba1f63486e3 rdf:first cskg-ont:OtherEntity ;
    rdf:rest ( cskg-ont:Task ) .

_:N4e18b9c498974871914b740750923559 rdf:first cskg-ont:Material ;
    rdf:rest ( cskg-ont:Method cskg-ont:Task ) .

_:N4e7a9d25374a46eaa62690a71ad33f8e rdf:first cskg-ont:OtherEntity ;
    rdf:rest ( cskg-ont:Task ) .

_:N4feb4b172418496b9cddd5491d233379 rdf:first cskg-ont:Method ;
    rdf:rest ( cskg-ont:Metric cskg-ont:OtherEntity cskg-ont:Task ) .

_:N5008815c7f54406ebfed799503327bd8 rdf:first cskg-ont:Method ;
    rdf:rest ( cskg-ont:Task ) .

_:N50446e187a55473ab0f0989c2ac7f867 rdf:first cskg-ont:Metric ;
    rdf:rest _:N40f02d1ecc854b74a70ec37d32c4bf90 .

_:N50a61ff4df5c4b7aa826851727f92c67 rdf:first cskg-ont:Method ;
    rdf:rest ( cskg-ont:OtherEntity cskg-ont:Task ) .

_:N520e9a6dbcf443ee814952ffc680b7b6 rdf:first cskg-ont:Method ;
    rdf:rest ( cskg-ont:Metric cskg-ont:OtherEntity cskg-ont:Task ) .

_:N522d819d3e7944d988c9aa0fa72aa7cc rdf:first cskg-ont:Metric ;
    rdf:rest _:N35114d9912c945a0bc02981db32295a0 .

_:N558198da5c4c42b3be0e39e1ffd907a7 rdf:first cskg-ont:Metric ;
    rdf:rest _:N29a9c9f01cfe4fe1b1fd134242cb1c5e .

_:N5677a88d408542d88ce5c4fae5f36055 rdf:first cskg-ont:Task ;
    rdf:rest () .

_:N56cc45be5c6a4a0ebc5ed308f2172fee rdf:first cskg-ont:Material ;
    rdf:rest ( cskg-ont:Method cskg-ont:Metric cskg-ont:OtherEntity cskg-ont:Task ) .

_:N57625f6e0e824d1baa081c6789b551af rdf:first cskg-ont:Task ;
    rdf:rest () .

_:N591bccf1bdce440c96de7871e38402d3 rdf:first cskg-ont:Task ;
    rdf:rest () .

_:N59a4d1ee28744c3882954a0272fc725f rdf:first cskg-ont:Method ;
    rdf:rest ( cskg-ont:OtherEntity cskg-ont:Task ) .

_:N5b0b153960204042a0fe414d1a9c5685 rdf:first cskg-ont:Metric ;
    rdf:rest ( cskg-ont:OtherEntity cskg-ont:Task ) .

_:N5b2c1a46608643829222f2c674a8abac rdf:first cskg-ont:Method ;
    rdf:rest ( cskg-ont:Task ) .

_:N5c5efb26c95345f0829f69e6d50dc8fc rdf:first cskg-ont:Metric ;
    rdf:rest ( cskg-ont:OtherEntity cskg-ont:Task ) .

_:N5c84cb782a7d4482aeba3457badd7177 rdf:first cskg-ont:Method ;
    rdf:rest ( cskg-ont:Metric cskg-ont:OtherEntity cskg-ont:Task ) .

_:N5cbd2eda905a4956997a79fe4844496c rdf:first cskg-ont:Task ;
    rdf:rest () .

_:N5d9a59e1221f43c69f4f26b3e4f9f613 rdf:first cskg-ont:OtherEntity ;
    rdf:rest ( cskg-ont:Task ) .

_:N5ddb0f8f14544684a3c415b94afc4bbd rdf:first cskg-ont:Method ;
    rdf:rest _:N2963f894553f49a59d7243ac245e0225 .

_:N5fbbdc3fa66241c99bbcde8e33f95c39 rdf:first cskg-ont:OtherEntity ;
    rdf:rest ( cskg-ont:Task ) .

_:N5fe522788cde495ca1bb64e112e23502 rdf:first cskg-ont:Material ;
    rdf:rest _:N1f8586395f3f44df965285eae6f0d62f .

_:N6112df70fd0e4d54adca4442ea379247 rdf:first cskg-ont:Material ;
    rdf:rest ( cskg-ont:Method cskg-ont:Metric cskg-ont:OtherEntity cskg-ont:Task ) .

_:N6119575bf35941569c6ab7270308ab3e rdf:first cskg-ont:Method ;
    rdf:rest ( cskg-ont:Metric cskg-ont:OtherEntity cskg-ont:Task ) .

_:N617e921762004303a78ceaee441ffc66 rdf:first cskg-ont:Method ;
    rdf:rest ( cskg-ont:Metric cskg-ont:OtherEntity cskg-ont:Task ) .

_:N61a8dbd1937f4d31b67dbaee188c59ee rdf:first cskg-ont:Method ;
    rdf:rest ( cskg-ont:OtherEntity cskg-ont:Task ) .

_:N61d6a5024bdb4c92b4ffc21b7a975485 rdf:first cskg-ont:Method ;
    rdf:rest _:N299af42e149844dab7f464259f954041 .

_:N61d81ca015bb448985107bb69adaf378 rdf:first cskg-ont:Metric ;
    rdf:rest _:N3db65a9894334b438c7228eddd38ab15 .

_:N64bf09bf9d9e4aba9d6a30bc97ffac59 rdf:first cskg-ont:OtherEntity ;
    rdf:rest _:N0e144eb248954797adce68c1c075fdc1 .

_:N663c6756c25b4c268db06123b1a0abe6 rdf:first cskg-ont:Task ;
    rdf:rest () .

_:N681184d503aa43f9a622374d73cb189f rdf:first cskg-ont:OtherEntity ;
    rdf:rest _:N3dc5fbb8d3084826b9ea8be6c864477e .

_:N6900e0d27bc8420c90ff8403f3c5a707 rdf:first cskg-ont:OtherEntity ;
    rdf:rest ( cskg-ont:Task ) .

_:N6a3dedba0d57497bbaec61c28e1f7844 rdf:first cskg-ont:Material ;
    rdf:rest ( cskg-ont:Method cskg-ont:Metric cskg-ont:OtherEntity cskg-ont:Task ) .

_:N6a8224dd3c734e8db140d5055bfb3751 rdf:first cskg-ont:OtherEntity ;
    rdf:rest _:N1dc22a3b12d248a2aa1fb13c6e1cc216 .

_:N6ab57cdef9aa49e39e40c8b3dc6d3b46 rdf:first cskg-ont:Method ;
    rdf:rest ( cskg-ont:OtherEntity ) .

_:N6b1e46881fdf4032b4850f4d11a29e90 rdf:first cskg-ont:Method ;
    rdf:rest ( cskg-ont:Task ) .

_:N6b76ec9cbbff4464b8a655fa74b4eac1 rdf:first cskg-ont:OtherEntity ;
    rdf:rest _:N591bccf1bdce440c96de7871e38402d3 .

_:N6c2147785886496b98d7fab6be269482 rdf:first cskg-ont:OtherEntity ;
    rdf:rest ( cskg-ont:Task ) .

_:N6d0085797928440fbd6b1aade70beb3a rdf:first cskg-ont:Material ;
    rdf:rest _:N2df8a031a69a43f0bd3609acb13a8391 .

_:N6d033e34d85641729fe8c87d6787b8ce rdf:first cskg-ont:Method ;
    rdf:rest ( cskg-ont:OtherEntity cskg-ont:Task ) .

_:N6dc928c6c6554043af92138c574792c2 rdf:first cskg-ont:Metric ;
    rdf:rest ( cskg-ont:OtherEntity cskg-ont:Task ) .

_:N6f54ea87e09d4c618511541b6674d4d0 rdf:first cskg-ont:Method ;
    rdf:rest ( cskg-ont:OtherEntity cskg-ont:Task ) .

_:N6fb0a71854ef4ba7a7e294439aea2ef0 rdf:first cskg-ont:Task ;
    rdf:rest () .

_:N6fb3b204067a486089a981cdadc94734 rdf:first cskg-ont:Method ;
    rdf:rest ( cskg-ont:Metric cskg-ont:OtherEntity cskg-ont:Task ) .

_:N6fcb67e71fee453b85f39b607a6a4f2d rdf:first cskg-ont:Method ;
    rdf:rest ( cskg-ont:Metric cskg-ont:OtherEntity cskg-ont:Task ) .

_:N7093cb0e39414a1184d610c021faa1dc rdf:first cskg-ont:OtherEntity ;
    rdf:rest ( cskg-ont:Task ) .

_:N70e019cdc4554e77a69a557c54a7ba48 rdf:first cskg-ont:Method ;
    rdf:rest ( cskg-ont:Task ) .

_:N723e6a4163b64ad3945d01bf4348540e rdf:first cskg-ont:OtherEntity ;
    rdf:rest ( cskg-ont:Task ) .

_:N7298627f4e284295a16a7339c4fc4813 rdf:first cskg-ont:Method ;
    rdf:rest ( cskg-ont:OtherEntity cskg-ont:Task ) .

_:N730645bc35c645f9aaae9e0839d4f34c rdf:first cskg-ont:Task ;
    rdf:rest () .

_:N730890a7db7841dd95c4fc0711824bee rdf:first cskg-ont:Material ;
    rdf:rest _:N00d71bc8dd4e4517a1c5280c66fd5727 .

_:N731bf5de6d314e42b2de5c85dc84237c rdf:first cskg-ont:Material ;
    rdf:rest _:N2a9751b860f74144a42cc41042e14948 .

_:N734a6e0edb8a44bc817bc5b2ab0c746d rdf:first cskg-ont:Method ;
    rdf:rest ( cskg-ont:Metric cskg-ont:OtherEntity ) .

_:N735c56d5f6624e848d7c295c2bb2619e rdf:first cskg-ont:Material ;
    rdf:rest _:N5c84cb782a7d4482aeba3457badd7177 .

_:N74569c929e3d4966af0c32d0af497feb rdf:first cskg-ont:Material ;
    rdf:rest ( cskg-ont:Method cskg-ont:Metric cskg-ont:OtherEntity cskg-ont:Task ) .

_:N76521fc121514fcfa869533fc5af483e rdf:first cskg-ont:Method ;
    rdf:rest _:N61d81ca015bb448985107bb69adaf378 .

_:N7685e5bf7e2a47febb3eda4040f7ad79 rdf:first cskg-ont:Method ;
    rdf:rest _:N0db2af1f81d343e58a846864fb771463 .

_:N76f34f6fc120407f890abc116c79e8f3 rdf:first cskg-ont:Method ;
    rdf:rest ( cskg-ont:Metric cskg-ont:OtherEntity cskg-ont:Task ) .

_:N77cf8a73c84f422583794b6f2ba0143a rdf:first cskg-ont:OtherEntity ;
    rdf:rest ( cskg-ont:Task ) .

_:N795424ed5f9647d5afdc00248c01f343 rdf:first cskg-ont:Method ;
    rdf:rest _:N77cf8a73c84f422583794b6f2ba0143a .

_:N7bea1a9c83b9427cb67c7c6dcbe76cb2 rdf:first cskg-ont:OtherEntity ;
    rdf:rest _:N4456b2e148ff43f782c96833687ceb36 .

_:N7d8104710c384d73822983e676468b2f rdf:first cskg-ont:Metric ;
    rdf:rest ( cskg-ont:OtherEntity cskg-ont:Task ) .

_:N7e48fb8d68b64478ae57af3cddafd514 rdf:first cskg-ont:Material ;
    rdf:rest ( cskg-ont:Method cskg-ont:OtherEntity cskg-ont:Task ) .

_:N7eddee1a91f3408daf859bda8b69f700 rdf:first cskg-ont:Metric ;
    rdf:rest _:N7bea1a9c83b9427cb67c7c6dcbe76cb2 .

_:N7f36b9e8a5df4474a59539cc0afcf3fc rdf:first cskg-ont:Method ;
    rdf:rest ( cskg-ont:OtherEntity cskg-ont:Task ) .

_:N7f835d9496bb4b6fbb19ecee06c40b51 rdf:first cskg-ont:Material ;
    rdf:rest ( cskg-ont:Method cskg-ont:Metric cskg-ont:OtherEntity cskg-ont:Task ) .

_:N7fda587f2e1d46bb94743bea4bd9ef8c rdf:first cskg-ont:OtherEntity .

_:N8061d737b75b4a94b4880089ebbca371 rdf:first cskg-ont:Method ;
    rdf:rest ( cskg-ont:Task ) .

_:N80aae899d0944bc68bf342da8c5204b7 rdf:first cskg-ont:Metric ;
    rdf:rest ( cskg-ont:OtherEntity cskg-ont:Task ) .

_:N81aa8379608142b596e531e743e8cc70 rdf:first cskg-ont:Material ;
    rdf:rest ( cskg-ont:Method cskg-ont:Metric cskg-ont:OtherEntity cskg-ont:Task ) .

_:N81b9b4b5be0344598af89b33a25ecf02 rdf:first cskg-ont:Method ;
    rdf:rest _:N730645bc35c645f9aaae9e0839d4f34c .

_:N8631ae39328c4deaa23b71a74ee76ff8 rdf:first cskg-ont:Task ;
    rdf:rest () .

_:N86c40ff5de274756a8c344a92182cce6 rdf:first cskg-ont:Method ;
    rdf:rest _:N2a835df8a4064aa0940d3658f9a88740 .

_:N86f0b0f701344faa986264ea354e13e0 rdf:first cskg-ont:Task ;
    rdf:rest () .

_:N8704253fffa140c2ae6e7840dc66bf52 rdf:first cskg-ont:Method ;
    rdf:rest _:N034c522acc1f43e79cfa096a60a5a4bf .

_:N877e410744a94f51b2c7b485343c560d rdf:first cskg-ont:Method ;
    rdf:rest ( cskg-ont:Task ) .

_:N8a7962fb3418435fb18cca43f3390633 rdf:first cskg-ont:Method ;
    rdf:rest ( cskg-ont:Task ) .

_:N8b2d30035c8b4ef3b2abd3be57f6f26d rdf:first cskg-ont:Material ;
    rdf:rest ( cskg-ont:Method cskg-ont:Metric cskg-ont:OtherEntity cskg-ont:Task ) .

_:N8bb6e2dc99434de5b8d40a5c8dd67d84 rdf:first cskg-ont:OtherEntity ;
    rdf:rest () .

_:N8c0dc6b98a914d4cb24a814377be3ca4 rdf:first cskg-ont:Material ;
    rdf:rest ( cskg-ont:Method cskg-ont:Metric cskg-ont:OtherEntity cskg-ont:Task ) .

_:N8c725be6384b49be86b4bd8de124159f rdf:first cskg-ont:Method ;
    rdf:rest ( cskg-ont:Metric cskg-ont:OtherEntity cskg-ont:Task ) .

_:N8d239db890514b19a034f605f4384942 rdf:first cskg-ont:Material ;
    rdf:rest _:N4a029d256e3f4ccabd5dfedd3f8f799b .

_:N8db741d2ba1e4b3eb7d3b79444822bda rdf:first cskg-ont:Method ;
    rdf:rest ( cskg-ont:Task ) .

_:N8ecf5e69802f4f3897ba055868f38a9f rdf:first cskg-ont:Method ;
    rdf:rest _:N2d18cf49b3c04cc9a4ea4eede90ef669 .

_:N92bc57df2d1b42f28d5447f023087b71 rdf:first cskg-ont:Material ;
    rdf:rest ( cskg-ont:Method cskg-ont:OtherEntity cskg-ont:Task ) .

_:N93a23b0fe7724299b5042672ec9e063c rdf:first cskg-ont:OtherEntity ;
    rdf:rest _:N2deedadb5afa4736a373dfd38fa42c07 .

_:N94254133496d4b0caab3f18c08bc96fc rdf:first cskg-ont:Task ;
    rdf:rest () .

_:N96293f1e456e4aa1a91abfd8936512f9 rdf:first cskg-ont:Material ;
    rdf:rest _:N09a86850c1a84248bef86a1280c03fab .

_:N9632cf1022c4459695aae72752770704 rdf:first cskg-ont:Method ;
    rdf:rest _:N681184d503aa43f9a622374d73cb189f .

_:N96e1cab1e82a49c7ae6f492db5ce72a8 rdf:first cskg-ont:Method ;
    rdf:rest _:N40158b88d967434a97def16bcb94cd5d .

_:N978bce608f574d54be9750113e7c86b7 rdf:first cskg-ont:Material ;
    rdf:rest _:N76f34f6fc120407f890abc116c79e8f3 .

_:N9881ae9018924bfbbd8c9b41d0364a03 rdf:first cskg-ont:Method ;
    rdf:rest _:N2ab0f845007840f2817dbbf1e7f09161 .

_:N99ec7cf127d64de290d3f1f884202f46 rdf:first cskg-ont:Method ;
    rdf:rest _:N40cb30f91d0a4e95ba56ec763023fdd1 .

_:N9a578e7cec4b4f1ea03933303e4be01c rdf:first cskg-ont:Method ;
    rdf:rest _:N4144a6f05b134161b1b3b1111a4a6172 .

_:N9b50f8b954eb4bc18f2d5481947a8f5f rdf:first cskg-ont:Task ;
    rdf:rest () .

_:N9b568374c60c46eb95c44b8ae5045d1b rdf:first cskg-ont:Material ;
    rdf:rest ( cskg-ont:Method cskg-ont:Metric cskg-ont:OtherEntity cskg-ont:Task ) .

_:N9c6398929bb34900a9c330963fd4192b rdf:first cskg-ont:Material ;
    rdf:rest _:N0f57f9c0fb574da6b4d8eeddfb7e140f .

_:N9d7c0380d1aa4f27a595c940e9893be0 rdf:first cskg-ont:OtherEntity ;
    rdf:rest _:N9b50f8b954eb4bc18f2d5481947a8f5f .

_:N9e76422fd8884ee18717947852abf3d1 rdf:first cskg-ont:Material ;
    rdf:rest _:N4415d9965ef94e40bc097f3f8845482a .

_:N9eea739ba0204c0a81081b1e7d33e484 rdf:first cskg-ont:Method ;
    rdf:rest ( cskg-ont:OtherEntity cskg-ont:Task ) .

_:N9f732e7379154905a5d6ba424c4a7016 rdf:first cskg-ont:Method ;
    rdf:rest ( cskg-ont:OtherEntity cskg-ont:Task ) .

_:Na0259b27c17a45db9caad35db2ac940e rdf:first cskg-ont:Method ;
    rdf:rest _:N45cc845b31eb46ef95f5286ab3897d82 .

_:Na03844f48b204156b84d7736e01aa857 rdf:first cskg-ont:Method ;
    rdf:rest _:N522d819d3e7944d988c9aa0fa72aa7cc .

_:Na100b0c10ec14d30b3f2790661f5f6e3 rdf:first cskg-ont:Task ;
    rdf:rest () .

_:Na356d2df0e9f4b8f97aa289dfa302647 rdf:first cskg-ont:Method ;
    rdf:rest _:N7eddee1a91f3408daf859bda8b69f700 .

_:Na3af163922aa49cf835456d9c1ec2e0e rdf:first cskg-ont:Method ;
    rdf:rest _:N5d9a59e1221f43c69f4f26b3e4f9f613 .

_:Na4a0a43c163a4a2480fa62dc4d14c6b6 rdf:first cskg-ont:Task .

_:Na681d52fb845417888d501ff20dc90dc rdf:first cskg-ont:Task ;
    rdf:rest () .

_:Na70980d3772c4f048674783e67184426 rdf:first cskg-ont:Method ;
    rdf:rest _:N6c2147785886496b98d7fab6be269482 .

_:Naa4e219479ee432d8759ebabf17a7ed3 rdf:first cskg-ont:Metric .

_:Nabf46b7f40ae4cdd8f58b19bf4ec0121 rdf:first cskg-ont:Method ;
    rdf:rest _:N4e7a9d25374a46eaa62690a71ad33f8e .

_:Nac1e94fd760f4137bfe3e2f649a632df rdf:first cskg-ont:OtherEntity ;
    rdf:rest _:N5cbd2eda905a4956997a79fe4844496c .

_:Nac6fbfc780f04c96abbefd10268d4244 rdf:first cskg-ont:Method ;
    rdf:rest _:N257d067e1430474bb72e44c59338b853 .

_:Nad9e780e11e245feb262c42118beaeec rdf:first cskg-ont:Method ;
    rdf:rest ( cskg-ont:Metric cskg-ont:OtherEntity cskg-ont:Task ) .

_:Nae8e078731a848dd947cbe2a85f806c0 rdf:first cskg-ont:Method ;
    rdf:rest ( cskg-ont:Metric cskg-ont:Task ) .

_:Naf530c97807547b4b968d75509280201 rdf:first cskg-ont:Method ;
    rdf:rest _:N1cdab02fbcc34d56b8fc06487398d9ec .

_:Naf7fc878e3974ecdab51773457c7ed3c rdf:first cskg-ont:Method ;
    rdf:rest ( cskg-ont:Metric cskg-ont:OtherEntity cskg-ont:Task ) .

_:Nb10c9a24a3e14a7aa0fd94b2a1556274 rdf:first cskg-ont:Method ;
    rdf:rest _:N5c5efb26c95345f0829f69e6d50dc8fc .

_:Nb15e8fb36b104573ad5fb55b30465f46 rdf:first cskg-ont:Material ;
    rdf:rest _:Na70980d3772c4f048674783e67184426 .

_:Nb1c214f1420f4738b065050530135327 rdf:first cskg-ont:Material ;
    rdf:rest _:N11e9f14108554d7089f86ba543666fc1 .

_:Nb2197e4b62664a01a4fb35d3787a2d84 rdf:first cskg-ont:Material ;
    rdf:rest _:N2e9e6ef1333640e589ea584ea643f646 .

_:Nb36a7ff8a7854963a4310e91a3ba42b9 rdf:first cskg-ont:Method ;
    rdf:rest _:N9d7c0380d1aa4f27a595c940e9893be0 .

_:Nb5b38ffa33174ac59c94740eecffc0ff rdf:first cskg-ont:Method ;
    rdf:rest ( cskg-ont:Task ) .

_:Nb738ddf666eb4200a72a218e8fcc5b44 rdf:first cskg-ont:Method ;
    rdf:rest ( cskg-ont:OtherEntity ) .

_:Nb8618a57285245d587e857ead12825f9 rdf:first cskg-ont:Method ;
    rdf:rest _:N19b09e56a7074f239b7b775977ee484e .

_:Nb954154581a64ceab6e926a771eb05f5 rdf:first cskg-ont:Metric ;
    rdf:rest ( cskg-ont:OtherEntity cskg-ont:Task ) .

_:Nb9adc3514e8b445ba9ce9c38aebf8277 rdf:first cskg-ont:Material ;
    rdf:rest _:Nb10c9a24a3e14a7aa0fd94b2a1556274 .

_:Nba22dd89a8c94b3eaf63c4aa40934d23 rdf:first cskg-ont:Metric ;
    rdf:rest _:N3d2760c7b94d46f8988b575814731e67 .

_:Nbac7ff589cc44fbeb667e05ae00442e4 rdf:first cskg-ont:Metric ;
    rdf:rest _:N723e6a4163b64ad3945d01bf4348540e .

_:Nbe37745c79fd4ab689969d4c1161de0f rdf:first cskg-ont:Material ;
    rdf:rest _:N520e9a6dbcf443ee814952ffc680b7b6 .

_:Nbe565c8703474265bacc8cb84d5b4b9b rdf:first cskg-ont:Task ;
    rdf:rest () .

_:Nbea1219df12049c0bfbe855ae7a2b386 rdf:first cskg-ont:Metric ;
    rdf:rest _:N12251e1a74404f3ab76a34b31c80e154 .

_:Nbf1f096826664a98a572467c4cb1dbbc rdf:first cskg-ont:Method ;
    rdf:rest ( cskg-ont:Metric cskg-ont:OtherEntity ) .

_:Nc0682b64f8d94c5cb93b2fafffa841c9 rdf:first cskg-ont:Material ;
    rdf:rest _:N1561912a81c847a48e37f8fe62ea8da9 .

_:Nc2407a80d41e4752bd38da12f7ac9036 rdf:first cskg-ont:Method ;
    rdf:rest ( cskg-ont:Metric cskg-ont:OtherEntity cskg-ont:Task ) .

_:Nc27cc40c669e4d808654aae185022e72 rdf:first cskg-ont:Method ;
    rdf:rest _:N558198da5c4c42b3be0e39e1ffd907a7 .

_:Nc3278838c222444a8abfcbf9618f6ddd rdf:first cskg-ont:Material ;
    rdf:rest _:N2373b14852e941a6ab5afe3b9d88f739 .

_:Nc43bb1394aa0498d82d5f349078553d6 rdf:first cskg-ont:OtherEntity ;
    rdf:rest _:N94254133496d4b0caab3f18c08bc96fc .

_:Nc5faed894f284f14a0b896289729a195 rdf:first cskg-ont:Method ;
    rdf:rest _:N430f73b793f64a308b8ecaf12589c9d4 .

_:Nc606815abb864bd4a321295278fb1839 rdf:first cskg-ont:Method ;
    rdf:rest _:Na681d52fb845417888d501ff20dc90dc .

_:Nc638111f97e44827b9ca53c5852cf44f rdf:first cskg-ont:Material ;
    rdf:rest _:N61d6a5024bdb4c92b4ffc21b7a975485 .

_:Nc69d8f28eeae44b69fe557e13c871a15 rdf:first cskg-ont:Material ;
    rdf:rest _:Nad9e780e11e245feb262c42118beaeec .

_:Nc8656fb8f37f4bb394a50dfe11ba6699 rdf:first cskg-ont:Method ;
    rdf:rest _:Nbea1219df12049c0bfbe855ae7a2b386 .

_:Nc8c4767cc6ef46f8a25861820ae46988 rdf:first cskg-ont:Method ;
    rdf:rest ( cskg-ont:OtherEntity cskg-ont:Task ) .

_:Nc9d60d89e201453a827852c4171fa0b9 rdf:first cskg-ont:Method ;
    rdf:rest _:N119eaaa881924fb9a1c53daee8fb8aad .

_:Ncaa43fcc12804fc4af713d6e2d9ad1de rdf:first cskg-ont:Method ;
    rdf:rest _:N6fb0a71854ef4ba7a7e294439aea2ef0 .

_:Ncbc8ab1fa7404fc49c2c7a0c04a3e6ba rdf:first cskg-ont:Method ;
    rdf:rest ( cskg-ont:Metric cskg-ont:OtherEntity cskg-ont:Task ) .

_:Ncc6426fb211040e788d20d9a8fbb329f rdf:first cskg-ont:Material ;
    rdf:rest _:N795424ed5f9647d5afdc00248c01f343 .

_:Ncd87102e1ed241a9a2d06ba42fe83ef7 rdf:first cskg-ont:Method ;
    rdf:rest _:N80aae899d0944bc68bf342da8c5204b7 .

_:Ncdf6e2cf61dd4290a99aa498274fbec0 rdf:first cskg-ont:Metric ;
    rdf:rest _:N6a8224dd3c734e8db140d5055bfb3751 .

_:Ncdfb572572d84ac6a4f237a486287bc1 rdf:first cskg-ont:Material ;
    rdf:rest _:N8ecf5e69802f4f3897ba055868f38a9f .

_:Nce0557dbd7ae4893bc96be5698f3dc23 rdf:first cskg-ont:Method ;
    rdf:rest _:N8631ae39328c4deaa23b71a74ee76ff8 .

_:Ncfdc63e8b15f484980c654bbb381d874 rdf:first cskg-ont:Method ;
    rdf:rest _:N3a09effe5ff64429b58e4623de9425be .

_:Nd191ae0ae200481bb887f0f35d3ec2e3 rdf:first cskg-ont:Method ;
    rdf:rest _:Ncdf6e2cf61dd4290a99aa498274fbec0 .

_:Nd23715a6ce784ebea276c9b0286d577e rdf:first cskg-ont:Metric ;
    rdf:rest ( cskg-ont:OtherEntity cskg-ont:Task ) .

_:Nd3e52a04512b40b18bd59132f1f6dd79 rdf:first cskg-ont:Method ;
    rdf:rest _:N7093cb0e39414a1184d610c021faa1dc .

_:Nd4e8f33e93f546449e1f688820230547 rdf:first cskg-ont:Method ;
    rdf:rest _:Nba22dd89a8c94b3eaf63c4aa40934d23 .

_:Nd51307ed1d9d4bf69b42430837dfe01a rdf:first cskg-ont:Material ;
    rdf:rest _:Nd3e52a04512b40b18bd59132f1f6dd79 .

_:Nd54ba33077ed4ccfac4cfa540b6dfb3b rdf:first cskg-ont:OtherEntity ;
    rdf:rest _:N4c1c437c7b444582aa4c2f72c6b74e4f .

_:Nd5afc7bc15af43e789916077ea73d323 rdf:first cskg-ont:Material ;
    rdf:rest _:Nc27cc40c669e4d808654aae185022e72 .

_:Nd6025fa51b6342a7b7cb8c0b396f2920 rdf:first cskg-ont:Method ;
    rdf:rest _:N3723b329235e49c8a5b7258b6c711b1f .

_:Nd6272a8b7b4c4e03bb275c127d78968c rdf:first cskg-ont:Metric ;
    rdf:rest _:N4b7e598d1a17492eb3a9dcd8bada3f84 .

_:Nd676d456d0d7458d9adfca08c1076896 rdf:first cskg-ont:Method ;
    rdf:rest _:Nc43bb1394aa0498d82d5f349078553d6 .

_:Nd7c16df433f6442883d75a2e64b96814 rdf:first cskg-ont:Method ;
    rdf:rest _:N86f0b0f701344faa986264ea354e13e0 .

_:Nd9d3cb5042fa435d909c143c5abf5889 rdf:first cskg-ont:Method ;
    rdf:rest _:N2a286d19a6ef4645937787365e744938 .

_:Ndbe09fa2543648dfa26a5d61408b4826 rdf:first cskg-ont:Material ;
    rdf:rest _:N86c40ff5de274756a8c344a92182cce6 .

_:Ndd2ff035d7d34061b8ee1b547595359c rdf:first cskg-ont:Method ;
    rdf:rest _:N4e05af78719542ad89be8ba1f63486e3 .

_:Ne0ba79e5b12e47158b1b7b7c11a24709 rdf:first cskg-ont:Material ;
    rdf:rest _:Naf7fc878e3974ecdab51773457c7ed3c .

_:Ne3e26a5f2d07468eaa7eadf82409e8b2 rdf:first cskg-ont:Material ;
    rdf:rest _:N42a23b6e361949fa8910023566ec7e61 .

_:Ne660d8a8b28f40be8e11c6b184cefc89 rdf:first cskg-ont:Material ;
    rdf:rest _:N3098c2da615e44acb3a2f900cca7bdcb .

_:Ne7314ef2674b46eca62e0058f07e531d rdf:first cskg-ont:Material ;
    rdf:rest ( cskg-ont:Method cskg-ont:Metric cskg-ont:OtherEntity cskg-ont:Task ) .

_:Ne8d2676eeb2c418a9512972002cfe9c1 rdf:first cskg-ont:Method ;
    rdf:rest ( cskg-ont:OtherEntity cskg-ont:Task ) .

_:Ne8f861fb92844037ae957f2cb095eae7 rdf:first cskg-ont:Method ;
    rdf:rest _:Nd6272a8b7b4c4e03bb275c127d78968c .

_:Nea2961ad48ec4e35b98f125258f5a8fc rdf:first cskg-ont:Method ;
    rdf:rest _:Nd23715a6ce784ebea276c9b0286d577e .

_:Nea9fcddebb694eba888b37dfcd0e9eaf rdf:first cskg-ont:Material ;
    rdf:rest ( cskg-ont:Method cskg-ont:OtherEntity cskg-ont:Task ) .

_:Neb894581afa0459db490b19b2f570e40 rdf:first cskg-ont:Material ;
    rdf:rest _:N9eea739ba0204c0a81081b1e7d33e484 .

_:Necca16597cc740d3bda4e4bdeb17e568 rdf:first cskg-ont:Task .

_:Neda64d6d2b4e426e802c020bc69bdb4e rdf:first cskg-ont:OtherEntity ;
    rdf:rest _:N480f83d24a1c45de83a40e973ba3956a .

_:Nee485bbca21142bbaf7c8a5f9f19e5b0 rdf:first cskg-ont:Method ;
    rdf:rest _:Nb954154581a64ceab6e926a771eb05f5 .

_:Needbe9b275084955b0a3b4b061794441 rdf:first cskg-ont:Method ;
    rdf:rest _:Nbac7ff589cc44fbeb667e05ae00442e4 .

_:Nef00c76d78024dc3bf6cb12520c5c1ad rdf:first cskg-ont:Method ;
    rdf:rest _:Na100b0c10ec14d30b3f2790661f5f6e3 .

_:Nf12407bb0e7e423588239a7aa8c4fa25 rdf:first cskg-ont:Material ;
    rdf:rest _:Nac6fbfc780f04c96abbefd10268d4244 .

_:Nf1e19b5a54c14a98a1f505e2c893323a rdf:first cskg-ont:Material ;
    rdf:rest ( cskg-ont:Method cskg-ont:Metric cskg-ont:OtherEntity cskg-ont:Task ) .

_:Nf3d07dd91d9b4d488a785cb63ec3a7b3 rdf:first cskg-ont:Method ;
    rdf:rest _:N50446e187a55473ab0f0989c2ac7f867 .

_:Nf424a73fb51b4d4da172d2c4e2cff6f8 rdf:first cskg-ont:Method ;
    rdf:rest _:Nd54ba33077ed4ccfac4cfa540b6dfb3b .

_:Nf60a09212d3c42898cb80e2bcfd0d9a8 rdf:first cskg-ont:Material ;
    rdf:rest _:N93a23b0fe7724299b5042672ec9e063c .

_:Nf9d1e19cf21546c6ae3132384fa1a011 rdf:first cskg-ont:Method ;
    rdf:rest _:N186045bc966a430cb34e5a3f35a0a02b .

_:Nfa26b4d56386448b8a9a6be6105e3c9a rdf:first cskg-ont:Method ;
    rdf:rest _:N40e77d4153664c4eb14598c39d3ee18d .

_:Nfe2bdbbece0d4501aeaf5f43f05bb885 rdf:first cskg-ont:Method ;
    rdf:rest _:Neda64d6d2b4e426e802c020bc69bdb4e .

_:Nfe329097b9ee45348dcb75f440cef3bf rdf:first cskg-ont:Method ;
    rdf:rest _:N4a155d6abd7f4d4c8660cd91c540b4df .

_:N0053e46091564bada9a0447722971667 owl:unionOf _:N1cf57b2877cd4a7cb61eef8b52700525 .

_:N041d55ebb2344a4c821fed0b93a96c07 owl:unionOf _:N9c6398929bb34900a9c330963fd4192b .

_:N05212fdb40c2415597e72a670c36a9cb owl:unionOf _:N6f54ea87e09d4c618511541b6674d4d0 .

_:N05fff169cc7b47d38569f88b88d8e23f owl:unionOf _:N1eea0d6602294242a602aa68a749c1c4 .

_:N08286035189c4c1d815e149a72050a9d owl:unionOf _:N47f35a29d79543cbaa0e5cab36b29893 .

_:N08fd05694b3f44ebb87a0f020839acee owl:unionOf _:N74569c929e3d4966af0c32d0af497feb .

_:N0b422da05d3c4d2293fa30de0b98d6e1 owl:unionOf _:Ncc6426fb211040e788d20d9a8fbb329f .

_:N0b7d5a96f896460586a5c3412f211a2f owl:unionOf _:N734a6e0edb8a44bc817bc5b2ab0c746d .

_:N0bd7083d9bbc422f92e266e47b20363d owl:unionOf _:N8061d737b75b4a94b4880089ebbca371 .

_:N0c6045d04e2d4fb698e46d314ee9ca52 owl:unionOf _:Ncdfb572572d84ac6a4f237a486287bc1 .

_:N0dfe945b3ba44539b8d155270cf03b90 owl:unionOf _:N011a954ff1454870859edc81c98e13c6 .

_:N0e4608619db046fd8645d33a9c58429f owl:unionOf _:N8d239db890514b19a034f605f4384942 .

_:N0e7780581a8a4d36a89b991aa4e88270 owl:unionOf _:N6fb3b204067a486089a981cdadc94734 .

_:N0efe5afe2d9d443882349b3cf85ecb78 owl:unionOf _:N4066263359ba4b68b671418497961b7f .

_:N1067ae94682b42c18653eadaac85deff owl:unionOf _:Nc9d60d89e201453a827852c4171fa0b9 .

_:N1180ea8f3dc54e0d8b6efb545a5fd9fe owl:unionOf _:Ncaa43fcc12804fc4af713d6e2d9ad1de .

_:N1199cb3160fd4657961cd60acea9c881 owl:unionOf _:N1fe56bc13c4a4995a64686f65948fa21 .

_:N11e01c48cf0b41f8a07ab64da28f89b3 owl:unionOf _:N31aac8e62dcf413f9c5f65de23987062 .

_:N14089d541ce349aaaa4fd1b63fd36a00 owl:unionOf _:Nb8618a57285245d587e857ead12825f9 .

_:N1457e755bb5841c594cfec96662ad8f6 owl:unionOf _:N2e107529b2064bf0b902dc8bb3a3591f .

_:N153e4415eed74d11915734588e6374d6 owl:unionOf _:Na03844f48b204156b84d7736e01aa857 .

_:N15a8080dcfdb43bf8d293acae48153f4 owl:unionOf _:Nc606815abb864bd4a321295278fb1839 .

_:N1802d0de86f3405b9653a79f47cac09e owl:unionOf _:N617e921762004303a78ceaee441ffc66 .

_:N1a90f39251084963a0e43a269d1c9d13 owl:unionOf _:N9e76422fd8884ee18717947852abf3d1 .

_:N1b0212194ffc4a3eae84da8bbd9c1a17 owl:unionOf _:N8c0dc6b98a914d4cb24a814377be3ca4 .

_:N1b7fcb3709b14ff3b9f3959d221e3dca owl:unionOf _:N2c81e927804a4ff4884f1b82083fc89d .

_:N1bb86d25c9754b338b0a373bccca95bf owl:unionOf _:Nc2407a80d41e4752bd38da12f7ac9036 .

_:N1d89778f5eee4becb135ae54ea6ac098 owl:unionOf _:Ne0ba79e5b12e47158b1b7b7c11a24709 .

_:N1f3d128b6fda402dbc1b86103dfda554 owl:unionOf _:Nc8c4767cc6ef46f8a25861820ae46988 .

_:N1f6623cc3bef4f9e98932345e573de01 owl:unionOf _:Nfe2bdbbece0d4501aeaf5f43f05bb885 .

_:N20e3c93bde28431db37c1313ed671e6e owl:unionOf _:N9632cf1022c4459695aae72752770704 .

_:N238d5b5ca3454fa5bc4c9fa1a192c826 owl:unionOf _:N877e410744a94f51b2c7b485343c560d .

_:N247eb93c5ce04deba8a07ed3bdad5221 owl:unionOf _:N45e4b0c46cf4411194e41d6476691ae3 .

_:N266241773fb747198e8cee8f7c80f0ce owl:unionOf _:N21d9b923903a48b19be22b0d4b532307 .

_:N2824d69514f949f49091964a1b85a3a6 owl:unionOf _:N367e19eb79e2485886a26583cbdbe537 .

_:N2a8dec03baeb4ec8b05703ac02a71e46 owl:unionOf _:N735c56d5f6624e848d7c295c2bb2619e .

_:N2a981ddad09442f3bbf2168fd92d119a owl:unionOf _:N0babd092f4c140e18b0709bfcfbd29be .

_:N2a9dfb5c771247ff9bbfac03e665e224 owl:unionOf _:Nb2197e4b62664a01a4fb35d3787a2d84 .

_:N2aa6a5f8122f449185ed52bbf0a15b7f owl:unionOf _:Nb738ddf666eb4200a72a218e8fcc5b44 .

_:N2af9352be5834a908acd7941b06493e3 owl:unionOf _:N2c35b28be3a84d698e6f1a34ce3a4f2e .

_:N2cbdf4d21ad247858a139a0db3288bb9 owl:unionOf _:N4e18b9c498974871914b740750923559 .

_:N2ef7f44fc61b4c279d0516a584ce1183 owl:unionOf _:N6119575bf35941569c6ab7270308ab3e .

_:N3002f74f0b844bec8d66e889c133c828 owl:unionOf _:N24fb30e7071b427b81e35556f82eeb57 .

_:N30ac83d4034e493dbbf4dced9bfc0300 owl:unionOf _:Nb9adc3514e8b445ba9ce9c38aebf8277 .

_:N3104c110b5ba4b969038f41603f6014c owl:unionOf _:Ndbe09fa2543648dfa26a5d61408b4826 .

_:N325b3b8c68e44ac286527bae7a46fc96 owl:unionOf _:N70e019cdc4554e77a69a557c54a7ba48 .

_:N32d7ae61b2634b3fa1855613b102b731 owl:unionOf _:N50a61ff4df5c4b7aa826851727f92c67 .

_:N33b475fad8e94666ab0c0d8f6bb77516 owl:unionOf _:N7685e5bf7e2a47febb3eda4040f7ad79 .

_:N35e6671791614fab9c31cbb63e75adba owl:unionOf _:N81b9b4b5be0344598af89b33a25ecf02 .

_:N3a1bcb2947c843f1be540ff3d252bbe9 owl:unionOf _:N0456c28cc753463a9889c94521a23f1f .

_:N3affbed2bf194787b6196c968430d26c owl:unionOf _:Nb1c214f1420f4738b065050530135327 .

_:N3c0397721de747b089088a59bba638b3 owl:unionOf _:Nef00c76d78024dc3bf6cb12520c5c1ad .

_:N3e79eb16e49543fe827090de5929a49d owl:unionOf _:N1b3b49f603664825990870d68a672ae1 .

_:N40a65d8582d6409cae8d3048379836d9 owl:unionOf _:Nd9d3cb5042fa435d909c143c5abf5889 .

_:N4546f13a64de4f31ae43d05836a73544 owl:unionOf _:Nf3d07dd91d9b4d488a785cb63ec3a7b3 .

_:N47b3eb8ba4ff46eeae0ebc5471a01be0 owl:unionOf _:N5fe522788cde495ca1bb64e112e23502 .

_:N497f9c02321348b5a5460e2adbe2e14d owl:unionOf _:Ndd2ff035d7d34061b8ee1b547595359c .

_:N49ce4eca3edd4cc78b03a189cc38cd71 owl:unionOf _:Nd5afc7bc15af43e789916077ea73d323 .

_:N4a044612beb04386bcdaada212d06ee5 owl:unionOf _:N7e48fb8d68b64478ae57af3cddafd514 .

_:N4aeafb7a405e4e7b91141051e25e7321 owl:unionOf _:Nc5faed894f284f14a0b896289729a195 .

_:N4cb06259f0a746d599629e4aa410af9d owl:unionOf _:Nd51307ed1d9d4bf69b42430837dfe01a .

_:N4d1a78f54cdb41009c4456a977760171 owl:unionOf _:Nb15e8fb36b104573ad5fb55b30465f46 .

_:N4f8cc36c01214c6ba562824bbde43bd2 owl:unionOf _:N3aba3bf8fd7842f18b83804c7274fd83 .

_:N500da0682b05415fbc855afa0ad3b3de owl:unionOf _:N4a9f24282a744be9ab82ea96076d3b84 .

_:N502287740d5e4306a36a494e175957e8 owl:unionOf _:N6d033e34d85641729fe8c87d6787b8ce .

_:N51d8015b10504c6db235279c00bf373e owl:unionOf _:Nee485bbca21142bbaf7c8a5f9f19e5b0 .

_:N5454fd48e8d24c3ba6385a8dbd5c286e owl:unionOf _:N5ddb0f8f14544684a3c415b94afc4bbd .

_:N546ebba2acea45c98854bbcd3e5e186c owl:unionOf _:Nc69d8f28eeae44b69fe557e13c871a15 .

_:N58074e7205704ced9fcc9e9a6a38b145 owl:unionOf _:N6fcb67e71fee453b85f39b607a6a4f2d .

_:N587d559e54b447ee9b6a96be613707c2 owl:unionOf _:N0129a28476bc4a44b69b62e01577102a .

_:N5ae634f65eac4fedb488fffb891db558 owl:unionOf _:N023503d98460488bbdd07ce517757a57 .

_:N5b30fa28b8f649bc95dba7dbc8229030 owl:unionOf _:N76521fc121514fcfa869533fc5af483e .

_:N5c7e8edce3d54f2e84a531e2b82c0fb4 owl:unionOf _:N56cc45be5c6a4a0ebc5ed308f2172fee .

_:N5d064c0a456041dea42da6099d2c09a5 owl:unionOf _:Nc0682b64f8d94c5cb93b2fafffa841c9 .

_:N60a43915fb6c4bd483370f770935a5b9 owl:unionOf _:N1413d27637dd4dc58047ee00d272c5e5 .

_:N6164b28feaa64c4c9bea7aaae8ca2c72 owl:unionOf _:Nc3278838c222444a8abfcbf9618f6ddd .

_:N618060df18e6473e9d6a6ba16882c462 owl:unionOf _:Nfe329097b9ee45348dcb75f440cef3bf .

_:N643c09c87dac4699a09b44bac23ba7db owl:unionOf _:N4b5346c25d774880b44f01831511c94c .

_:N64948af7aad5415789b62c973ad807e4 owl:unionOf _:N2b8deef03b8041459b09cbac8445885e .

_:N65a40cf82d8c4baaaa10dd77428da2b4 owl:unionOf _:N34cf4ac27cd14acc8a9e5c86f40b77c4 .

_:N66dc74126f5c44409fda43db68f1be57 owl:unionOf _:N96e1cab1e82a49c7ae6f492db5ce72a8 .

_:N67712a1fb05f4cd4bd69c7bc8c6b53fb owl:unionOf _:N59a4d1ee28744c3882954a0272fc725f .

_:N689f07c9e0f04b3d90b900367988b31d owl:unionOf _:Na0259b27c17a45db9caad35db2ac940e .

_:N69404871f6734e52a230c04a387f8ba5 owl:unionOf _:Needbe9b275084955b0a3b4b061794441 .

_:N6c31b3331102496698c40fe4ec35d364 owl:unionOf _:Na4a0a43c163a4a2480fa62dc4d14c6b6 .

_:N6c9bffc4afb84f59b54c806a405408b6 owl:unionOf _:N19894926da5f445c802f7f78a4941b57 .

_:N6fbd7b79b82641238ccb201b4c0fc275 owl:unionOf _:N3b8a3884fb07482ea066c60f81fdb2bb .

_:N6fc28ae3bc614aa5a75fd033d634fbf2 owl:unionOf _:N9f732e7379154905a5d6ba424c4a7016 .

_:N70a6aff9428c4ea997f361b97a6d662c owl:unionOf _:N7fda587f2e1d46bb94743bea4bd9ef8c .

_:N729c182289a44f1cb3a3d8590f8f879c owl:unionOf _:Nd191ae0ae200481bb887f0f35d3ec2e3 .

_:N7326ea397df347f1ab490fea703779f6 owl:unionOf _:N1f6ce42b5c8e4b8abf63d1980ed56df8 .

_:N74f6d56423f346dc8b3f8d870cfd2926 owl:unionOf _:Nf60a09212d3c42898cb80e2bcfd0d9a8 .

_:N75eaaf8f7d944145995cee9c2dc4b1f4 owl:unionOf _:N120815489be6482e80d47cbe4598bd44 .

_:N76f3d2c578754615a35c5ed25ed29481 owl:unionOf _:Nabf46b7f40ae4cdd8f58b19bf4ec0121 .

_:N7737e44cf65944dc83e0afa0502ac699 owl:unionOf _:Naf530c97807547b4b968d75509280201 .

_:N77f97df3763b4e5380481a85960e8fd2 owl:unionOf _:N10c75405423145ad9b67500e6227edb8 .

_:N78e421076cfc4a1ea744c6a381116451 owl:unionOf _:N03db5811abeb473ebcfb21d29ef1e54f .

_:N7ae089cecafe4d34ae8b2bb2964db95b owl:unionOf _:Nd676d456d0d7458d9adfca08c1076896 .

_:N7b2ed255dc74415284c07048e5bd44cf owl:unionOf _:N0ee15839e545403a8684f2493e10f215 .

_:N7b68838e3777448ab5f7047aa5a6120f owl:unionOf _:N4200428de3004e1b9f8159d40a616358 .

_:N7d3fce177c8d4cb5af61d158778e6aee owl:unionOf _:N3434b435995a4420b4d116058085dc7c .

_:N8018a76176324d59bbe6d65bbdb0c9e4 owl:unionOf _:Nf1e19b5a54c14a98a1f505e2c893323a .

_:N8207716fbb6a4c14a67b17f93eb075d0 owl:unionOf _:Nb5b38ffa33174ac59c94740eecffc0ff .

_:N834f5e422e534f37a004eeed1df1d02a owl:unionOf _:N8b2d30035c8b4ef3b2abd3be57f6f26d .

_:N842e98b9e8e240b8b24fc5a53f53effa owl:unionOf _:N3c6bb5052f0e4113b86c3397056dd720 .

_:N849ae1a9a93447adb97c0b77a0f8eb8e owl:unionOf _:Ncd87102e1ed241a9a2d06ba42fe83ef7 .

_:N858c8dd2315f4e72a9b242c8785d8099 owl:unionOf _:N118f61bc94274d738cc61e8251fd7937 .

_:N8653196663b34e288e5950f343e490a8 owl:unionOf _:Nf9d1e19cf21546c6ae3132384fa1a011 .

_:N8a58b70d2de6491b9e2460616c6f8e88 owl:unionOf _:N5008815c7f54406ebfed799503327bd8 .

_:N8e228a8aba9841f88141006ed0d039c8 owl:unionOf _:Ne3e26a5f2d07468eaa7eadf82409e8b2 .

_:N8ed691a078b54c38be50433903e66463 owl:unionOf _:Ne7314ef2674b46eca62e0058f07e531d .

_:N8fe46fa8ab734ea18a302a274498734c owl:unionOf _:N6a3dedba0d57497bbaec61c28e1f7844 .

_:N9022ec3d1df544c39293f06d4a2915b4 owl:unionOf _:N2e148bde616249df9f9ea506b71853f7 .

_:N924787736fc3410a819e8c65bb11079a owl:unionOf _:N96293f1e456e4aa1a91abfd8936512f9 .

_:N955dfd3e9c954207b4ffe0c9f2f9daf2 owl:unionOf _:Nce0557dbd7ae4893bc96be5698f3dc23 .

_:N9651cd8605e0463690c4598807c85aca owl:unionOf _:N4292e225ac6a43a8873173d3288395e2 .

_:N96bcde7c4ac345708387678406877c6f owl:unionOf _:N9881ae9018924bfbbd8c9b41d0364a03 .

_:N988dc0f7e5f6414780c74ecda82f8bcb owl:unionOf _:N0b81f8e9173b4da7af9fd434760c39ec .

_:N99f8dc357c4f4b7da81b5653cc759ff7 owl:unionOf _:N978bce608f574d54be9750113e7c86b7 .

_:N9c7a820d81f24625baa100d6ee6bbd5e owl:unionOf _:N730890a7db7841dd95c4fc0711824bee .

_:N9ca46b7d5ba948fb8d1bce22a5201cb9 owl:unionOf _:N6112df70fd0e4d54adca4442ea379247 .

_:N9ee201229f954e9cb0c1d007f3277890 owl:unionOf _:Nf12407bb0e7e423588239a7aa8c4fa25 .

_:N9f08bcc4907946cfb720f28808183be3 owl:unionOf _:N075a3987b8854f719d98d1afb8b9091e .

_:Na1375b14902d42048768204c5ce0711f owl:unionOf _:Nd4e8f33e93f546449e1f688820230547 .

_:Na18faff524ce44c3a7bd793776599add owl:unionOf _:Nc8656fb8f37f4bb394a50dfe11ba6699 .

_:Na29cd5ad9ddc439d8d35a10b6625d264 owl:unionOf _:N8c725be6384b49be86b4bd8de124159f .

_:Na3b25ebacb6c48179625b2df35224994 owl:unionOf _:N6ab57cdef9aa49e39e40c8b3dc6d3b46 .

_:Na4e8e1ac70ae44409f0bd9176f121197 owl:unionOf _:Necca16597cc740d3bda4e4bdeb17e568 .

_:Na5876f2af4d34f668446c417e896ca6f owl:unionOf _:Nbf1f096826664a98a572467c4cb1dbbc .

_:Na677c9cf1eec4b199058fa4c7497de9a owl:unionOf _:Nfa26b4d56386448b8a9a6be6105e3c9a .

_:Na8087c12038741179751d08d18e7e3bc owl:unionOf _:N5b2c1a46608643829222f2c674a8abac .

_:Na8f5f43e5b904317a7bbba3fbb34a41c owl:unionOf _:N61a8dbd1937f4d31b67dbaee188c59ee .

_:Naa71c951c7094ee78260e723b1581218 owl:unionOf _:Na356d2df0e9f4b8f97aa289dfa302647 .

_:Naca3ac89fa7b4a57ae86bcc28519a296 owl:unionOf _:Nb36a7ff8a7854963a4310e91a3ba42b9 .

_:Nb30f3123fa034f52bf3b37967b773741 owl:unionOf _:N3d2f8cadfc9c4f5ba45ed135df7cb414 .

_:Nb4d555962720432b9706eed1174a7f35 owl:unionOf _:Naa4e219479ee432d8759ebabf17a7ed3 .

_:Nb537d70acb5d4f7b83ce9774ba62ee76 owl:unionOf _:N240edaabfc2c4e91893560f4141a176a .

_:Nb5fb8f3ae4ef4e2093ed8d706e47a824 owl:unionOf _:Na3af163922aa49cf835456d9c1ec2e0e .

_:Nba6a0d4144a14fc188678d3c3fff1a40 owl:unionOf _:Ncbc8ab1fa7404fc49c2c7a0c04a3e6ba .

_:Nbaa39987224f457e8b27f689c11db5c6 owl:unionOf _:Ne8f861fb92844037ae957f2cb095eae7 .

_:Nbad3c5cc49e541bcab922a7e6e1576e7 owl:unionOf _:N8704253fffa140c2ae6e7840dc66bf52 .

_:Nbc27e6b3f2f34bc39339daacb1b90191 owl:unionOf _:N6d0085797928440fbd6b1aade70beb3a .

_:Nbc785b4cd6cb4bcfa9eaa81652c25a8f owl:unionOf _:N4feb4b172418496b9cddd5491d233379 .

_:Nbcdeafe6bedf4949bb33dd323b560164 owl:unionOf _:N361a34ee78c04d41815578223f4c6713 .

_:Nbda0a556387e4fe5a06a56ee9bf2b863 owl:unionOf _:N731bf5de6d314e42b2de5c85dc84237c .

_:Nbdede62bcfd74bcd89207501aff28ae0 owl:unionOf _:N1553508c847c4d9883f924d768d7d093 .

_:Nc386a051f3e9404782512bb5046e9df6 owl:unionOf _:N4308eed296ca492584eb19c2b2c42f72 .

_:Nc42629e2ebbf4afd9c50c37db59f9d93 owl:unionOf _:N4907e29ab3de44b0b301768d30338480 .

_:Nc5e1db55c2f049efb0984d63efb8a66e owl:unionOf _:Nae8e078731a848dd947cbe2a85f806c0 .

_:Nc6e13c900be140a09f05f8a8026e8bd1 owl:unionOf _:Ncfdc63e8b15f484980c654bbb381d874 .

_:Nc935650e9b464fcc9855696059362122 owl:unionOf _:N92bc57df2d1b42f28d5447f023087b71 .

_:Nd209a2155624478ea7c6565c8ea0f04a owl:unionOf _:N29ab5816c51a475e8a7054f629b8f26b .

_:Nd3ca8cbb75dc405ca9d7fef969d2dc40 owl:unionOf _:Nea9fcddebb694eba888b37dfcd0e9eaf .

_:Nd5ef3a6440db43dfb488042b013f990a owl:unionOf _:N7f36b9e8a5df4474a59539cc0afcf3fc .

_:Nd728889fde2d409ea84799397b8adbbb owl:unionOf _:N350fe24abc3d428590192eb6697b7977 .

_:Ndc503fa6ad354569a9c6b9e17e337ef8 owl:unionOf _:N407d7f57fc85445b9a32144c59267441 .

_:Ndfef39aead1d4430a1744fb242c62a0d owl:unionOf _:N1dc8fb95861e4fc6bed44e38610589e8 .

_:Ne16adafdc323491d984944c180663627 owl:unionOf _:Ne8d2676eeb2c418a9512972002cfe9c1 .

_:Ne250491a99094a61a35c8792c5f8c59c owl:unionOf _:N011bd47746d04fc5b98754f3e568b573 .

_:Ne5f8f2eed38342769aec9a55551ff1a3 owl:unionOf _:Nd6025fa51b6342a7b7cb8c0b396f2920 .

_:Ne6c5b294919942d0a05ec31ccf7d1e5f owl:unionOf _:N1f8ce8aaf1e74ea8a1fb96b371455890 .

_:Ne749f6d04ff04b2cbee667ec125f6efb owl:unionOf _:Nea2961ad48ec4e35b98f125258f5a8fc .

_:Ne7974f69047f4510883a7ef0862ea28f owl:unionOf _:N81aa8379608142b596e531e743e8cc70 .

_:Ne820e56ea37d4cc8b0b1e18266d61899 owl:unionOf _:N99ec7cf127d64de290d3f1f884202f46 .

_:Ne84f44c11bdf4d58a6f9736f48b3ae13 owl:unionOf _:Nbe37745c79fd4ab689969d4c1161de0f .

_:Ne8dc2f8964064602885a66d293f855e5 owl:unionOf _:N9b568374c60c46eb95c44b8ae5045d1b .

_:Neada5e5673584d3b9a7f574d65dadc46 owl:unionOf _:N9a578e7cec4b4f1ea03933303e4be01c .

_:Nebf399080e1a4380a2c8f1c7401f0c10 owl:unionOf _:Nd7c16df433f6442883d75a2e64b96814 .

_:Nf0d2aa6e99b04ae6944e92df8712aec0 owl:unionOf _:N09face0f27f44b09928bdb466a779e0c .

_:Nf29389327a4f4441a7638e9b87845ca2 owl:unionOf _:N8db741d2ba1e4b3eb7d3b79444822bda .

_:Nf64606f7c1a94762924496d321d021f3 owl:unionOf _:Nc638111f97e44827b9ca53c5852cf44f .

_:Nf653e74b64c64b5fb48fb838f3e9088c owl:unionOf _:Nf424a73fb51b4d4da172d2c4e2cff6f8 .

_:Nf6875e68b52748d698406e26489862c3 owl:unionOf _:N7298627f4e284295a16a7339c4fc4813 .

_:Nf70066e61f4d46c1993c8d54a7fc726c owl:unionOf _:N6b1e46881fdf4032b4850f4d11a29e90 .

_:Nf911d4c28edc48f1bb6ec24f81c0a277 owl:unionOf _:N0d17d2e9665f44e598089a1898c44b34 .

_:Nf9274a4f2b844ee292c2dc38853f9e4c owl:unionOf _:N7f835d9496bb4b6fbb19ecee06c40b51 .

_:Nf9a039f5b7e649a9afbe2d6d8659f9fb owl:unionOf _:Neb894581afa0459db490b19b2f570e40 .

_:Nfd15102f89754dcdb6b4cea4fe32762e owl:unionOf _:Ne660d8a8b28f40be8e11c6b184cefc89 .

_:Nfe8a492d8bc446d6badfb8ef747c73f5 owl:unionOf _:N8a7962fb3418435fb18cca43f3390633 .

